new fintype branch

src/matroid.lean
@@ -3,10 +3,262 @@ Matroids, after Chapter 1 of Oxley, Matroid Theory, 1992.
 -/
 import data.finset tactic.wlog data.equiv.list tactic.find
 
-variables {α : Type*} {β : Type*} [decidable_eq α]
+variables {α : Type*} {β : Type*}
+/- For mathlib?: -/
+/- Everything from here to inter_of_subsete is by Mario Carneiro:
+https://gist.github.com/digama0/edc2a9fe4d468c3921c87650eea5b77a -/
+namespace multiset
+open nat
+
+@[simp] theorem card_filter_map_le {α β} {f : α → option β}
+  (s : multiset α) : card (filter_map f s) ≤ card s :=
+multiset.induction_on s (nat.zero_le _) begin
+  intros a s IH,
+  cases h : f a,
+  { rw [filter_map_cons_none _ _ h, card_cons],
+    exact le_succ_of_le IH, },
+  { rw [filter_map_cons_some _ _ _ h, card_cons, card_cons],
+    exact succ_le_succ IH, },
+end
+
+end multiset
 
 namespace finset
-/- For mathlib? -/
+open nat
+
+def filter_map {α β} [decidable_eq β] (f : α → option β) (s : finset α) : finset β :=
+(s.1.filter_map f).to_finset
+
+@[simp] theorem filter_map_empty {α β} [decidable_eq β] (f : α → option β) :
+  filter_map f ∅ = ∅ := rfl
+
+@[simp] theorem mem_filter_map {α β} [decidable_eq β] {f : α → option β} {s : finset α}
+  {b : β} : b ∈ s.filter_map f ↔ ∃ a ∈ s, b ∈ f a :=
+by { simp only [filter_map, exists_prop, multiset.mem_filter_map, multiset.mem_to_finset], refl, }
+
+theorem card_filter_map_le {α β} [decidable_eq β] {f : α → option β} {s : finset α} :
+  card (s.filter_map f) ≤ card s :=
+le_trans (multiset.card_le_of_le $ multiset.erase_dup_le _)
+  (multiset.card_filter_map_le _)
+
+theorem filter_map_insert_none {α β} [decidable_eq α] [decidable_eq β]
+  (f : α → option β) {a : α} {s : finset α} (hf : f a = none) :
+  filter_map f (insert a s) = filter_map f s :=
+begin
+  by_cases a ∈ s,
+  { rw insert_eq_of_mem h },
+  { simp only [filter_map, multiset.ndinsert_of_not_mem h,
+      multiset.filter_map_cons_none _ _ hf, finset.insert_val], },
+end
+
+theorem filter_map_insert_some {α β} [decidable_eq α] [decidable_eq β]
+  (f : α → option β) {a : α} {s : finset α} {b} (hf : f a = some b) :
+  filter_map f (insert a s) = insert b (filter_map f s) :=
+begin
+  by_cases a ∈ s,
+  { rw [insert_eq_of_mem h, insert_eq_of_mem],
+    exact mem_filter_map.2 ⟨_, h, hf⟩, },
+  { simp only [filter_map, multiset.ndinsert_of_not_mem h,
+      multiset.filter_map_cons_some _ _ _ hf, multiset.to_finset_cons, finset.insert_val], },
+end
+
+theorem mem_of_card_filter_map {α β} [decidable_eq α] [decidable_eq β] {f : α → option β} {s : finset α}
+  (h : card (s.filter_map f) = card s) {a} (ha : a ∈ s) : ∃ b, b ∈ f a :=
+begin
+  cases h' : f a with b, swap, {exact ⟨b, rfl⟩},
+  refine (not_succ_le_self (card (erase s a)) (_ : _ + 1 ≤ _)).elim,
+  rw [← insert_erase ha, filter_map_insert_none f h',
+    card_insert_of_not_mem (not_mem_erase _ _)] at h, rw ← h,
+  apply card_filter_map_le,
+end
+
+theorem inj_of_card_filter_map {α β} [decidable_eq α] [decidable_eq β] {f : α → option β} {s : finset α}
+  (H : card (s.filter_map f) = card s) {a a'} (ha : a ∈ s) (ha' : a' ∈ s)
+    {b} (h1 : b ∈ f a) (h2 : b ∈ f a') : a = a' :=
+begin
+  by_contra h,
+  rw [← insert_erase ha', filter_map_insert_some f h2,
+    card_insert_of_not_mem (not_mem_erase _ _), insert_eq_of_mem] at H,
+  { refine (not_succ_le_self (card (erase s a')) (_ : _ + 1 ≤ _)).elim,
+    rw ← H, apply card_filter_map_le },
+  { exact mem_filter_map.2 ⟨_, mem_erase.2 ⟨h, ha⟩, h1⟩ }
+end
+
+theorem exists_subset_filter_map_eq
+  {α β} [decidable_eq α] [decidable_eq β] (f : α → option β) (s : finset α) :
+  ∃ t ⊆ s, s.filter_map f = filter_map f t ∧ card (t.filter_map f) = card t :=
+begin
+  refine finset.induction_on s ⟨∅, by { simp only [finset.empty_subset, finset.card_empty,
+    exists_prop_of_true, finset.filter_map_empty, and_self, eq_self_iff_true] }⟩ _,
+  rintro a s as ⟨t, ss, st, ct⟩,
+  cases h : f a with b,
+  { refine ⟨t, subset.trans ss (subset_insert _ _), _, ct⟩,
+    simpa only [filter_map_insert_none f h] },
+  simp only [filter_map_insert_some f h],
+  by_cases h' : b ∈ filter_map f s,
+  { simp only [h', exists_prop, insert_eq_of_mem],
+    exact ⟨t, subset.trans ss (subset_insert _ _), st, ct⟩ },
+  { refine ⟨insert a t, _⟩,
+    have ha := mt (@ss _) as,
+    rw [filter_map_insert_some f h],
+    refine ⟨insert_subset_insert _ ss, by rw st, _⟩,
+    rw [← st, card_insert_of_not_mem h', st, ct, card_insert_of_not_mem ha], }
+end
+
+def finset_embed {X : finset α} (S : finset {x // x ∈ X}) : finset α :=
+S.map $ function.embedding.subtype _
+
+lemma finset_embed_inj {X : finset α} : function.injective
+  (λ (S : finset {x // x ∈ X}), finset_embed S):=
+begin
+  unfold function.injective,
+  intros S T h,
+  simp only [ext, subtype.forall] at h ⊢,
+  intros a ha,
+  simp only [finset_embed, function.embedding.subtype, exists_prop,
+    exists_and_distrib_right, exists_eq_right, function.embedding.coe_fn_mk, mem_map,
+    subtype.exists] at h,
+  exact iff.intro (λ H, exists.elim ((h a).mp (exists.intro ha H)) (λ ha_, id))
+    (λ H, exists.elim ((h a).mpr (exists.intro ha H)) (λ ha_, id)),
+end
+
+instance finset_embed_coe (X : finset α) : has_coe (finset {x : α // x ∈ X}) (finset α) :=
+⟨finset_embed⟩
+
+def finset_finset_embed {X : finset α} (S : finset (finset {x // x ∈ X})) : finset (finset α) :=
+S.map $ ⟨finset_embed, finset_embed_inj⟩
+
+instance finset_finset_embed_coe (X : finset α) : has_coe (finset (finset {x : α // x ∈ X}))
+  (finset (finset α)) :=
+⟨finset_finset_embed⟩
+
+-- need some basic theorems about finset_finset_embed_coe
+
+lemma finset_embed_coe_def {X : finset α} (S : finset {x // x ∈ X}) : ↑S = finset_embed S :=
+rfl
+
+lemma finset_finset_embed_coe_def {X : finset α} (S : finset (finset {x // x ∈ X})) : ↑S = finset_finset_embed S :=
+rfl
+
+/-lemma finset_embed_mem_univ {X : finset α} (x : finset {a // a ∈ X}) : (↑x : α) ∈ X :=
+begin
+end-/
+
+lemma finset_embed_subset_univ {X : finset α} (S : finset {a // a ∈ X}) : ↑S ⊆ X :=
+by { simp only [subset_iff, finset_embed_coe_def, finset_embed, function.embedding.subtype,
+    exists_prop, exists_and_distrib_right, exists_eq_right, function.embedding.coe_fn_mk,
+    mem_map, subtype.exists, exists_imp_distrib],
+  exact λ _ ha _, ha, }
+
+lemma finset_embed_mem {X : finset α} {S : finset {a : α // a ∈ X}} {x : {a : α // a ∈ X}} :
+  x ∈ S ↔ x.val ∈ (↑S : finset α) :=
+by { simp only [finset_embed_coe_def, finset_embed, function.embedding.subtype,
+    exists_prop, exists_and_distrib_right, subtype.eta, exists_eq_right,
+    function.embedding.coe_fn_mk, mem_map, subtype.exists],
+  exact iff.intro (λ h, ⟨x.2, mem_def.mp h⟩) (λ h, h.2), }
+
+/-lemma finset_embed_finset_mem {X : finset α} {S : finset (finset {a : α // a ∈ X})}
+  {x : finset {a : α // a ∈ X}} : x ∈ S ↔ ↑x ∈ (↑S) :=
+sorry-/
+/-
+lemma aux : insert e ↑x = ↑(insert e x) := sorry-/
+
+lemma finset_embed_subset {X : finset α} {x y : finset {a // a ∈ X}} :
+  x ⊆ y ↔ ↑x ⊆ (↑y : finset α) :=
+by { simp only [subset_iff, finset_embed_coe_def, finset_embed, function.embedding.subtype,
+    exists_prop, exists_and_distrib_right, exists_eq_right, function.embedding.coe_fn_mk,
+    mem_map, subtype.forall, subtype.exists, exists_imp_distrib],
+  exact iff.intro (λ h a ha H, exists.intro ha (h a ha H))
+    (λ h a ha H, exists.elim (h ha H) (λ ha_ hay, hay)), }
+
+lemma finset_embed_card [decidable_eq α] {X : finset α} (x : finset {a // a ∈ X}) : card x = card (↑x : finset α) :=
+by { rw [finset_embed_coe_def, finset_embed],
+  exact (map_eq_image (function.embedding.subtype _) x).symm ▸
+    (card_image_of_injective x (function.embedding.subtype _).2).symm, }
+
+section prestrict
+variables [decidable_eq α] [fintype α]
+
+/-- def by Mario Carneiro https://leanprover.zulipchat.com/#narrow/stream/113489-new-members/subject/finset.20of.20subtype.20from.20filter/near/134578668 -/
+def prestrict (X : finset α) (I : finset α) : option (finset {x : α // x ∈ X}) :=
+if h : _ then some
+  ⟨I.1.pmap (λ x h', ⟨x, h'⟩) h,
+    multiset.nodup_pmap (λ _ _ _ _, subtype.mk_eq_mk.1) I.2⟩ else none
+
+lemma prestrict_eq_none {X : finset α} (I : finset α) : prestrict X I = none ↔ ¬ I ⊆ X :=
+begin
+  split,
+  { intros h hIX,
+    by_cases H : ∀ a, a ∈ I.val → a ∈ X,
+    { change dite _ _ _ = none at h,
+      rw dif_pos H at h,
+      cases h, },
+    { rcases not_forall.1 H with ⟨x, hx⟩,
+      rw [not_imp, ←mem_def] at hx,
+      exact hx.2 (hIX hx.1), }, },
+  { intro hIX,
+    exact dif_neg hIX, },
+end
+
+lemma prestrict_eq_some_aux {X : finset α} {I : finset α} (h : ∀ a, a ∈ I.val → a ∈ X) :
+  let I' : finset {x // x ∈ X} :=
+    {val := multiset.pmap (λ x h', ⟨x, h'⟩) (I.val) h,
+    nodup := prestrict._proof_1 X I h} in
+  ↑I' = I :=
+begin
+  intro I',
+  rw [←val_inj, finset_embed_coe_def, finset_embed, map_val, multiset.map_pmap, le_antisymm_iff],
+  split,
+  { have hnodup := multiset.nodup_pmap _ I.2,
+    rw [multiset.le_iff_subset hnodup, multiset.subset_iff],
+    { intros x hx,
+      rw multiset.mem_pmap at hx,
+      rcases hx with ⟨a, haI, H⟩,
+      convert haI,
+      subst H,
+      refl, },
+    intros a ha b hb H,
+    have hinj : (⟨a, ha⟩ : {x // x ∈ X}) = ⟨b, hb⟩ := (function.embedding.subtype _).2 H,
+    exact subtype.mk_eq_mk.1 hinj, },
+  { rw [multiset.le_iff_subset I.2, multiset.subset_iff],
+    intros x hx,
+    rw multiset.mem_pmap,
+    use [x, hx],
+    refl, },
+end
+
+lemma prestrict_eq_some_of_subset {X : finset α} {I : finset α} (h : I ⊆ X)
+  : ∃ I', prestrict X I = some I' ∧ ↑I' = I :=
+begin
+  let I' := _,
+  have : prestrict X I = some I' := dif_pos h,
+  use [I', this],
+  exact prestrict_eq_some_aux h,
+end
+
+lemma subset_of_prestrict_eq_some {X : finset α} {I : finset α} {I' : finset {x : α // x ∈ X}}
+  (h : prestrict X I = some I') : I ⊆ X ∧ ↑I' = I :=
+begin
+  by_cases H : ∀ a, a ∈ I.val → a ∈ X,
+  { split,
+    { exact H, },
+    { change dite _ _ _ = _ at h,
+      rw [dif_pos H, option.some_inj] at h,
+      subst h,
+      exact prestrict_eq_some_aux H, }, },
+  { exfalso,
+    change dite _ _ _ = _ at h,
+    rw dif_neg H at h,
+    cases h, },
+end
+
+def prestrict_subset {X Y : finset α} (h : X ⊆ Y) : finset {x // x ∈ Y} :=
+sorry
+
+end prestrict
+
+variable [decidable_eq α]
+
 lemma inter_of_subset {A B : finset α} (h : A ⊆ B) : A ∩ B = A :=
 lattice.inf_of_le_left h
 
@@ -14,7 +266,7 @@ lemma subset_iff_sdiff_eq_empty {x y : finset α} : x ⊆ y ↔ x \ y = ∅ :=
 by simp only [sdiff_eq_filter, eq_empty_iff_forall_not_mem, subset_iff, not_and,
   not_not, finset.mem_filter]
 
-lemma empty_sdiff (E : finset α): E \ ∅ = E :=
+lemma empty_sdiff (E : finset α) : E \ ∅ = E :=
 by simp only [ext, finset.not_mem_empty, and_true, iff_self, finset.mem_sdiff,
   not_false_iff, forall_true_iff]
 
@@ -23,7 +275,7 @@ lemma sdiff_subset (A B : finset α): A \ B ⊆ A :=
 
 lemma sdiff_eq_sdiff_inter (A B : finset α) : A \ B = A \ (A ∩ B) :=
 by { simp only [ext, not_and, mem_sdiff, mem_inter],
-  exact λ a, iff.intro (λ h, ⟨h.1, λ x, h.2⟩) (λ h, ⟨h.1, h.2 h.1⟩) }
+  exact λ a, iff.intro (λ h, ⟨h.1, λ x, h.2⟩) (λ h, ⟨h.1, h.2 h.1⟩), }
 
 lemma card_eq_inter_sdiff (A B : finset α) : card A = card (A ∩ B) + card (A \ B) :=
 begin
@@ -32,7 +284,7 @@ begin
       (by { intro ha, by_cases h : a ∈ B, { exact or.inl ⟨ha, h⟩ }, { exact or.inr ⟨ha, h⟩ } }) },
   have : disjoint (A \ B) (A ∩ B) := by simp only [disjoint, empty_subset, inf_eq_inter,
     inter_empty, sdiff_inter_self, inter_left_comm, le_iff_subset],
-  replace this := card_disjoint_union this, rwa [hA, add_comm] at this
+  replace this := card_disjoint_union this, rwa [hA, add_comm] at this,
 end
 
 lemma card_sdiff_eq (A B : finset α) : card (A \ B) = card A - card (A ∩ B) :=
@@ -48,7 +300,7 @@ begin
     (congr_arg card $ union_sdiff_self_eq_union.symm).substr (card_disjoint_union Hdis).symm,
   calc
   card A + card B = card A + card (B \ A) + card (A ∩ B) : by rw [add_assoc, hBA]
-  ... = card (A ∪ B) + card (A ∩ B) : by rw H
+  ... = card (A ∪ B) + card (A ∩ B) : by rw H,
 end
 
 /- proof by Kenny Lau https://leanprover.zulipchat.com/#narrow/stream/113489-new-members/subject/choosing.20from.20difference.20of.20finsets/near/133624012 -/
@@ -80,7 +332,7 @@ instance decidable_not_forall (c₁ : finset (finset α)) :
 decidable_of_iff (∃ x ∈ c₁, Q x) $ by simp only [exists_prop, not_forall_not]
 
 instance decidable_exists_and_mem : decidable (∃ e, e ∈ F ∧ P e) :=
-decidable_of_iff (∃ e ∈ F, P e) $ by simp only [exists_prop, not_forall_not]
+decidable_of_iff (∃ e ∈ F, P e) $ by simp only [exists_prop]
 
 end inst
 
@@ -92,149 +344,158 @@ open finset
 
 namespace matroid
 
-variables {E : finset α}
+variables (E : Type*) [decidable_eq E] [fintype E]
 
-/-- `indep E` is the type of matroids (encoded as systems of independent sets) with ground set `E` :
-`finset α` -/
-structure indep (E : finset α) :=
-(indep : finset (finset α))
-(indep_subset_powerset_ground : indep ⊆ powerset E)
+/-- `indep E` is the type of matroids (in the independent set representation)
+with ground set `E` (encoded in Lean as a fintype). -/
+structure of_indep :=
+(indep : finset (finset E))
 -- (I1)
 (empty_mem_indep : ∅ ∈ indep)
 -- (I2)
 (indep_of_subset_indep {x y} (hx : x ∈ indep) (hyx : y ⊆ x) : y ∈ indep)
 -- (I3)
-(indep_exch {x y} (hx : x ∈ indep) (hy : y ∈ indep) (hcard : card x < card y)
+(indep_exch {x y : finset E} (hx : x ∈ indep) (hy : y ∈ indep) (hcard : card x < card y)
     : ∃ e, e ∈ y \ x ∧ insert e x ∈ indep)
---attribute [class] indep
 
-instance indep_repr [has_repr α] (E : finset α) : has_repr (indep E) :=
+
+namespace of_indep
+
+instance repr [has_repr E] : has_repr (of_indep E) :=
 ⟨λ m, has_repr.repr m.indep⟩
 
-theorem eq_of_indep_eq : ∀ {M₁ M₂ : indep E}, M₁.1 = M₂.1 → M₁ = M₂
-  | ⟨I₁, p₁, q₁, r₁, s₁⟩ ⟨I₂, p₂, q₂, r₂, s₂⟩ h :=
+variable {E}
+
+theorem eq_of_indep_eq : ∀ {M₁ M₂ : of_indep E}, M₁.1 = M₂.1 → M₁ = M₂
+  | ⟨I₁, p₁, q₁, r₁⟩ ⟨I₂, p₂, q₂, r₂⟩ h :=
 by simpa only []
 
 /-- A circuit of a matroid is a minimal dependent subset of the ground set -/
-def is_circuit (x : finset α) (m : indep E) : Prop :=
+def is_circuit (x : finset E) (m : of_indep E) : Prop :=
 x ∉ m.indep ∧ ∀ y, y ⊂ x → y ∈ m.indep
 
 /-- proof by Mario Carneiro https://leanprover.zulipchat.com/#narrow/stream/113489-new-members/subject/finsets.2C.20decidable_mem.2C.20and.20filter/near/133708937 -/
-instance decidable_circuit (x : finset α) (m : indep E) : decidable (is_circuit x m) :=
+instance decidable_circuit (x : finset E) (m : of_indep E) : decidable (is_circuit x m) :=
 decidable_of_iff (x ∉ m.indep ∧ ∀ y ∈ (powerset x).erase x, y ∈ m.indep)
 begin
   simp only [is_circuit, has_ssubset.ssubset, mem_powerset, and_imp, mem_erase],
   refine and_congr iff.rfl (forall_congr $ λ y, _),
   refine ⟨λ H h₁ h₂, H (mt _ h₂) h₁, λ H h₁ h₂, H h₂ $ mt _ h₁⟩,
-  { rintro rfl, refl }, { exact subset.antisymm h₂ }
+  { rintro rfl, refl }, { exact subset.antisymm h₂, },
 end
 
-instance decidable_circuit_subset (x : finset α) (m : indep E) :
-  decidable (∃ (y : finset α) (H : y ⊆ x), is_circuit y m) :=
-decidable_of_iff (∃ (y : finset α) (H : y ∈ powerset x), is_circuit y m) $
+instance decidable_circuit_subset (x : finset E) (m : of_indep E) :
+  decidable (∃ (y : finset E) (H : y ⊆ x), is_circuit y m) :=
+decidable_of_iff (∃ (y : finset E) (H : y ∈ powerset x), is_circuit y m) $
   by simp only [exists_prop, mem_powerset]
 
 /- should I make this definition reducible? I don't know when to use attributes... -/
-def circuits_circ_of_indep (m : indep E) : finset (finset α) :=
-(powerset E).filter (λ S, is_circuit S m)
+def circuits_circuits (m : of_indep E) : finset (finset E) :=
+(powerset univ).filter (λ S, is_circuit S m)
 
-lemma C2_of_indep (m : indep E) (x y : finset α) (hx : x ∈ circuits_circ_of_indep m)
-  (hy : y ∈ circuits_circ_of_indep m) (hxy : x ⊆ y) : x = y :=
+lemma C2 (m : of_indep E) (x y : finset E) (hx : x ∈ circuits_circuits m)
+  (hy : y ∈ circuits_circuits m) (hxy : x ⊆ y) : x = y :=
 begin
-  simp only [circuits_circ_of_indep, is_circuit, mem_filter] at *,
+  simp only [circuits_circuits, is_circuit, mem_filter] at hx hy hxy,
   have hnxy : ¬x ⊂ y := λ h, hx.2.1 $ hy.2.2 x h,
-  rw ←lt_iff_ssubset at hnxy, rw [←le_iff_subset, le_iff_eq_or_lt] at hxy,
-  exact or.elim hxy id (λ hxy2, false.elim $ hnxy hxy2)
+  rw ←lt_iff_ssubset at hnxy,
+  rw [←le_iff_subset, le_iff_eq_or_lt] at hxy,
+  cases hxy,
+  { exact hxy, },
+  { exact (hnxy hxy).elim, },
 end
 
-theorem dep_iff_circuit_subset {x : finset α} (m : indep E) :
-  x ⊆ E → (x ∉ m.indep ↔ ∃ y ⊆ x, is_circuit y m) :=
-λ hxE, iff.intro (λ hxd, exists.elim (min_fun_of_ne_empty card (ne_empty_of_mem $
-    mem_filter.mpr ⟨mem_powerset.mpr $ subset.refl x, hxd⟩)) $
-  λ a ha, exists.elim ha $
-    λ ha2 hamin, exists.intro a $ have hax : a ⊆ x := mem_powerset.mp (mem_filter.mp ha2).1,
-      exists.intro hax $ by { unfold is_circuit,
-        exact ⟨(mem_filter.mp ha2).2, by { intros y hy, by_contra h,
-          exact not_le_of_lt (card_lt_card hy) (hamin y $ mem_filter.mpr ⟨mem_powerset.mpr $
-            subset.trans (le_of_lt $ lt_iff_ssubset.mpr hy) hax, h⟩) }⟩ }) $
-  λ H, exists.elim H $ λ a ha, exists.elim ha $
-    by { intros hax hacirc hxi, unfold is_circuit at hacirc,
-    exact hacirc.1 (m.indep_of_subset_indep hxi hax) }
+theorem dep_iff_circuit_subset (x : finset E) (m : of_indep E) :
+  x ∉ m.indep ↔ ∃ y ⊆ x, is_circuit y m :=
+begin
+  split,
+  { intro hxd,
+    rcases min_fun_of_ne_empty card (ne_empty_of_mem $
+      mem_filter.mpr ⟨mem_powerset.mpr $ subset.refl x, hxd⟩) with ⟨a, ha, hamin⟩,
+    have hax : a ⊆ x := mem_powerset.mp (mem_filter.mp ha).1,
+    use [a, hax], split,
+    { exact (mem_filter.mp ha).2, },
+    { intros y hy, by_contra h,
+      refine not_le_of_lt (card_lt_card hy) _,
+      refine hamin y (mem_filter.mpr ⟨_, h⟩),
+      refine mem_powerset.mpr (subset.trans _ hax),
+      exact (le_of_lt $ lt_iff_ssubset.mpr hy), } },
+  { rintros ⟨a, ⟨hax, hacirc⟩⟩ hxi,
+    exact hacirc.1 (m.indep_of_subset_indep hxi hax), },
+end
 
 /-- Lemma 1.1.3 -/
-lemma C3_of_indep (m : indep E) (x y : finset α) (e : α) (hx : x ∈ circuits_circ_of_indep m)
-  (hy : y ∈ circuits_circ_of_indep m) (hxny : x ≠ y) (he : e ∈ x ∩ y) :
-  ∃ z, z ∈ circuits_circ_of_indep m ∧ z ⊆ erase (x ∪ y) e :=
-have hxmy : x \ y ≠ ∅ := mt subset_iff_sdiff_eq_empty.mpr $ mt (C2_of_indep m x y hx hy) hxny,
-  exists.elim (exists_mem_of_ne_empty hxmy) $
-    by { clear hxny hxmy,
-    intros a ha, simp only [circuits_circ_of_indep, mem_powerset, mem_filter, mem_sdiff, mem_inter]
-      at ha hx hy he,
-    have hxai : erase x a ∈ m.indep := by { unfold is_circuit at hx,
-      exact hx.2.2 (erase x a) (erase_ssubset ha.1) },
-    let F := (powerset (x ∪ y)).filter (λ S, erase x a ⊆ S ∧ S ∈ m.indep),
-    have hxaF : erase x a ∈ F := mem_filter.2 ⟨mem_powerset.mpr $ subset.trans (erase_subset a x) $
-      @subset_union_left _ _ x y, ⟨subset.refl _, hxai⟩⟩, clear hxai,
-    exact exists.elim (max_fun_of_ne_empty card $ ne_empty_of_mem hxaF)
-      (λ I hEI2, exists.elim hEI2 $ by { clear hxaF hEI2,
-        exact λ hIF hI,
-          have hIFindep : I ∈ m.indep := (mem_filter.mp hIF).2.2,
-          have hIdep : _ → I ∉ m.indep := (dep_iff_circuit_subset m $ mem_powerset.1 $
-            m.indep_subset_powerset_ground hIFindep).2,
-          have hIFxa : erase x a ⊆ I := (mem_filter.mp hIF).2.1,
-          have hIxuy : I ⊆ x ∪ y := mem_powerset.mp (mem_filter.mp hIF).1,
-          have haniI : a ∉ I :=
-            λ H, have hxI : x ⊆ I := (insert_erase ha.1) ▸ insert_subset.mpr ⟨H, hIFxa⟩,
-              have ∃ A ⊆ I, is_circuit A m := exists.intro x (exists.intro hxI hx.2),
-              hIdep this hIFindep,
-          have hEg : ∃ g ∈ y, g ∉ I :=
-            by { have hIdep2 := mt hIdep, simp only [not_exists, exists_prop, not_and, not_not]
-              at hIdep2,
-            have hyI0 := mt (hIdep2 hIFindep y), simp only [not_not] at hyI0,
-            have hYI : ¬y ⊆ I := hyI0 hy.2,
-            have this := exists_mem_of_ne_empty (mt subset_iff_sdiff_eq_empty.mpr hYI),
-            simp only [mem_sdiff] at this, simpa only [exists_prop] },
-          exists.elim hEg $ λ g hEg2, exists.elim hEg2 $ by { clear hEg hEg2 hIdep,
-            intros hgy hgnI,
-            have hga : g ≠ a := λ H, ha.2 (H ▸ hgy),
-            have hIag : I ⊆ erase (erase (x ∪ y) a) g :=
-              subset_iff.mpr (λ xx hxx, mem_erase.mpr ⟨λ hgg, hgnI $ hgg ▸ hxx,
-                mem_erase.mpr ⟨λ hgga, haniI $ hgga ▸ hxx, mem_of_subset hIxuy hxx⟩⟩),
-            have haxuy : a ∈ x ∪ y := mem_union_left y ha.1,
-            have hcardxye : card (erase (x ∪ y) a) = nat.pred (card (x ∪ y)) :=
-              card_erase_of_mem haxuy,
-            have hpcard : nat.pred (card (x ∪ y)) > 0 := by { rw ←hcardxye,
-              exact card_pos.mpr (ne_empty_of_mem $ mem_erase.mpr ⟨hga, mem_union_right x hgy⟩) },
-            have hcard : card I < card (erase (x ∪ y) e) :=
-              calc card I ≤ card (erase (erase (x ∪ y) a) g) : card_le_of_subset hIag
-              ... = nat.pred (nat.pred (card (x ∪ y))) : by rw [card_erase_of_mem
-                (mem_erase.mpr ⟨hga, mem_union_right x hgy⟩), hcardxye]
-              ... < card (erase (x ∪ y) e) :
-                by { rw [card_erase_of_mem (mem_union_left y he.1),
-                ←nat.succ_pred_eq_of_pos hpcard], exact nat.lt_succ_self _ },
-            clear hga hIag haxuy hcardxye hpcard he,
-            by_contra h, simp only [circuits_circ_of_indep, mem_powerset, not_exists, and_imp,
-              mem_filter, not_and] at h,
-            have hinE : erase (x ∪ y) e ⊆ E :=
-              subset.trans (erase_subset e (x ∪ y)) (union_subset hx.1 hy.1),
-            have : (∀ x_1 : finset α, x_1 ⊆ erase (x ∪ y) e → ¬is_circuit x_1 m) :=
-              λ x1 hx1, (mt $ h x1 $ subset.trans hx1 hinE) $ not_not.mpr hx1,
-            have hindep := mt (dep_iff_circuit_subset m hinE).mp,
-              simp only [not_exists, exists_prop, not_and, not_not] at hindep,
-            replace hindep : erase (x ∪ y) e ∈ m.indep := hindep this,
-            have hfinal := m.indep_exch hIFindep hindep hcard,
-            exact exists.elim hfinal (λ El ⟨hElxy, hElindep⟩,
-              have hElF : insert El I ∈ F := mem_filter.mpr ⟨mem_powerset.mpr
-                (insert_subset.mpr ⟨(mem_erase.mp (mem_sdiff.mp hElxy).1).2, hIxuy⟩),
-                ⟨subset.trans hIFxa (subset_insert El I), hElindep⟩⟩,
-              have hcardEl : card I < card (insert El I) :=
-                by { rw card_insert_of_not_mem (mem_sdiff.mp hElxy).2,
-                exact lt_add_one (card I) },
-              not_lt.mpr (hI (insert El I) hElF) hcardEl) } }) }
+lemma C3 (m : of_indep E) (x y : finset E) (e : E) (hx : x ∈ m.circuits_circuits)
+  (hy : y ∈ m.circuits_circuits) (hxny : x ≠ y) (he : e ∈ x ∩ y) :
+  ∃ z, z ∈ m.circuits_circuits ∧ z ⊆ erase (x ∪ y) e :=
+begin
+  have hxmy : x \ y ≠ ∅ := mt subset_iff_sdiff_eq_empty.mpr (mt (m.C2 x y hx hy) hxny),
+  rcases exists_mem_of_ne_empty hxmy with ⟨a, ha⟩, clear hxny hxmy,
+  simp only [circuits_circuits, mem_powerset, mem_filter, mem_sdiff, mem_inter]
+    at ha hx hy he,
+  have hxai : erase x a ∈ m.indep := by { unfold is_circuit at hx,
+    exact hx.2.2 (erase x a) (erase_ssubset ha.1) },
+  let F := (powerset (x ∪ y)).filter (λ S, erase x a ⊆ S ∧ S ∈ m.indep),
+  have hxaF : erase x a ∈ F := mem_filter.2 ⟨mem_powerset.mpr $ subset.trans (erase_subset a x) $
+    subset_union_left x y, ⟨subset.refl _, hxai⟩⟩, clear hxai,
+  rcases (max_fun_of_ne_empty card $ ne_empty_of_mem hxaF) with ⟨I, ⟨hIF, hI⟩⟩, clear hxaF,
+  have hIFindep : I ∈ m.indep := (mem_filter.mp hIF).2.2,
+  have hIdep : _ → I ∉ m.indep := (dep_iff_circuit_subset I m).2,
+  have hIFxa : erase x a ⊆ I := (mem_filter.mp hIF).2.1,
+  have hIxuy : I ⊆ x ∪ y := mem_powerset.mp (mem_filter.mp hIF).1,
+  have haniI : a ∉ I :=
+    λ H, have hxI : x ⊆ I := (insert_erase ha.1) ▸ insert_subset.mpr ⟨H, hIFxa⟩,
+      have ∃ A ⊆ I, is_circuit A m := exists.intro x (exists.intro hxI hx.2),
+      hIdep this hIFindep,
+  have hEg : ∃ g ∈ y, g ∉ I :=
+    by { have hIdep2 := mt hIdep, simp only [not_exists, exists_prop, not_and, not_not]
+      at hIdep2,
+    have hyI0 := mt (hIdep2 hIFindep y), simp only [not_not] at hyI0,
+    have hYI : ¬y ⊆ I := hyI0 hy.2,
+    have this := exists_mem_of_ne_empty (mt subset_iff_sdiff_eq_empty.mpr hYI),
+    simp only [mem_sdiff] at this, simpa only [exists_prop], },
+  rcases hEg with ⟨g, ⟨hgy, hgnI⟩⟩, clear hIdep,
+  have hga : g ≠ a := λ H, ha.2 (H ▸ hgy),
+  have hIag : I ⊆ erase (erase (x ∪ y) a) g :=
+    subset_iff.mpr (λ xx hxx, mem_erase.mpr ⟨λ hgg, hgnI $ hgg ▸ hxx,
+      mem_erase.mpr ⟨λ hgga, haniI $ hgga ▸ hxx, mem_of_subset hIxuy hxx⟩⟩),
+  have haxuy : a ∈ x ∪ y := mem_union_left y ha.1,
+  have hcardxye : card (erase (x ∪ y) a) = nat.pred (card (x ∪ y)) :=
+    card_erase_of_mem haxuy,
+  have hpcard : nat.pred (card (x ∪ y)) > 0 := by { rw ←hcardxye,
+    exact card_pos.mpr (ne_empty_of_mem $ mem_erase.mpr ⟨hga, mem_union_right x hgy⟩), },
+  have hcard : card I < card (erase (x ∪ y) e) :=
+    calc card I ≤ card (erase (erase (x ∪ y) a) g) : card_le_of_subset hIag
+    ... = nat.pred (nat.pred (card (x ∪ y))) : by rw [card_erase_of_mem
+      (mem_erase.mpr ⟨hga, mem_union_right x hgy⟩), hcardxye]
+    ... < card (erase (x ∪ y) e) :
+      by { rw [card_erase_of_mem (mem_union_left y he.1),
+      ←nat.succ_pred_eq_of_pos hpcard], exact nat.lt_succ_self _, },
+  clear hga hIag haxuy hcardxye hpcard he,
+  by_contra h, simp only [circuits_circuits, mem_powerset, not_exists, and_imp,
+    mem_filter, not_and] at h,
+  have : (∀ x_1 : finset E, x_1 ⊆ erase (x ∪ y) e → ¬is_circuit x_1 m) :=
+    λ x1 hx1, (mt $ h x1 $ subset_univ x1) $ not_not.mpr hx1,
+  have hindep := mt (dep_iff_circuit_subset (erase (x ∪ y) e) m).mp,
+  simp only [not_exists, exists_prop, not_and, not_not] at hindep,
+  replace hindep : erase (x ∪ y) e ∈ m.indep := hindep this,
+  rcases (m.indep_exch hIFindep hindep hcard) with ⟨El, ⟨hElxy, hElindep⟩⟩,
+  have hElF : insert El I ∈ F := mem_filter.mpr ⟨mem_powerset.mpr
+    (insert_subset.mpr ⟨(mem_erase.mp (mem_sdiff.mp hElxy).1).2, hIxuy⟩),
+    ⟨subset.trans hIFxa (subset_insert El I), hElindep⟩⟩,
+  have hcardEl : card I < card (insert El I) :=
+    by { rw card_insert_of_not_mem (mem_sdiff.mp hElxy).2,
+    exact lt_add_one (card I), },
+  exact not_lt.mpr (hI (insert El I) hElF) hcardEl,
+end
 
-structure circuits (E : finset α) :=
-(circuits : finset (finset α))
-(circuits_subset_powerset_ground : circuits ⊆ powerset E)
+end of_indep
+
+open of_indep
+variable (E)
+
+structure of_circuits :=
+(circuits : finset (finset E))
 -- (C1)
 (empty_not_mem_circuits : ∅ ∉ circuits)
 -- (C2)
@@ -244,338 +505,400 @@ structure circuits (E : finset α) :=
   ∃ z, z ∈ circuits ∧ z ⊆ erase (x ∪ y) e)
 --attribute [class] circuits
 
-instance circuits_repr [has_repr α] (E : finset α) : has_repr (circuits E) :=
+namespace of_circuits
+
+instance repr [has_repr E] : has_repr (of_circuits E) :=
 ⟨λ c, has_repr.repr c.circuits⟩
 
-theorem eq_of_circ_eq : ∀ {C₁ C₂ : circuits E}, C₁.1 = C₂.1 → C₁ = C₂
-  | ⟨c₁, p₁, q₁, r₁, s₁⟩ ⟨c₂, p₂, q₂, r₂, s₂⟩ h :=
+variable {E}
+
+theorem eq_of_circ_eq : ∀ {C₁ C₂ : of_circuits E}, C₁.1 = C₂.1 → C₁ = C₂
+  | ⟨c₁, p₁, q₁, r₁⟩ ⟨c₂, p₂, q₂, r₂⟩ h :=
 by simpa only []
 
-def circuits_of_indep (m : indep E) : circuits E :=
-{ circuits := circuits_circ_of_indep m,
-  circuits_subset_powerset_ground := filter_subset _,
+end of_circuits
+
+namespace of_indep
+
+variable {E}
+
+def circuits (m : of_indep E) : of_circuits E :=
+{ circuits := m.circuits_circuits,
   empty_not_mem_circuits :=
     begin
-      simp only [circuits_circ_of_indep, is_circuit, mem_filter, not_and],
-      exact λ h h1, (h1 m.empty_mem_indep).elim
+      simp only [circuits_circuits, is_circuit, mem_filter, not_and],
+      intros h h1, exfalso,
+      exact h1 m.empty_mem_indep,
     end,
-  circuits_eq_of_subset := C2_of_indep m,
-  circuit_elim := C3_of_indep m }
+  circuits_eq_of_subset := m.C2,
+  circuit_elim := m.C3 }
+
+end of_indep
+
+namespace of_circuits
+open of_indep
+variable {E}
 
 /- make reducible? -/
-def indep_indep_of_circuits (C : circuits E) : finset (finset α) :=
-(powerset E).filter (λ S, ∀ c ∈ C.circuits, ¬c ⊆ S)
+def indep_indep (C : of_circuits E) : finset (finset E) :=
+(powerset univ).filter (λ S, ∀ c ∈ C.circuits, ¬c ⊆ S)
 
 /-- first part of Theorem 1.1.4 -/
-lemma I2_of_circuits (C : circuits E) (x y : finset α) : x ∈ indep_indep_of_circuits C → y ⊆ x →
-  y ∈ indep_indep_of_circuits C :=
+lemma I2 (C : of_circuits E) (x y : finset E) : x ∈ C.indep_indep → y ⊆ x →
+  y ∈ C.indep_indep :=
 begin
-  simp only [indep_indep_of_circuits, mem_powerset, and_imp, mem_filter],
-  exact λ hxE hx hxy, ⟨subset.trans hxy hxE, λ c hc H, hx c hc $ subset.trans H hxy⟩
+  simp only [indep_indep, mem_powerset, and_imp, mem_filter],
+  exact λ hxE hx hxy, ⟨subset.trans hxy hxE, λ c hc H, hx c hc $ subset.trans H hxy⟩,
 end
 
 /-- second part of Theorem 1.1.4 -/
-lemma I3_of_circuits (C : circuits E) (x y : finset α) (hx : x ∈ indep_indep_of_circuits C)
-  (hy : y ∈ indep_indep_of_circuits C) (hcardxy : card x < card y)
-  : ∃ e, e ∈ y \ x ∧ insert e x ∈ indep_indep_of_circuits C :=
+lemma I3 (C : of_circuits E) (x y : finset E) (hx : x ∈ C.indep_indep)
+  (hy : y ∈ C.indep_indep) (hcardxy : card x < card y)
+  : ∃ e, e ∈ y \ x ∧ insert e x ∈ C.indep_indep :=
 begin
-  unfold indep_indep_of_circuits at ⊢,
-  simp only [indep_indep_of_circuits, mem_powerset, mem_filter] at hx hy,
+  unfold indep_indep at ⊢,
+  simp only [indep_indep, mem_powerset, mem_filter] at hx hy,
   by_contra h,
   simp only [mem_powerset, not_exists, and_imp, mem_filter, not_and, mem_sdiff] at h,
   let F := (powerset $ x ∪ y).filter (λ S, (∀ c ∈ C.circuits, ¬c ⊆ S) ∧ card x < card S),
   have hyF : y ∈ F := mem_filter.mpr ⟨mem_powerset.mpr $ subset_union_right x y,
     ⟨hy.2, hcardxy⟩⟩,
-  exact exists.elim (min_fun_of_ne_empty (λ f, card (x \ f)) $ ne_empty_of_mem hyF)
-    (λ z Hz, exists.elim Hz $ by { clear hcardxy Hz hyF,
-      intros hz hminz,
-      have hzxuy : z ⊆ x ∪ y := mem_powerset.mp (mem_filter.mp hz).1,
-      replace hz := (mem_filter.mp hz).2,
-      exact exists.elim (exists_sdiff_of_card_lt hz.2)
-        (by { intros a ha, rw mem_sdiff at ha,
-        have hxsdiffz : x \ z ≠ ∅ :=
-          by { intro H,
-          have Hxsubz : x ⊆ z := subset_iff_sdiff_eq_empty.mpr H,
-          have hay : a ∈ y := or.elim (mem_union.mp $ mem_of_subset hzxuy ha.1)
-            (λ Hax, false.elim $ ha.2 Hax) id,
-          have haindep : insert a x ∈ indep_indep_of_circuits C := I2_of_circuits C z (insert a x)
-            (by { simp only [indep_indep_of_circuits, mem_powerset, mem_filter],
-            exact ⟨subset.trans hzxuy $ union_subset hx.1 hy.1, hz.1⟩ })
-            (insert_subset.mpr ⟨ha.1, Hxsubz⟩),
-          simp only [indep_indep_of_circuits, mem_powerset, mem_filter] at haindep,
-          exact h a hay ha.2 haindep.1 haindep.2 },
-        exact exists.elim (exists_mem_of_ne_empty hxsdiffz)
-          (by { clear h ha hxsdiffz,
-          intros e he, rw mem_sdiff at he,
-          let T : α → finset α := λ f, erase (insert e z) f,
-          have hTf1 : ∀ f, f ∈ z \ x → T f ⊆ x ∪ y :=
-            by { intros f hf, rw [mem_sdiff] at hf,
-            rw [subset_iff],
-            intros gg hgg, simp only [mem_insert, mem_erase, ne.def] at hgg,
-            simp only [mem_union],
-            exact or.elim hgg.2 (λ gge, or.inl $ gge.symm ▸ he.1)
-              (λ ggz, mem_union.mp $ mem_of_subset hzxuy ggz) },
-          have hTf2 : ∀ f, f ∈ z \ x → card (x \ T f) < card (x \ z) :=
-            by { intros f hf, rw mem_sdiff at hf,
-            suffices H : x \ T f ⊂ x \ z, exact card_lt_card H,
-            by { simp only [ssubset_iff, exists_prop, mem_insert, not_forall_not, not_and,
-                            mem_sdiff, mem_erase],
-              exact exists.intro e
-                ⟨λ h_, ⟨λ hef, hf.2 $ hef ▸ he.1, or.inl rfl⟩,
-                by { rw [subset_iff],
-                  intros gg hgg,
-                  simp only [mem_insert, not_and, mem_sdiff, mem_erase, ne.def] at hgg,
-                  have ggnef : gg ≠ f := λ ggef, or.elim hgg
-                    (λ gge, (gge.symm ▸ he.2) $ ggef.substr hf.1) (λ H, (ggef.substr hf.2) H.1),
-                  have he0 := mem_sdiff.mpr he,
-                  exact or.elim hgg (λ gge, gge.symm ▸ he0)
-                  (λ H, mem_sdiff.mpr ⟨H.1, λ ggz, (H.2 ggnef) $ or.inr ggz⟩) }⟩ } },
-          have hTfindep : ∀ f, f ∈ z \ x → T f ∉ indep_indep_of_circuits C :=
-            by { intros f hf,
-            simp only [indep_indep_of_circuits, mem_powerset, mem_filter, not_and],
-            intros hTfE H,
-            have HTf1 : T f ⊆ x ∪ y := hTf1 f hf,
-            have HTf2 : card (x \ T f) < card (x \ z) := hTf2 f hf,
-            rw mem_sdiff at hf,
-            have HTfcard : card z = card (T f) :=
-              by { simp only [card_erase_of_mem (mem_insert.mpr $ or.inr hf.1),
-              card_insert_of_not_mem he.2, mem_insert, card_insert_of_not_mem, nat.pred_succ] },
-            replace HTfcard : card x < card (T f) := HTfcard ▸ hz.2,
-            have : T f ∈ F := mem_filter.mpr ⟨mem_powerset.mpr HTf1, ⟨H, HTfcard⟩⟩,
-            exact not_lt.mpr (hminz (T f) this) HTf2 },
-          have hTfC : ∀ f, f ∈ z \ x → ∃ c ∈ C.circuits, c ⊆ T f :=
-            by { intros f hf,
-            have : T f ∉ indep_indep_of_circuits C := hTfindep f hf,
-              simp only [indep_indep_of_circuits, mem_powerset, mem_filter, not_and] at this,
-            have hfc := this (subset.trans (hTf1 f hf) $ union_subset hx.1 hy.1),
-            by_contra H, simp only [not_exists, exists_prop, not_and] at H, contradiction },
-          exact exists.elim (exists_sdiff_of_card_lt hz.2) (λ g hg, exists.elim (hTfC g hg) $
-              λ Cg hCg, exists.elim hCg $
-                by { clear hCg hTf1 hTf2 hTfindep hg,
-                intros HCg1 HCg2,
-                have hCgsub : Cg ⊆ insert e z := subset.trans HCg2 (erase_subset g $ insert e z),
-                rw [subset_iff] at HCg2,
-                have HCgzx : Cg ∩ (z \ x) ≠ ∅ :=
-                  λ H, suffices Cg ⊆ x, from hx.2 Cg HCg1 this,
-                    suffices H1 : Cg ⊆ erase (insert e (x ∩ z)) g, from
-                    suffices H2 : erase (insert e (x ∩ z)) g ⊆ x, from
-                    subset.trans H1 H2,
-                    show erase (insert e (x ∩ z)) g ⊆ x, by
-                      { rw [subset_iff],
-                      intros gg hgg,
-                      simp only [mem_insert, mem_erase, mem_inter] at hgg,
-                      exact or.elim hgg.2 (λ gge, gge.symm ▸ he.1) (λ ggxggz, ggxggz.1) },
-                    show Cg ⊆ erase (insert e (x ∩ z)) g, by
-                      { rw [subset_iff],
-                      intros gg hgg,
-                      replace HCg2 : gg ∈ T g := HCg2 hgg,
-                      simp only [mem_insert, mem_erase, mem_inter] at HCg2 ⊢,
-                      split,
-                        { exact HCg2.1 },
-                        { rw eq_empty_iff_forall_not_mem at H,
-                        replace H : gg ∉ Cg ∩ (z \ x) := H gg,
-                        simp only [not_and, mem_sdiff, not_not, mem_inter] at H,
-                      exact or.elim HCg2.2 (λ gge, or.inl gge) (λ ggz, or.inr ⟨H hgg ggz, ggz⟩) } },
-                clear HCg2,
-                exact exists.elim (exists_mem_of_ne_empty HCgzx)
-                  (by { intros h0 hh0, rw [mem_inter] at hh0,
-                  exact exists.elim (hTfC h0 hh0.2)
-                    (λ Ch0 HCh0, exists.elim HCh0 $ λ hCh0circ hCh0T,
-                      have hCgneCh0 : Cg ≠ Ch0 :=
-                        λ H, have hh0Ch0 : h0 ∉ Ch0 := λ HH, (mem_erase.mp $
-                          mem_of_subset hCh0T HH).1 rfl, (H.symm ▸ hh0Ch0) hh0.1,
-                      have hCh0sub : Ch0 ⊆ insert e z :=
-                        subset.trans hCh0T (erase_subset h0 $ insert e z),
-                      have heCgCh0 : e ∈ Cg ∩ Ch0 :=
-                        by { rw mem_inter, split,
-                          { by_contra heCg, have hCgz : Cg ⊆ z :=
-                              (erase_eq_of_not_mem heCg) ▸ (subset_insert_iff.mp hCgsub),
-                            exact hz.1 Cg HCg1 hCgz },
-                          { by_contra heCh0, have hCh0z : Ch0 ⊆ z :=
-                              (erase_eq_of_not_mem heCh0) ▸ (subset_insert_iff.1 hCh0sub),
-                            exact hz.1 Ch0 hCh0circ hCh0z } },
-                      exists.elim (C.circuit_elim HCg1 hCh0circ hCgneCh0 heCgCh0) $
-                        λ CC ⟨hCCcirc, hCCCguCh0⟩,
-                          have hCCz : CC ⊆ z :=
-                            by { rw [subset_iff],
-                            intros t ht,
-                            rw [subset_iff] at hCCCguCh0,
-                            have htCguCh0 := hCCCguCh0 ht,
-                              simp only [mem_union, mem_erase] at htCguCh0,
-                            rw [subset_iff] at hCgsub hCh0sub,
-                            have orCg : t ∈ Cg → t ∈ z :=
-                              λ htCg, or.elim (mem_insert.mp $ hCgsub htCg)
-                                (λ H, false.elim $ htCguCh0.1 H) id,
-                            have orCh0 : t ∈ Ch0 → t ∈ z :=
-                              λ htCh0, or.elim (mem_insert.mp $ hCh0sub htCh0)
-                              (λ H, false.elim $ htCguCh0.1 H) id,
-                            exact or.elim htCguCh0.2 orCg orCh0 },
-                          hz.1 CC hCCcirc hCCz) }) }) }) }) })
+  rcases (min_fun_of_ne_empty (λ f, card (x \ f)) $ ne_empty_of_mem hyF) with ⟨z, ⟨hz, hminz⟩⟩,
+  clear hcardxy hyF,
+  have hzxuy : z ⊆ x ∪ y := mem_powerset.mp (mem_filter.mp hz).1,
+  replace hz := (mem_filter.mp hz).2,
+  rcases (exists_sdiff_of_card_lt hz.2) with ⟨a, ha⟩,
+  rw mem_sdiff at ha,
+  have hxsdiffz : x \ z ≠ ∅ :=
+    by { intro H,
+    have Hxsubz : x ⊆ z := subset_iff_sdiff_eq_empty.mpr H,
+    have hay : a ∈ y := or.elim (mem_union.mp $ mem_of_subset hzxuy ha.1)
+      (λ Hax, false.elim $ ha.2 Hax) id,
+    have haindep : insert a x ∈ C.indep_indep := C.I2 z (insert a x)
+      (by { simp only [indep_indep, mem_powerset, mem_filter],
+      exact ⟨subset.trans hzxuy $ union_subset hx.1 hy.1, hz.1⟩, })
+      (insert_subset.mpr ⟨ha.1, Hxsubz⟩),
+    simp only [indep_indep, mem_powerset, mem_filter] at haindep,
+    exact h a hay ha.2 haindep.1 haindep.2, },
+  rcases (exists_mem_of_ne_empty hxsdiffz) with ⟨e, he⟩,
+  clear h ha hxsdiffz,
+  rw mem_sdiff at he,
+  let T : E → finset E := λ f, erase (insert e z) f,
+  have hTf1 : ∀ f, f ∈ z \ x → T f ⊆ x ∪ y :=
+    by { intros f hf, rw [mem_sdiff] at hf,
+    rw [subset_iff],
+    intros gg hgg, simp only [mem_insert, mem_erase, ne.def] at hgg,
+    simp only [mem_union],
+    rcases hgg.2 with rfl | hggz,
+    { exact or.inl he.1, },
+    exact (mem_union.mp $ mem_of_subset hzxuy hggz) },
+  have hTf2 : ∀ f, f ∈ z \ x → card (x \ T f) < card (x \ z) :=
+    by { intros f hf, rw mem_sdiff at hf,
+    suffices H : x \ T f ⊂ x \ z, exact card_lt_card H,
+    by { simp only [ssubset_iff, exists_prop, mem_insert, not_forall_not, not_and,
+                    mem_sdiff, mem_erase],
+      use e, split,
+      { intro _, split,
+        { intro hef, exact hf.2 (hef ▸ he.1), },
+        { exact or.inl rfl, } },
+      { rw [subset_iff],
+        intros gg hgg,
+        simp only [mem_insert, not_and, mem_sdiff, mem_erase, ne.def] at hgg,
+        have ggnef : gg ≠ f := by { intro ggef,
+          rcases hgg with gge | H,
+          { exact ((gge.symm ▸ he.2) $ ggef.substr hf.1), },
+          { exact (ggef.substr hf.2) H.1, } },
+        have he0 : e ∈ x \ z := mem_sdiff.mpr he,
+        rcases hgg with gge | H,
+        { exact gge.symm ▸ he0, },
+        { exact mem_sdiff.mpr ⟨H.1, λ ggz, (H.2 ggnef) $ or.inr ggz⟩, } } } },
+  have hTfindep : ∀ f, f ∈ z \ x → T f ∉ C.indep_indep :=
+    by { intros f hf,
+    simp only [indep_indep, mem_powerset, mem_filter, not_and],
+    intros hTfE H,
+    have HTf1 : T f ⊆ x ∪ y := hTf1 f hf,
+    have HTf2 : card (x \ T f) < card (x \ z) := hTf2 f hf,
+    rw mem_sdiff at hf,
+    have HTfcard : card z = card (T f) :=
+      by { simp only [card_erase_of_mem (mem_insert.mpr $ or.inr hf.1),
+      card_insert_of_not_mem he.2, mem_insert, card_insert_of_not_mem, nat.pred_succ], },
+    replace HTfcard : card x < card (T f) := HTfcard ▸ hz.2,
+    have : T f ∈ F := mem_filter.mpr ⟨mem_powerset.mpr HTf1, ⟨H, HTfcard⟩⟩,
+    exact not_lt.mpr (hminz (T f) this) HTf2, },
+  have hTfC : ∀ f, f ∈ z \ x → ∃ c ∈ C.circuits, c ⊆ T f :=
+    by { intros f hf,
+    have : T f ∉ C.indep_indep := hTfindep f hf,
+      simp only [indep_indep, mem_powerset, mem_filter, not_and] at this,
+    have hfc := this (subset.trans (hTf1 f hf) $ union_subset hx.1 hy.1),
+    by_contra H, simp only [not_exists, exists_prop, not_and] at H, contradiction, },
+  rcases (exists_sdiff_of_card_lt hz.2) with ⟨g, hg⟩,
+  rcases (hTfC g hg) with ⟨Cg, ⟨HCg1, HCg2⟩⟩,
+  clear hTf1 hTf2 hTfindep hg hy hminz hzxuy,
+  have hCgsub : Cg ⊆ insert e z := subset.trans HCg2 (erase_subset g $ insert e z),
+  rw [subset_iff] at HCg2,
+  have HCgzx : Cg ∩ (z \ x) ≠ ∅ := by { intro H,
+    suffices : Cg ⊆ x, from hx.2 Cg HCg1 this,
+    suffices H1 : Cg ⊆ erase (insert e (x ∩ z)) g, from
+    suffices H2 : erase (insert e (x ∩ z)) g ⊆ x, from
+    subset.trans H1 H2,
+    show erase (insert e (x ∩ z)) g ⊆ x, by { rw [subset_iff],
+      intros gg hgg,
+      simp only [mem_insert, mem_erase, mem_inter] at hgg,
+      rcases hgg.2 with gge | ggxggz,
+      { exact gge.symm ▸ he.1, },
+      { exact ggxggz.1, } },
+    show Cg ⊆ erase (insert e (x ∩ z)) g, by
+      { rw [subset_iff],
+      intros gg hgg,
+      replace HCg2 : gg ∈ T g := HCg2 hgg,
+      simp only [mem_insert, mem_erase, mem_inter] at HCg2 ⊢,
+      split,
+      { exact HCg2.1, },
+      { rw eq_empty_iff_forall_not_mem at H,
+        replace H : gg ∉ Cg ∩ (z \ x) := H gg,
+        simp only [not_and, mem_sdiff, not_not, mem_inter] at H,
+        rcases HCg2.2 with gge | ggz,
+        { exact or.inl gge, },
+        { exact or.inr ⟨H hgg ggz, ggz⟩, } } } },
+  clear HCg2 he hx,
+  rcases (exists_mem_of_ne_empty HCgzx) with ⟨h0, hh0⟩, clear HCgzx,
+  rw [mem_inter] at hh0,
+  rcases (hTfC h0 hh0.2) with ⟨Ch0, ⟨hCh0circ, hCh0T⟩⟩, clear hTfC,
+  have hCgneCh0 : Cg ≠ Ch0 :=
+    λ H, have hh0Ch0 : h0 ∉ Ch0 := λ HH, (mem_erase.mp $
+      mem_of_subset hCh0T HH).1 rfl, (H.symm ▸ hh0Ch0) hh0.1,
+  have hCh0sub : Ch0 ⊆ insert e z :=
+    subset.trans hCh0T (erase_subset h0 $ insert e z),
+  have heCgCh0 : e ∈ Cg ∩ Ch0 :=
+    by { rw mem_inter, split,
+      { by_contra heCg, have hCgz : Cg ⊆ z :=
+          (erase_eq_of_not_mem heCg) ▸ (subset_insert_iff.mp hCgsub),
+        exact hz.1 Cg HCg1 hCgz },
+      { by_contra heCh0, have hCh0z : Ch0 ⊆ z :=
+          (erase_eq_of_not_mem heCh0) ▸ (subset_insert_iff.1 hCh0sub),
+        exact hz.1 Ch0 hCh0circ hCh0z } },
+  rcases (C.circuit_elim HCg1 hCh0circ hCgneCh0 heCgCh0) with ⟨CC, ⟨hCCcirc, hCCCguCh0⟩⟩,
+  clear HCg1 hCh0circ hCgneCh0 heCgCh0,
+  have hCCz : CC ⊆ z :=
+    by { rw [subset_iff],
+    intros t ht,
+    rw [subset_iff] at hCCCguCh0,
+    have htCguCh0 := hCCCguCh0 ht,
+      simp only [mem_union, mem_erase] at htCguCh0,
+    rw [subset_iff] at hCgsub hCh0sub,
+    rcases htCguCh0.2 with htCg | htCh0,
+    { rcases (mem_insert.mp $ hCgsub htCg) with Hte | Htz,
+      { exfalso, exact htCguCh0.1 Hte, },
+      { exact Htz, } },
+    { rcases (mem_insert.mp $ hCh0sub htCh0) with Hte | Htz,
+      { exfalso, exact htCguCh0.1 Hte },
+      { exact Htz, } } },
+  exact hz.1 CC hCCcirc hCCz,
 end
 
-def indep_of_circuits (C : circuits E) : indep E :=
-⟨indep_indep_of_circuits C,
-by simp only [indep_indep_of_circuits, filter_subset],
-mem_filter.mpr
-  ⟨empty_mem_powerset E, λ c hc H, C.empty_not_mem_circuits $ (subset_empty.mp H) ▸ hc⟩,
-I2_of_circuits C,
-I3_of_circuits C⟩
+def indep (C : of_circuits E) : of_indep E :=
+{ indep := C.indep_indep,
+  empty_mem_indep := mem_filter.mpr
+    ⟨empty_mem_powerset univ, λ c hc H, C.empty_not_mem_circuits $ (subset_empty.mp H) ▸ hc⟩,
+  indep_of_subset_indep := C.I2,
+  indep_exch := C.I3 }
 
-instance circ_indep : has_coe (circuits E) (indep E) := ⟨indep_of_circuits⟩
-instance indep_circ : has_coe (indep E) (circuits E) := ⟨circuits_of_indep⟩
+/- Not sure if these instances are a good idea... -/
+-- instance circ_indep : has_coe (circuits E) (indep E) := ⟨indep_of_circuits⟩
+-- instance indep_circ : has_coe (indep E) (circuits E) := ⟨circuits_of_indep⟩
 
 /-- third part of Theorem 1.1.4 -/
-theorem circ_indep_circ : ∀ C : circuits E, C = circuits_of_indep (indep_of_circuits C)
-  | ⟨c₁, p₁, q₁, r₁, s₁⟩ :=
-by { simp only [indep_of_circuits, circuits_of_indep, indep_indep_of_circuits,
-  circuits_circ_of_indep, is_circuit, ext, mem_filter, mem_powerset, and_imp, not_and],
-exact λ c, iff.intro
-  (λ hc : c ∈ c₁, have ce : c ⊆ E := mem_powerset.mp (mem_of_subset p₁ hc),
-  ⟨ce, ⟨λ _ H, (H c hc) $ subset.refl c, λ f hf,
-    ⟨subset.trans (le_of_lt $ lt_iff_ssubset.mpr hf) ce,
-    λ g hg H, have Hc : g < c := lt_of_le_of_lt (le_iff_subset.mpr H) $ lt_iff_ssubset.mpr hf,
-      have r : g = c := r₁ hg hc $ le_of_lt Hc, (not_le_of_lt Hc) $ le_of_eq r.symm⟩⟩⟩) $
-  λ hc, have ∃ c_1 ∈ c₁, c_1 ⊆ c := by { have := not_forall.mp (hc.2.1 hc.1),
-    simpa only [exists_prop, not_forall_not] },
-  exists.elim this $ λ c' H, exists.elim H $ by { intros hc' hcc',
-    by_cases h : c = c', { exact h.symm ▸ hc' },
-      { have hc'lt : c' ⊂ c := lt_of_le_of_ne (le_iff_subset.mpr hcc') (ne.symm h),
-        have : c' ∉ c₁ := mt ((hc.2.2 c' hc'lt).2 c') (not_not.mpr $ subset.refl c'),
-        exact false.elim (this hc') } } }
-
-theorem indep_circ_indep (M : indep E) : M = indep_of_circuits (circuits_of_indep M) :=
-suffices M.indep = (indep_of_circuits $ circuits_of_indep M).indep, from eq_of_indep_eq this,
+theorem circ_indep_circ : ∀ C : of_circuits E, C = C.indep.circuits
+  | ⟨c₁, p₁, q₁, r₁⟩ :=
 begin
-  simp only [circuits_of_indep, indep_of_circuits, circuits_circ_of_indep, indep_indep_of_circuits,
+  simp only [of_circuits.indep, of_indep.circuits, indep_indep,
+  circuits_circuits, is_circuit, ext, mem_filter, mem_powerset, and_imp, not_and],
+  intro c,
+  split,
+  { intro hc,
+    have ce : c ⊆ univ := subset_univ c,
+    simp only [ce, true_and, forall_prop_of_true, not_forall, not_not],
+    split,
+    { use [c, hc], refl },
+    { intros f hf, split,
+      { exact subset.trans (le_of_lt $ lt_iff_ssubset.mpr hf) ce, },
+      { intros g hg H,
+        have Hc : g < c := lt_of_le_of_lt (le_iff_subset.mpr H) (lt_iff_ssubset.mpr hf),
+        have r : g = c := q₁ hg hc (le_of_lt Hc),
+        exact (not_le_of_lt Hc) (le_of_eq r.symm), } } },
+  { rintro ⟨hc, ⟨Hc1, Hc2⟩⟩,
+    have : ∃ c' ∈ c₁, c' ⊆ c := by { have := not_forall.mp (Hc1 hc),
+    simpa only [exists_prop, not_forall_not] },
+    rcases this with ⟨c', ⟨hc', hcc'⟩⟩,
+    by_cases h : c = c',
+    { exact h.symm ▸ hc' },
+    { have hc'lt : c' ⊂ c := lt_of_le_of_ne (le_iff_subset.mpr hcc') (ne.symm h),
+      have : c' ∉ c₁ := mt ((Hc2 c' hc'lt).2 c') (not_not.mpr $ subset.refl c'),
+      exact (this hc').elim, } },
+end
+
+end of_circuits
+
+namespace of_indep
+open of_circuits
+variable {E}
+
+theorem indep_circ_indep (M : of_indep E) : M = M.circuits.indep :=
+suffices M.indep = M.circuits.indep.indep, from eq_of_indep_eq this,
+begin
+  simp only [of_indep.circuits, of_circuits.indep, circuits_circuits, indep_indep,
     ext, mem_powerset, and_imp, mem_filter],
   intro I,
-  have hI : I ∈ M.indep → I ⊆ E := λ H, mem_powerset.mp $
-    mem_of_subset (M.indep_subset_powerset_ground) H,
+  have hI : I ∈ M.indep → I ⊆ univ := λ H, subset_univ I,
   rw [←and_iff_right_of_imp hI, and_congr_right],
-  intro hIE, have := not_iff_not_of_iff (dep_iff_circuit_subset M hIE),
+  intro hIE, have := not_iff_not_of_iff (dep_iff_circuit_subset I M),
   simp only [not_exists, exists_prop, not_and, not_not] at this,
   rw [this, forall_congr],
-  exact λ a, ⟨λ h h₁ h₂ h₃, (h h₃) h₂, λ h h₁ h₂, h (subset.trans h₁ hIE) h₂ h₁⟩
+  exact λ a, ⟨λ h h₁ h₂ h₃, (h h₃) h₂, λ h h₁ h₂, h (subset.trans h₁ hIE) h₂ h₁⟩,
 end
 
 /-- Proposition 1.1.6 -/
-theorem existsu_circuit_of_dep_of_insert_indep {I : finset α} {e : α} {m : indep E}
-  (hI : I ∈ m.indep) (he : e ∈ E) (hIe : insert e I ∉ m.indep) :
-  ∃ c, c ∈ circuits_circ_of_indep m ∧ c ⊆ insert e I ∧ e ∈ c ∧
-  ∀ c' ∈ circuits_circ_of_indep m, c' ⊆ insert e I ∧ e ∈ c → c' = c :=
-by { simp only [circuits_circ_of_indep, mem_powerset, and_imp, mem_filter],
-exact have hIE : I ⊆ E, from mem_powerset.mp (mem_of_subset m.indep_subset_powerset_ground hI),
-have hIeE : insert e I ⊆ E, from insert_subset.mpr ⟨he, hIE⟩,
-have hc : _, from (dep_iff_circuit_subset m hIeE).mp hIe,
-exists.elim hc $ λ c hEc, exists.elim hEc $ λ hceI hccirc,
-  have hcE : c ⊆ E := subset.trans hceI hIeE,
+theorem existsu_circuit_of_dep_of_insert {I : finset E} {e : E} {m : of_indep E}
+  (hI : I ∈ m.indep) (hIe : insert e I ∉ m.indep) :
+  ∃ c, c ∈ m.circuits_circuits ∧ c ⊆ insert e I ∧ e ∈ c ∧
+  ∀ c', c' ∈ m.circuits_circuits → c' ⊆ insert e I → c' = c :=
+begin
+  simp only [circuits_circuits, mem_powerset, and_imp, mem_filter],
+  have hIE : I ⊆ univ, from subset_univ I,
+  have hc : ∃ (y : finset E) (H : y ⊆ insert e I), is_circuit y m,
+    from (dep_iff_circuit_subset (insert e I) m).mp hIe, clear hIe,
+  rcases hc with ⟨c, ⟨hceI, hccirc⟩⟩,
+  have hcE : c ⊆ univ := subset_univ c,
   have hecirc : ∀ c' ⊆ insert e I, is_circuit c' m → e ∈ c' :=
     by { intros c' hc'eI hc'circ,
-    have h₁ := subset_insert_iff.mp hc'eI,
-    by_contra h,
-    have h₂ := (erase_eq_of_not_mem h).symm,
-    have h₃ : c' ⊆ I := calc
-    c' = erase c' e : h₂
-    ... ⊆ I : h₁,
-    exact (dep_iff_circuit_subset m hIE).mpr (exists.intro c' $ exists.intro h₃ $ hc'circ) hI },
+      have h₁ := subset_insert_iff.mp hc'eI,
+      by_contra h,
+      have h₂ := (erase_eq_of_not_mem h).symm,
+      have h₃ : c' ⊆ I := calc
+      c' = erase c' e : h₂
+      ... ⊆ I : h₁,
+      refine (dep_iff_circuit_subset I m).mpr _ hI,
+      use [c', h₃], exact hc'circ, },
   have hec : e ∈ c := hecirc c hceI hccirc,
-  exists.intro c $ by { exact ⟨⟨hcE, hccirc⟩, ⟨hceI,⟨hec, by { intros c' hc'E hc'circ hc'eI _,
-    have hec' : e ∈ c' := hecirc c' hc'eI hc'circ,
-    have hcuc'eI : erase (c ∪ c') e ⊆ I := by {
-      simp only [subset_iff, and_imp, mem_union, mem_insert, mem_erase, ne.def] at hceI hc'eI ⊢,
-      exact λ a hane ha, or.elim ha (λ H, or.elim (hceI H) (λ H, false.elim $ hane H) id)
-        (λ H, or.elim (hc'eI H) (λ H, false.elim $ hane H) id) },
-    have : erase (c ∪ c') e ∈ m.indep := m.indep_of_subset_indep hI hcuc'eI,
-    by_contra h,
-    have C3 := C3_of_indep m c c' e,
-      simp only [circuits_circ_of_indep, mem_powerset, and_imp,
-        filter_congr_decidable, mem_filter, mem_inter] at C3,
-    exact exists.elim (C3 hcE hccirc hc'E hc'circ (ne.symm h) hec hec')
-      (λ c₀ hc₀, (dep_iff_circuit_subset m hIE).mpr (exists.intro c₀ $ exists.intro
-        (subset.trans hc₀.2 hcuc'eI) hc₀.1.2) hI) }⟩⟩⟩ } }
+  use c,
+  split, { exact ⟨hcE, hccirc⟩, }, { split, { exact hceI, }, { split, { exact hec, },
+  { intros c' hc'E hc'circ hc'eI,
+  have hec' : e ∈ c' := hecirc c' hc'eI hc'circ,
+  have hcuc'eI : erase (c ∪ c') e ⊆ I :=
+    by { simp only [subset_iff, and_imp, mem_union, mem_insert, mem_erase, ne.def]
+      at hceI hc'eI ⊢,
+      rintros a hane (H | H),
+      { rcases (hceI H) with H' | H', { exact (hane H').elim, }, { exact H', } },
+      { rcases (hc'eI H) with H' | H', { exact (hane H').elim ,}, { exact H', } } },
+  have : erase (c ∪ c') e ∈ m.indep := m.indep_of_subset_indep hI hcuc'eI,
+  by_contra h,
+  have C3 := m.C3 c c' e,
+    simp only [circuits_circuits, mem_powerset, and_imp,
+      filter_congr_decidable, mem_filter, mem_inter] at C3,
+  rcases (C3 hcE hccirc hc'E hc'circ (ne.symm h) hec hec') with ⟨c₀, ⟨⟨hc₀, hc₀circ⟩, hc₀erase⟩⟩,
+  refine (dep_iff_circuit_subset I m).mpr _ hI,
+  use [c₀, subset.trans hc₀erase hcuc'eI], exact hc₀circ, } } },
+end
 
 section encodable
-variable [encodable α]
+variable [encodable E]
 
-def circuit_of_dep_of_insert_indep {I : finset α} {e : α} {m : indep E}
-  (hI : I ∈ m.indep) (he : e ∈ E) (hIe : insert e I ∉ m.indep) : finset α :=
-encodable.choose (existsu_circuit_of_dep_of_insert_indep hI he hIe)
+def circuit_of_dep_of_insert_indep {I : finset E} {e : E} {m : of_indep E}
+  (hI : I ∈ m.indep) (hIe : insert e I ∉ m.indep) : finset E :=
+encodable.choose (existsu_circuit_of_dep_of_insert hI hIe)
 
 local notation `cdii` := circuit_of_dep_of_insert_indep
 
-def circuit_of_dep_of_insert_indep_spec {I : finset α} {e : α} {m : indep E}
-  (hI : I ∈ m.indep) (he : e ∈ E) (hIe : insert e I ∉ m.indep) :
-  cdii hI he hIe ∈ circuits_circ_of_indep m ∧ cdii hI he hIe ⊆ insert e I ∧
-  e ∈ cdii hI he hIe ∧ ∀ (c' : finset α), c' ∈ circuits_circ_of_indep m →
-  c' ⊆ insert e I ∧ e ∈ cdii hI he hIe → c' = cdii hI he hIe  :=
-encodable.choose_spec (existsu_circuit_of_dep_of_insert_indep hI he hIe)
+lemma circuit_of_dep_of_insert_indep_spec {I : finset E} {e : E} {m : of_indep E}
+  (hI : I ∈ m.indep) (hIe : insert e I ∉ m.indep) :
+  cdii hI hIe ∈ m.circuits_circuits ∧ cdii hI hIe ⊆ insert e I ∧
+  e ∈ cdii hI hIe ∧ ∀ c', c' ∈ m.circuits_circuits →
+  c' ⊆ insert e I → c' = cdii hI hIe :=
+encodable.choose_spec (existsu_circuit_of_dep_of_insert hI hIe)
 
 end encodable
 
+end of_indep
+
 -- § 1.2
 
-def is_basis (x : finset α) (m : indep E) : Prop :=
-x ∈ m.indep ∧ (∀ y ⊆ E, x ⊂ y → y ∉ m.indep)
+namespace of_indep
+variable {E}
 
-instance decidable_basis (x : finset α) (m : indep E) : decidable (is_basis x m) :=
-decidable_of_iff (x ∈ m.indep ∧ (∀ y ∈ powerset E, x ⊂ y → y ∉ m.indep)) $
+def is_basis (x : finset E) (m : of_indep E) : Prop :=
+x ∈ m.indep ∧ (∀ y, x ⊂ y → y ∉ m.indep)
+
+instance decidable_basis (x : finset E) (m : of_indep E) : decidable (is_basis x m) :=
+decidable_of_iff (x ∈ m.indep ∧ (∀ y, x ⊂ y → y ∉ m.indep)) $
   by simp only [is_basis, iff_self, finset.mem_powerset]
 
 /-- Lemma 1.2.1 -/
-theorem bases_of_indep_card_eq {x y : finset α} {m : indep E} : is_basis x m → is_basis y m →
+theorem bases_of_indep_card_eq {x y : finset E} {m : of_indep E} : is_basis x m → is_basis y m →
   card x = card y :=
 begin
   intros hx hy,
   by_contra heq,
   wlog h : card x < card y using [x y, y x],
-  exact lt_or_gt_of_ne heq,
+  { exact lt_or_gt_of_ne heq, },
   unfold is_basis at hx hy,
-  exact exists.elim (m.indep_exch hx.1 hy.1 h) (λ e ⟨he1, he2⟩,
-    have hins : insert e x ⊆ E := mem_powerset.mp
-      (mem_of_subset (m.indep_subset_powerset_ground) he2),
-    have hememx : e ∉ x := (mem_sdiff.mp he1).2,
-    (hx.2 (insert e x) hins $ ssubset_insert hememx) he2)
+  rcases (m.indep_exch hx.1 hy.1 h) with ⟨e, ⟨he1, he2⟩⟩,
+  have hememx : e ∉ x := (mem_sdiff.mp he1).2,
+  exact (hx.2 (insert e x) $ ssubset_insert hememx) he2,
 end
 
-theorem exists_basis_containing_indep {I : finset α} {m : indep E} (h : I ∈ m.indep) :
-  ∃ B : finset α, I ⊆ B ∧ is_basis B m :=
-let F := (m.indep).filter (λ a, I ⊆ a) in
-have FI : I ∈ F := mem_filter.mpr ⟨h, subset.refl I⟩,
-exists.elim (max_fun_of_ne_empty card $ ne_empty_of_mem FI) $
-  λ B HB, exists.elim HB $ by { clear HB, intros HBF Hg, rw mem_filter at HBF,
-    have hBB : is_basis B m := ⟨HBF.1, λ y hy hBy hyI,
-      have hxsy : I ⊆ y := le_of_lt $ lt_of_le_of_lt (le_iff_subset.mpr HBF.2) $
-        lt_iff_ssubset.mpr hBy,
-      have hyF : y ∈ F := mem_filter.mpr ⟨hyI, hxsy⟩,
-      lt_irrefl (card B) $ lt_of_lt_of_le (card_lt_card hBy) $ Hg y hyF⟩,
-    exact exists.intro B ⟨HBF.2, hBB⟩ }
+theorem exists_basis_containing_indep {I : finset E} {m : of_indep E} (h : I ∈ m.indep) :
+  ∃ B : finset E, I ⊆ B ∧ is_basis B m :=
+begin
+  let F := (m.indep).filter (λ a, I ⊆ a),
+  have FI : I ∈ F := mem_filter.mpr ⟨h, subset.refl I⟩,
+  rcases (max_fun_of_ne_empty card $ ne_empty_of_mem FI) with ⟨B, ⟨HBF, Hg⟩⟩,
+  rw mem_filter at HBF,
+  have hBB : is_basis B m := ⟨HBF.1, λ y hBy hyI,
+    have hxsy : I ⊆ y := le_of_lt $ lt_of_le_of_lt (le_iff_subset.mpr HBF.2) $
+      lt_iff_ssubset.mpr hBy,
+    have hyF : y ∈ F := mem_filter.mpr ⟨hyI, hxsy⟩,
+    lt_irrefl (card B) $ lt_of_lt_of_le (card_lt_card hBy) $ Hg y hyF⟩,
+  use B, exact ⟨HBF.2, hBB⟩,
+end
 
 section encodable
 
-def basis_containing_indep [encodable α] {I : finset α} {m : indep E} (h : I ∈ m.indep) :
-  finset α :=
+variable [encodable E]
+
+def basis_containing_indep {I : finset E} {m : of_indep E} (h : I ∈ m.indep) :
+  finset E :=
 encodable.choose $ exists_basis_containing_indep h
 
 local notation `bci` := basis_containing_indep
 
-def basis_containing_indep_spec [encodable α] {I : finset α} {m : indep E} (h : I ∈ m.indep) :
+lemma basis_containing_indep_spec {I : finset E} {m : of_indep E} (h : I ∈ m.indep) :
   I ⊆ bci h ∧ is_basis (bci h) m :=
 encodable.choose_spec $ exists_basis_containing_indep h
 
 end encodable
 
-theorem dep_of_card_gt_card_basis {x B : finset α} {m : indep E} (hB : is_basis B m)
+theorem dep_of_card_gt_card_basis {x B : finset E} {m : of_indep E} (hB : is_basis B m)
   (hcard : card B < card x) : x ∉ m.indep :=
-λ hxI, exists.elim (exists_basis_containing_indep hxI) $ λ B' hB',
-  ne_of_lt (lt_of_lt_of_le hcard $ card_le_of_subset hB'.1) $ bases_of_indep_card_eq hB hB'.2
+begin
+  intro hxI,
+  rcases (exists_basis_containing_indep hxI) with ⟨B', ⟨hxB', hB'basis⟩⟩,
+  refine ne_of_lt (lt_of_lt_of_le hcard $ card_le_of_subset hxB') _,
+  exact bases_of_indep_card_eq hB hB'basis,
+end
 
-theorem card_of_indep_le_card_basis {x B : finset α} {m : indep E} (hx : x ∈ m.indep)
+theorem card_of_indep_le_card_basis {x B : finset E} {m : of_indep E} (hx : x ∈ m.indep)
   (hB : is_basis B m) : card x ≤ card B :=
-by { by_contra h, exact dep_of_card_gt_card_basis hB (lt_of_not_ge h) hx }
+begin
+  by_contra h,
+  exact dep_of_card_gt_card_basis hB (lt_of_not_ge h) hx,
+end
 
-structure bases (E : finset α) :=
-(bases : finset (finset α))
-(bases_subset_powerset_ground : bases ⊆ powerset E)
+end of_indep
+
+variable (E)
+
+structure of_bases :=
+(bases : finset (finset E))
 -- (B1)
 (bases_not_empty : bases ≠ ∅)
 -- (B2)
@@ -583,67 +906,89 @@ structure bases (E : finset α) :=
     : ∃ a, a ∈ y \ x ∧ insert a (erase x e) ∈ bases)
 --attribute [class] bases
 
-instance bases_repr [has_repr α] (E : finset α) : has_repr (bases E) :=
+namespace of_bases
+
+instance bases_repr [has_repr E] : has_repr (of_bases E) :=
 ⟨λ b, has_repr.repr b.bases⟩
 
-theorem eq_of_base_eq : ∀ {B₁ B₂ : bases E}, B₁.1 = B₂.1 → B₁ = B₂
-  | ⟨b₁, p₁, q₁, r₁⟩ ⟨b₂, p₂, q₂, r₂⟩ h :=
+variable {E}
+
+theorem eq_of_base_eq : ∀ {B₁ B₂ : of_bases E}, B₁.1 = B₂.1 → B₁ = B₂
+  | ⟨b₁, p₁, q₁⟩ ⟨b₂, p₂, q₂⟩ h :=
 by simpa only []
 
-def bases_bases_of_indep (m : indep E) : finset (finset α) :=
-(powerset E).filter (λ S, is_basis S m)
+end of_bases
 
-lemma B1_of_indep (m : indep E) : bases_bases_of_indep m ≠ ∅ :=
-by { simp only [is_basis, bases_bases_of_indep, ext, ne.def, mem_filter, mem_powerset,
+namespace of_indep
+
+variable {E}
+
+def bases_bases (m : of_indep E) : finset (finset E) :=
+(powerset univ).filter (λ S, is_basis S m)
+
+lemma B1 (m : of_indep E) : m.bases_bases ≠ ∅ :=
+begin
+  simp only [is_basis, bases_bases, ext, ne.def, mem_filter, mem_powerset,
     not_mem_empty, not_and, iff_false],
-  exact λ h, exists.elim (max_fun_of_ne_empty card $ ne_empty_of_mem m.empty_mem_indep)
-  (λ a ha, exists.elim ha $ λ ha1 hg, (h a (mem_powerset.mp $
-    mem_of_subset m.indep_subset_powerset_ground ha1)
-  ha1) $ λ F _ Fcontainsa Findep, not_le_of_lt (card_lt_card Fcontainsa) $ hg F Findep) }
+  intro h,
+  rcases max_fun_of_ne_empty card (ne_empty_of_mem m.empty_mem_indep) with ⟨a, ⟨ha1, hg⟩⟩,
+  refine (h a (subset_univ a) ha1) _,
+  intros F Fcontainsa Findep,
+  refine not_le_of_lt (card_lt_card Fcontainsa) _,
+  exact hg F Findep,
+end
 
 /- Lemma 1.2.2 -/
-lemma B2_of_indep (m : indep E) : ∀ (x y : finset α) (e : α), x ∈ bases_bases_of_indep m →
-  y ∈ bases_bases_of_indep m → e ∈ x \ y →
-  ∃ a, a ∈ y \ x ∧ insert a (erase x e) ∈ bases_bases_of_indep m :=
-by { simp only [is_basis, bases_bases_of_indep, filter_and, mem_filter, mem_sdiff,
+lemma B2 (m : of_indep E) : ∀ (x y : finset E) (e : E), x ∈ m.bases_bases →
+  y ∈ m.bases_bases → e ∈ x \ y →
+  ∃ a, a ∈ y \ x ∧ insert a (erase x e) ∈ m.bases_bases :=
+begin
+  simp only [is_basis, bases_bases, filter_and, mem_filter, mem_sdiff,
   mem_powerset, and_imp],
-exact λ x y e hxE hxI hx hyE hyI hy hex hey,
-  have hxr : erase x e ∈ m.indep := m.indep_of_subset_indep hxI $ erase_subset e x,
+  intros x y e hxE hxI hx hyE hyI hy hex hey,
+  have hxr : erase x e ∈ m.indep := m.indep_of_subset_indep hxI (erase_subset e x),
   have hxB : is_basis x m := ⟨hxI, hx⟩, have hyB : is_basis y m := ⟨hyI, hy⟩,
   have hcard : card (erase x e) < card y := calc
     card (erase x e) < card x : card_lt_card $ erase_ssubset hex
     ... = card y : bases_of_indep_card_eq hxB hyB,
-  exists.elim (m.indep_exch hxr hyI hcard) $
-    by { clear hxr hyI hcard hyB, intros a ha,
-      have ha1 := mem_sdiff.mp ha.1,
-      have hae : a ≠ e := λ hae, hey $ hae ▸ ha1.1,
-      have hax : a ∉ x := by { simp only [not_and, mem_erase, ne.def] at ha1, exact ha1.2 hae },
-      have hcx : card x > 0 := card_pos.mpr (ne_empty_of_mem hex),
-      have hayycard : card (insert a $ erase x e) = card x := calc
-        card (insert a $ erase x e) = nat.pred (card x) + 1 : by rw [card_insert_of_not_mem ha1.2,
-            card_erase_of_mem hex]
-        ... = card x : nat.succ_pred_eq_of_pos hcx,
-      exact exists.intro a ⟨⟨ha1.1, hax⟩, mem_powerset.mp $
-        mem_of_subset m.indep_subset_powerset_ground ha.2, ha.2,
-        λ _ _ hayy, dep_of_card_gt_card_basis hxB $ hayycard ▸ (card_lt_card hayy)⟩ } }
+  rcases (m.indep_exch hxr hyI hcard) with ⟨a, ha⟩,
+  clear hxr hyI hcard hyB,
+  have ha1 := mem_sdiff.mp ha.1,
+  have hae : a ≠ e := λ hae, hey $ hae ▸ ha1.1,
+  have hax : a ∉ x := by { simp only [not_and, mem_erase, ne.def] at ha1, exact ha1.2 hae },
+  have hcx : card x > 0 := card_pos.mpr (ne_empty_of_mem hex),
+  have hayycard : card (insert a $ erase x e) = card x := calc
+    card (insert a $ erase x e) = nat.pred (card x) + 1 : by rw [card_insert_of_not_mem ha1.2,
+        card_erase_of_mem hex]
+    ... = card x : nat.succ_pred_eq_of_pos hcx,
+  use a, simp only [ha1.1, hax, true_and, not_false_iff, ha.2, subset_univ],
+  intros y' hayy,
+  refine dep_of_card_gt_card_basis hxB _,
+  exact hayycard ▸ (card_lt_card hayy),
+end
 
-def bases_of_indep (m : indep E) : bases E :=
-⟨bases_bases_of_indep m,
-filter_subset _,
-B1_of_indep m,
-B2_of_indep m⟩
+def bases (m : of_indep E) : of_bases E :=
+{ bases := bases_bases m,
+  bases_not_empty := m.B1,
+  basis_exch := m.B2 }
+
+end of_indep
+
+namespace of_bases
+open of_indep
+variable {E}
 
 /-- Lemma 1.2.4 -/
-theorem bases_card_eq {x y : finset α} {b : bases E} (hx : x ∈ b.bases) (hy : y ∈ b.bases) :
+theorem bases_card_eq {x y : finset E} {b : of_bases E} (hx : x ∈ b.bases) (hy : y ∈ b.bases) :
   card x = card y :=
 begin
   by_contra heq,
   wlog h : card y < card x using [x y, y x],
   exact lt_or_gt_of_ne (ne.symm heq), clear heq,
-  let F : finset (finset α × finset α) := (finset.product b.bases b.bases).filter
-    (λ e : finset α × finset α, card e.1 < card e.2),
+  let F : finset (finset E × finset E) := (finset.product b.bases b.bases).filter
+    (λ e : finset E × finset E, card e.1 < card e.2),
   have hyx : (y, x) ∈ F := mem_filter.mpr ⟨mem_product.mpr ⟨hy, hx⟩, h⟩, clear hy hx,
-  exact exists.elim (min_fun_of_ne_empty (λ f : finset α × finset α, card (f.2 \ f.1)) $
+  exact exists.elim (min_fun_of_ne_empty (λ f : finset E × finset E, card (f.2 \ f.1)) $
       ne_empty_of_mem hyx)
     (λ a ha, exists.elim ha $ by { clear hyx ha,
       intros haF Ha, replace haF := mem_filter.mp haF,
@@ -651,7 +996,7 @@ begin
       exact exists.elim (exists_sdiff_of_card_lt haF.2)
         (λ e he, exists.elim (b.basis_exch hab.2 hab.1 he) $ λ aa ⟨haa1, haa2⟩,
           by { rw mem_sdiff at haa1,
-          let a2 : finset α := insert aa (erase a.2 e),
+          let a2 : finset E := insert aa (erase a.2 e),
           have haani : aa ∉ erase a.2 e := λ h, haa1.2 (mem_erase.mp h).2,
           have hea2 : e ∈ a.2 := (mem_sdiff.mp he).1,
           have hpos : 0 < card a.2 := card_pos.mpr (ne_empty_of_mem hea2),
@@ -674,81 +1019,83 @@ begin
           exact not_le_of_lt hcard (Ha (a.1, a2) ha2F) }) })
 end
 
-def indep_indep_of_bases (b : bases E) : finset (finset α) :=
-(powerset E).filter (λ x, ∃ a ∈ b.bases, x ⊆ a)
+def indep_indep (b : of_bases E) : finset (finset E) :=
+(powerset univ).filter (λ x, ∃ a ∈ b.bases, x ⊆ a)
 
 /-- first part of Theorem 1.2.3 -/
-def indep_of_bases (b : bases E) : indep E :=
-⟨indep_indep_of_bases b,
-filter_subset _,
-mem_filter.mpr ⟨empty_mem_powerset E, exists.elim (exists_mem_of_ne_empty b.bases_not_empty) $
-    λ a ha, exists.intro a $ exists.intro ha $ empty_subset a⟩,
-begin
-  intros x y hx hxy, simp only [indep_indep_of_bases, mem_powerset, filter_congr_decidable,
-    exists_prop, mem_filter] at hx ⊢,
-  exact ⟨subset.trans hxy hx.1,
-    exists.elim hx.2 $ λ a ha, exists.intro a ⟨ha.1, subset.trans hxy ha.2⟩⟩
-end,
-begin
-  intros x y hx hy hcard, unfold indep_indep_of_bases at *,
-  let F := (b.bases).filter (λ S, S ⊆ y),
-  by_contra h, simp only [mem_powerset, not_exists, and_imp, filter_congr_decidable,
-    exists_prop, mem_filter, not_and, mem_sdiff] at hx hy h,
-  exact exists.elim hx.2 (λ b1 hb1, exists.elim hy.2 $ λ b2 hb2, exists.elim
-    (min_fun_of_ne_empty (λ f, card (f \ (y ∪ b1))) $ ne_empty_of_mem $ mem_filter.mpr hb2) $
-    λ B2 hEB2, exists.elim hEB2 $ by { clear hb2 b2 hEB2,
-      intros hB2filt hB2min, replace hB2filt : B2 ∈ b.bases ∧ y ⊆ B2 := mem_filter.mp hB2filt,
-      have hysdiff : y \ b1 = y \ x := by { simp only [ext, mem_sdiff],
-        exact λ gg, ⟨λ hgg, ⟨hgg.1, λ hggnx, hgg.2 $ mem_of_subset hb1.2 hggnx⟩,
-          λ hgg, ⟨hgg.1, λ ggb1, h gg hgg.1 hgg.2 (insert_subset.mpr
-          ⟨mem_of_subset hy.1 hgg.1, hx.1⟩) b1 hb1.1 $ insert_subset.mpr ⟨ggb1, hb1.2⟩⟩⟩ },
-      have hB2yub1: B2 \ (y ∪ b1) = ∅ := by { by_contra H,
-        exact exists.elim (exists_mem_of_ne_empty H) (by { clear H,
-          intros X hX, simp only [not_or_distrib, mem_union, mem_sdiff] at hX,
-          have hXB2b1 : X ∈ B2 \ b1 := by { rw mem_sdiff, exact ⟨hX.1, hX.2.2⟩ },
-          exact exists.elim (b.basis_exch hB2filt.1 hb1.1 hXB2b1)
-            (λ Y ⟨hYb1B2, hYbases⟩, by { rw mem_sdiff at hYb1B2 hXB2b1,
-              have hssubY : insert Y (erase B2 X) \ (y ∪ b1) ⊂  B2 \ (y ∪ b1) :=
-                by { rw [ssubset_iff],
-                exact exists.intro X (by {
-                  simp only [subset_iff, not_or_distrib, mem_union, mem_insert, not_and, mem_sdiff,
-                    not_not, mem_erase, not_true, or_false, ne.def, false_and, or_false,
-                    eq_self_iff_true],
-                  exact ⟨λ hXY, false.elim $ hYb1B2.2 (hXY ▸ hXB2b1.1),
-                  λ gg hgg, or.elim hgg (λ ggx, ggx.symm ▸ hX) $ λ ggor2, or.elim ggor2.1
-                    (λ ggY, false.elim $ (ggY ▸ ggor2.2.2) hYb1B2.1) $
-                      λ ggXB2, ⟨ggXB2.2, ggor2.2⟩⟩ }) },
-              replace hssubY := card_lt_card hssubY,
-              have hysubY : y ⊆ insert Y (erase B2 X) := by {
-                simp only [subset_iff, mem_insert, mem_erase, ne.def],
-                exact λ gg hgg, or.inr ⟨λ ggx, hX.2.1 $ ggx ▸ hgg, mem_of_subset hB2filt.2 hgg⟩ },
-              exact not_lt_of_le (hB2min (insert Y $ erase B2 X) $ mem_filter.mpr
-                  ⟨hYbases, hysubY⟩) hssubY }) }) }, clear hB2min,
+def indep (b : of_bases E) : of_indep E :=
+{ indep := b.indep_indep,
+  empty_mem_indep := mem_filter.mpr ⟨empty_mem_powerset univ,
+    exists.elim (exists_mem_of_ne_empty b.bases_not_empty) $
+      λ a ha, exists.intro a $ exists.intro ha $ empty_subset a⟩,
+  indep_of_subset_indep := begin
+      intros x y hx hxy,
+      simp only [indep_indep, mem_powerset, filter_congr_decidable,
+        exists_prop, mem_filter] at hx ⊢,
+      split, { exact subset.trans hxy hx.1, },
+      { rcases hx.2 with ⟨a, ha⟩, use a, exact ⟨ha.1, subset.trans hxy ha.2⟩, },
+    end,
+  indep_exch := begin
+    intros x y hx hy hcard, unfold indep_indep at hx hy ⊢,
+    let F := (b.bases).filter (λ S, S ⊆ y),
+    by_contra h, simp only [mem_powerset, not_exists, and_imp, filter_congr_decidable,
+      exists_prop, mem_filter, not_and, mem_sdiff] at hx hy h,
+    rcases hx.2 with ⟨b1, ⟨hb1bases, hxb1⟩⟩,
+    rcases hy.2 with ⟨b2, hb2⟩,
+    have := (min_fun_of_ne_empty (λ f, card (f \ (y ∪ b1))) $
+      ne_empty_of_mem $ mem_filter.mpr hb2),
+    rcases this with ⟨B2, ⟨hB2filt, hB2min⟩⟩, clear hb2 b2,
+    replace hB2filt : B2 ∈ b.bases ∧ y ⊆ B2 := mem_filter.mp hB2filt,
+    have hysdiff : y \ b1 = y \ x := by { simp only [ext, mem_sdiff],
+      exact λ gg, ⟨λ hgg, ⟨hgg.1, λ hggnx, hgg.2 $ mem_of_subset hxb1 hggnx⟩,
+        λ hgg, ⟨hgg.1, λ ggb1, h gg hgg.1 hgg.2 (insert_subset.mpr
+        ⟨mem_of_subset hy.1 hgg.1, hx.1⟩) b1 hb1bases $ insert_subset.mpr ⟨ggb1, hxb1⟩⟩⟩, },
+    have hB2yub1: B2 \ (y ∪ b1) = ∅ := by { by_contra H,
+      rcases (exists_mem_of_ne_empty H) with ⟨X, hX⟩, clear H,
+      simp only [not_or_distrib, mem_union, mem_sdiff] at hX,
+      have hXB2b1 : X ∈ B2 \ b1 := by { rw mem_sdiff, exact ⟨hX.1, hX.2.2⟩ },
+      rcases (b.basis_exch hB2filt.1 hb1bases hXB2b1) with ⟨Y, ⟨hYb1B2, hYbases⟩⟩,
+      rw mem_sdiff at hYb1B2 hXB2b1,
+      have hssubY : insert Y (erase B2 X) \ (y ∪ b1) ⊂  B2 \ (y ∪ b1) :=
+        by { rw [ssubset_iff],
+        use X,
+        simp only [subset_iff, not_or_distrib, mem_union, mem_insert, not_and, mem_sdiff,
+          not_not, mem_erase, not_true, or_false, ne.def, false_and, or_false,
+          eq_self_iff_true],
+        exact ⟨λ hXY, (hYb1B2.2 $ hXY ▸ hXB2b1.1).elim,
+        λ gg hgg, or.elim hgg (λ ggx, ggx.symm ▸ hX) $ λ ggor2, or.elim ggor2.1
+          (λ ggY, false.elim $ ((ggY ▸ ggor2.2.2) hYb1B2.1)) $
+            λ ggXB2, ⟨ggXB2.2, ggor2.2⟩⟩, },
+      replace hssubY := card_lt_card hssubY,
+      have hysubY : y ⊆ insert Y (erase B2 X) := by {
+        simp only [subset_iff, mem_insert, mem_erase, ne.def],
+        exact λ gg hgg, or.inr ⟨λ ggx, hX.2.1 $ ggx ▸ hgg, mem_of_subset hB2filt.2 hgg⟩ },
+      exact not_lt_of_le (hB2min (insert Y $ erase B2 X) $ mem_filter.mpr
+          ⟨hYbases, hysubY⟩) hssubY }, clear hB2min,
       rw [←subset_iff_sdiff_eq_empty, subset_iff] at hB2yub1, simp only [mem_union] at hB2yub1,
       have hB2b1y : B2 \ b1 = y \ b1 := by { simp only [ext, mem_sdiff],
         exact λ gg, ⟨λ hgg, ⟨or.elim (hB2yub1 hgg.1) id $ λ hb1, false.elim $ hgg.2 hb1, hgg.2⟩,
             λ hgg, ⟨mem_of_subset hB2filt.2 hgg.1, hgg.2⟩⟩ },
       rw [hysdiff] at hB2b1y, clear hysdiff,
       have hb1xuB2 : b1 \ (x ∪ B2) = ∅ := by { by_contra H,
-        exact exists.elim (exists_mem_of_ne_empty H)
-          (by { intros X hX, simp only [not_or_distrib, mem_union, mem_sdiff] at hX,
-          exact exists.elim (b.basis_exch hb1.1 hB2filt.1 $ mem_sdiff.mpr ⟨hX.1, hX.2.2⟩)
-            (by { intros Y hY, rw mem_sdiff at hY,
-            have hYyx : Y ∈ y ∧ Y ∉ x := mem_sdiff.mp (hB2b1y ▸ (mem_sdiff.mpr hY.1)),
-            have hxYsub : insert Y x ⊆ insert Y (erase b1 X) := by {
-              simp only [subset_iff, mem_insert, mem_erase, ne.def],
-              exact λ gg hgg, or.elim hgg (λ ggY, or.inl ggY) $ λ ggx, or.inr ⟨λ ggX, hX.2.1 $
-                ggX ▸ ggx, mem_of_subset hb1.2 ggx⟩ },
-            have : insert Y x ⊆ E := insert_subset.mpr ⟨mem_of_subset hy.1 hYyx.1, hx.1⟩,
-            exact h Y hYyx.1 hYyx.2 this (insert Y $ erase b1 X) hY.2 hxYsub }) }) },
+        rcases (exists_mem_of_ne_empty H) with ⟨X, hX⟩,
+        simp only [not_or_distrib, mem_union, mem_sdiff] at hX,
+        rcases (b.basis_exch hb1bases hB2filt.1 $ mem_sdiff.mpr ⟨hX.1, hX.2.2⟩) with ⟨Y, hY⟩,
+        rw mem_sdiff at hY,
+        have hYyx : Y ∈ y ∧ Y ∉ x := mem_sdiff.mp (hB2b1y ▸ (mem_sdiff.mpr hY.1)),
+        have hxYsub : insert Y x ⊆ insert Y (erase b1 X) := by {
+          simp only [subset_iff, mem_insert, mem_erase, ne.def],
+          exact λ gg hgg, or.elim hgg (λ ggY, or.inl ggY) $ λ ggx, or.inr ⟨λ ggX, hX.2.1 $
+            ggX ▸ ggx, mem_of_subset hxb1 ggx⟩ },
+        exact h Y hYyx.1 hYyx.2 (subset_univ (insert Y x)) (insert Y $ erase b1 X) hY.2 hxYsub, },
       clear h hx hy,
       rw [←subset_iff_sdiff_eq_empty, subset_iff] at hb1xuB2, simp only [mem_union] at hb1xuB2,
       have hb1B2 : b1 \ B2 = x \ B2 := by { simp only [ext, mem_sdiff],
         exact λ gg, ⟨λ hgg, ⟨or.elim (hb1xuB2 hgg.1) id $ λ ggB2, false.elim $ hgg.2 ggB2, hgg.2⟩,
-            λ hgg, ⟨mem_of_subset hb1.2 hgg.1, hgg.2⟩⟩ }, clear hb1xuB2,
+            λ hgg, ⟨mem_of_subset hxb1 hgg.1, hgg.2⟩⟩ }, clear hb1xuB2,
       replace hb1B2 : b1 \ B2 ⊆ x \ y := hb1B2.symm ▸ (sdiff_subset_sdiff (subset.refl x)
           hB2filt.2),
-      have hcardeq : card b1 = card B2 := bases_card_eq hb1.1 hB2filt.1,
+      have hcardeq : card b1 = card B2 := bases_card_eq hb1bases hB2filt.1,
       have hcardb1B2 : card (b1 \ B2) = card (B2 \ b1) := calc
         card (b1 \ B2) = card b1 - card (b1 ∩ B2) : card_sdiff_eq b1 B2
         ... = card B2 - card (B2 ∩ b1) : by rw [hcardeq, inter_comm]
@@ -759,134 +1106,214 @@ begin
         ... ≤ card (x \ y) : card_le_of_subset hb1B2,
       rw [card_sdiff_eq y x, card_sdiff_eq x y, inter_comm] at hcardcontra0,
       have hcardcontra : card y ≤ card x := nat.le_of_le_of_sub_le_sub_right
-          (card_le_of_subset $ @inter_subset_left _ _ x y) hcardcontra0,
-      exact not_lt_of_le hcardcontra hcard })
-end⟩
+          (card_le_of_subset $ inter_subset_left x y) hcardcontra0,
+      exact not_lt_of_le hcardcontra hcard,
+    end }
 
-instance base_indep : has_coe (bases E) (indep E) := ⟨indep_of_bases⟩
-instance indep_base : has_coe (indep E) (bases E) := ⟨bases_of_indep⟩
+-- instance base_indep : has_coe (bases E) (indep E) := ⟨indep_of_bases⟩
+-- instance indep_base : has_coe (indep E) (bases E) := ⟨bases_of_indep⟩
 
 /-- second part of Theorem 1.2.3 -/
-theorem base_indep_base (B : bases E) : B = bases_of_indep (indep_of_bases B) :=
-suffices B.bases = (bases_of_indep $ indep_of_bases B).bases, from eq_of_base_eq this,
-by { simp only [indep_of_bases, bases_of_indep, indep_indep_of_bases, is_basis,
-  ext, bases_bases_of_indep, mem_filter, mem_powerset, not_and, not_exists, exists_prop],
-exact λ b, iff.intro
-  (λ hb, have hB : b ⊆ E := mem_powerset.mp (mem_of_subset B.bases_subset_powerset_ground hb),
-    ⟨hB, ⟨⟨hB, exists.intro b ⟨hb, subset.refl b⟩⟩, λ b' _ hbb' _ _ hx H,
-    (ne_of_lt $ lt_of_lt_of_le (card_lt_card hbb') $ card_le_of_subset H) $ bases_card_eq hb hx⟩⟩) $
-  λ hb, exists.elim hb.2.1.2 $ λ a ha, have a ⊆ E := mem_powerset.mp $
-    B.bases_subset_powerset_ground ha.1, by { by_cases h : a = b,
-      { exact h ▸ ha.1 },
-      { have hba : b ⊂ a := lt_iff_ssubset.mp (lt_of_le_of_ne (le_iff_subset.mpr ha.2) $ ne.symm h),
-        exact false.elim (hb.2.2 a this hba this a ha.1 $ subset.refl a) } } }
+theorem base_indep_base (B : of_bases E) : B = B.indep.bases :=
+suffices B.bases = B.indep.bases.bases, from eq_of_base_eq this,
+begin
+  simp only [of_bases.indep, of_indep.bases, indep_indep, is_basis,
+  ext, bases_bases, mem_filter, mem_powerset, not_and, not_exists, exists_prop],
+  intro b, split,
+  { intro hb,
+    have hB : b ⊆ univ := subset_univ b,
+    split,
+    { exact hB, },
+    { split, { split, { exact hB, }, { use b, exact ⟨hb, subset.refl b⟩, } },
+      { intros b' hbb' _ _ hx H,
+        exact (ne_of_lt $ lt_of_lt_of_le (card_lt_card hbb') $ card_le_of_subset H)
+          (bases_card_eq hb hx) } } },
+  { rintro ⟨_, ⟨⟨_, hbexists⟩, hb⟩⟩, rcases hbexists with ⟨a, ⟨habases, hba⟩⟩,
+    have : a ⊆ univ := subset_univ a,
+    by_cases h : a = b,
+    { exact h ▸ habases, },
+    { have hba' : b ⊂ a := lt_iff_ssubset.mp (lt_of_le_of_ne (le_iff_subset.mpr hba) $ ne.symm h),
+      exact (hb a hba' this a habases $ subset.refl a).elim, } },
+end
 
-theorem indep_base_indep (M : indep E) : M = indep_of_bases (bases_of_indep M) :=
-suffices M.indep = (indep_of_bases $ bases_of_indep M).indep, from eq_of_indep_eq this,
-by { simp only [indep_of_bases, bases_of_indep, indep_indep_of_bases, is_basis,
-  ext, bases_bases_of_indep, mem_filter, mem_powerset, exists_prop],
-  exact λ I, iff.intro (λ hI, ⟨mem_powerset.mp $ mem_of_subset M.indep_subset_powerset_ground hI,
-  exists.elim (exists_basis_containing_indep hI) $ λ B hB, by { unfold is_basis at hB,
-    exact exists.intro B ⟨⟨mem_powerset.1 $ mem_of_subset M.indep_subset_powerset_ground hB.2.1,
-      hB.2⟩, hB.1⟩ }⟩) $ λ hI, exists.elim hI.2 $ λ B hB, M.indep_of_subset_indep hB.1.2.1 hB.2 }
+end of_bases
+
+namespace of_indep
+open of_bases
+variable {E}
+
+theorem indep_base_indep (M : of_indep E) : M = M.bases.indep :=
+suffices M.indep = M.bases.indep.indep, from eq_of_indep_eq this,
+begin
+  simp only [of_bases.indep, of_indep.bases, indep_indep, is_basis,
+  ext, bases_bases, mem_filter, mem_powerset, exists_prop],
+  intro I, split,
+  { intro hI, split,
+    { exact subset_univ I, },
+    { rcases (exists_basis_containing_indep hI) with ⟨B, hB⟩,
+      unfold is_basis at hB,
+      use B, exact ⟨⟨subset_univ B, hB.2⟩, hB.1⟩ } },
+  { rintro ⟨hIuniv, hIexists⟩, rcases hIexists with ⟨B, ⟨⟨hBuniv, ⟨hBindep, hB'⟩⟩, hIB⟩⟩,
+    exact M.indep_of_subset_indep hBindep hIB, },
+end
 
 /-- Corollary 1.2.6 -/
-theorem existsu_fund_circ_of_basis {m : indep E} {B : finset α} (hB : is_basis B m) {e : α}
-  (he : e ∈ E \ B) : ∃ C, C ∈ circuits_circ_of_indep m ∧ C ⊆ insert e B ∧
-  ∀ C' ∈ circuits_circ_of_indep m, C' ⊆ insert e B → C' = C :=
+theorem existsu_fund_circ_of_basis {m : of_indep E} {B : finset E} (hB : is_basis B m) {e : E}
+  (he : e ∈ univ \ B) : ∃ C, C ∈ m.circuits_circuits ∧ C ⊆ insert e B ∧
+  ∀ C' ∈ m.circuits_circuits, C' ⊆ insert e B → C' = C :=
 begin
   unfold is_basis at hB, rw mem_sdiff at he,
-  have : insert e B ∉ m.indep := hB.2 (insert e B) (insert_subset.mpr ⟨he.1,
-    mem_powerset.mp $ mem_of_subset m.indep_subset_powerset_ground hB.1⟩) (ssubset_insert he.2),
-  replace := existsu_circuit_of_dep_of_insert_indep hB.1 he.1 this,
-  exact exists.elim this (λ C ⟨hCcirc, HC⟩, exists.intro C $
-    ⟨hCcirc, ⟨HC.1, λ C' hC'circ hC', HC.2.2 C' hC'circ ⟨hC', HC.2.1⟩⟩⟩)
+  have : insert e B ∉ m.indep := hB.2 (insert e B) (ssubset_insert he.2),
+  replace := existsu_circuit_of_dep_of_insert hB.1 this,
+  rcases this with ⟨C, ⟨hCcirc, ⟨HCinsert, ⟨_, HC⟩⟩⟩⟩,
+  use C,
+  exact ⟨hCcirc, ⟨HCinsert, λ C' hC'circ hC', HC C' hC'circ hC'⟩⟩,
 end
 
 section encodable
 
-def fund_circ_of_basis [encodable α] {m : indep E} {B : finset α} (hB : is_basis B m) {e : α}
-  (he : e ∈ E \ B) : finset α :=
+variable [encodable E]
+
+def fund_circ_of_basis {m : of_indep E} {B : finset E} (hB : is_basis B m) {e : E}
+  (he : e ∈ univ \ B) : finset E :=
 encodable.choose (existsu_fund_circ_of_basis hB he)
 
-def fund_circ_of_basis_spec [encodable α] {m : indep E} {B : finset α} (hB : is_basis B m) {e : α}
-  (he : e ∈ E \ B) : fund_circ_of_basis hB he ∈ circuits_circ_of_indep m ∧
-  fund_circ_of_basis hB he  ⊆ insert e B ∧ ∀ C' ∈ circuits_circ_of_indep m, C' ⊆ insert e B →
+lemma fund_circ_of_basis_spec {m : of_indep E} {B : finset E} (hB : is_basis B m) {e : E}
+  (he : e ∈ univ \ B) : fund_circ_of_basis hB he ∈ m.circuits_circuits ∧
+  fund_circ_of_basis hB he  ⊆ insert e B ∧ ∀ C' ∈ m.circuits_circuits, C' ⊆ insert e B →
   C' = fund_circ_of_basis hB he :=
 encodable.choose_spec (existsu_fund_circ_of_basis hB he)
 
 end encodable
 
+end of_indep
+
 -- § 1.3
+namespace of_indep
 
-def indep_of_restriction (m : indep E) {X : finset α} (hXE : X ⊆ E) : finset (finset α) :=
-(m.indep).filter (λ I, I ⊆ X)
+variable {E}
 
-def restriction (m : indep E) {X : finset α} (hXE : X ⊆ E) : indep X :=
-⟨indep_of_restriction m hXE,
-by simp only [indep_of_restriction, subset_iff, and_imp, imp_self,
-  mem_powerset, mem_filter, forall_true_iff],
-by simp only [indep_of_restriction, m.empty_mem_indep, empty_subset, and_self, mem_filter],
-by { unfold indep_of_restriction, exact λ x y hx hy, mem_filter.mpr
-  ⟨m.indep_of_subset_indep (mem_filter.mp hx).1 hy, subset.trans hy (mem_filter.mp hx).2⟩ },
-by { unfold indep_of_restriction, exact λ x y hx hy hcard,
-  have hxm : x ∈ m.indep := (mem_filter.mp hx).1, have hym : y ∈ m.indep := (mem_filter.mp hy).1,
-  have hxX : x ⊆ X := (mem_filter.mp hx).2, have hyX : y ⊆ X := (mem_filter.mp hy).2,
-  have H : _ := m.indep_exch hxm hym hcard,
-  let ⟨e, H, h₁⟩ := H in
-    ⟨e, H, mem_filter.mpr ⟨h₁, insert_subset.mpr ⟨mem_of_subset hyX (mem_sdiff.mp H).1, hxX⟩⟩⟩ }⟩
+/-- def by Mario Carneiro https://leanprover.zulipchat.com/#narrow/stream/113489-new-members/subject/finset.20of.20subtype.20from.20filter/near/134578668 -/
+def indep_of_restriction (m : of_indep E) (X : finset E) : finset (finset {x : E // x ∈ X}) :=
+(m.indep).filter_map $ prestrict X
+-- def indep_of_restriction (m : indep E) (X : finset E) : finset (finset E) :=
+-- (m.indep).filter (λ I, I ⊆ X)
 
-def deletion (m : indep E) {X : finset α} (hXE : X ⊆ E) : indep (E \ X) :=
-restriction m $ sdiff_subset E X
+lemma mem_restriction {m : of_indep E} {X : finset E} {x : finset {y : E // y ∈ X}} :
+x ∈ indep_of_restriction m X ↔ ↑x ∈ m.indep /-∧ ↑x ⊆ X -- just use finset_embed_subset_univ -/ :=
+begin
+  simp only [indep_of_restriction,
+    function.embedding.subtype, function.embedding.coe_fn_mk,
+    mem_filter_map],
+  split,
+  { rintro ⟨a, ⟨haindep, ha⟩⟩,
+    convert haindep,
+    rw option.mem_def at ha,
+    exact (subset_of_prestrict_eq_some ha).2, },
+  { intro h,
+    use [↑x, h],
+    rw option.mem_def,
+    have hsub : ↑x ⊆ X := finset_embed_subset_univ x,
+    rcases prestrict_eq_some_of_subset hsub with ⟨x', hx', H⟩,
+    rw [hx', ←finset_embed_inj H], },
+end
 
-notation m `¦` hxe := restriction m hxe
-notation m `\` hxe := deletion m hxe
+def restriction (m : of_indep E) (X : finset E) : of_indep {x : E // x ∈ X} :=
+{ indep := indep_of_restriction m X,
+  empty_mem_indep := mem_restriction.mpr m.empty_mem_indep,
+  indep_of_subset_indep := λ x y hx hyx, have hx' : ↑x ∈ m.indep := mem_restriction.mp hx,
+  have hyx' : ↑y ⊆ (↑x : finset E) := finset_embed_subset.mp hyx,
+  mem_restriction.mpr (m.indep_of_subset_indep hx' hyx'),
+  indep_exch := begin
+    intros x y hx hy hcard,
+    have hx' : _ := mem_restriction.mp hx, have hy' : _ := mem_restriction.mp hy,
+    have hcard' : card (↑x : finset E) < card ↑y := calc
+      card (↑x : finset E) = card x : (finset_embed_card x).symm
+      ... < card y : hcard
+      ... = card ↑y : finset_embed_card y,
+    have H : _ := m.indep_exch hx' hy' hcard',
+    rcases H with ⟨e, he⟩,
+    rw mem_sdiff at he,
+    have He : e ∈ X := mem_of_subset (finset_embed_subset_univ y) he.1.1,
+    let e' := subtype.mk e He,
+    have heyx : e' ∈ y \ x := mem_sdiff.mpr ⟨finset_embed_mem.mpr he.1.1,
+      λ H, he.1.2 $ finset_embed_mem.mp H⟩,
+    have heinsert : ↑(insert e' x) ∈ m.indep :=
+      by { have : (↑(insert e' x) : finset E) = insert e ↑x :=
+        by simp only [ext, finset_embed_coe_def, finset_embed, function.embedding.subtype,
+          exists_prop, finset.mem_map, iff_self, exists_and_distrib_right, finset.map_insert,
+          exists_eq_right, function.embedding.coe_fn_mk, finset.mem_insert, subtype.exists,
+          forall_true_iff],
+      exact this.symm ▸ he.2 },
+    have H : insert e' x ∈ indep_of_restriction m X :=
+      mem_restriction.mpr heinsert,
+    exact exists.intro e' ⟨heyx, H⟩,
+  end }
 
-lemma restriction_subset_restriction {X : finset α} (hX : X ⊆ E) (m : indep E) :
-  (m ¦ hX).indep ⊆ m.indep :=
-by { simp only [restriction, indep_of_restriction, subset_iff, and_imp,
-  filter_congr_decidable, mem_filter],
-  exact λ _ hX'I _, hX'I }
+-- what about {x : E // x ∉ X} ?
+def deletion (m : of_indep E) (X : finset E) : of_indep {x : E // x ∈ univ \ X} :=
+restriction m (univ \ X)
 
-lemma restriction_trans {X Y : finset α} (hXY : X ⊆ Y) (hY : Y ⊆ E) (m : indep E) :
-  (m ¦ subset.trans hXY hY) = ((m ¦ hY) ¦ hXY) :=
+notation m `¦` X := restriction m X
+notation m `\` X := deletion m X
+
+lemma restriction_subset_restriction (m : of_indep E) (X : finset E) :
+  ↑(m ¦ X).indep ⊆ m.indep :=
+begin
+  rw [subset_iff],
+  intros I hI,
+  rw [finset_finset_embed_coe_def, finset_finset_embed] at hI,
+  simp only [exists_prop, function.embedding.coe_fn_mk, mem_map] at hI,
+  rcases hI with ⟨I', hI'indep, rfl⟩,
+  simp only [restriction, indep_of_restriction, mem_filter_map] at hI'indep,
+  rcases hI'indep with ⟨a, haindep, haI'⟩,
+  rw [option.mem_def] at haI',
+  convert haindep,
+  have := subset_of_prestrict_eq_some haI',
+  rw [←finset_embed_coe_def, this.2],
+end
+
+lemma restriction_trans {X Y : finset E} (hXY : X ⊆ Y) (m : of_indep E) :
+  (m ¦ X) = ((m ¦ Y) ¦ X) :=
 by { simp only [restriction, indep_of_restriction, ext, mem_filter],
   exact λ I, iff.intro (λ h, ⟨⟨h.1, subset.trans h.2 hXY⟩, h.2⟩) $ λ h, ⟨h.1.1, h.2⟩ }
 
-lemma subset_restriction_indep {X Y : finset α} {m : indep E} (hX : X ∈ m.indep) (hXY : X ⊆ Y)
-  (hY : Y ⊆ E) : X ∈ (m ¦ hY).indep :=
+lemma subset_restriction_indep {X Y : finset E} {m : of_indep E} (hX : X ∈ m.indep) (hXY : X ⊆ Y)
+  : X ∈ (m ¦ Y).indep :=
 by { simp only [restriction, indep_of_restriction, mem_filter], exact ⟨hX, hXY⟩ }
 
 /-def spans (X : finset α) {Y : finset α} (hY : Y ⊆ E) (m : indep E) : Prop :=
 X ∈ bases_bases_of_indep (m ¦ hY)-/
 
-lemma exists_basis_of_subset {X : finset α} (hXE : X ⊆ E) (m : indep E) :
-  ∃ B, B ∈ bases_bases_of_indep (m ¦ hXE) :=
-exists_mem_of_ne_empty $ B1_of_indep (m ¦ hXE)
+lemma exists_basis_of_subset (X : finset E) (m : of_indep E) :
+  ∃ B, B ∈ (m ¦ X).bases_bases :=
+exists_mem_of_ne_empty $ B1 (m ¦ X)
 
 /-lemma inter_of_span_of_subset_span {m : indep E} {X Y bX bY : finset α} {hXE : X ⊆ E}
   (hbX : spans bX hXE m) {hYE : Y ⊆ E} (hbY : spans bY hYE m) (hbXbY : bX ⊆ bY) : bY ∩ X = bX :=
 sorry-/
 
+#exit
+
 section encodable
 variable [encodable α]
 
-def basis_of_subset {X : finset α} (hXE : X ⊆ E) (m : indep E) : finset α :=
-encodable.choose $ exists_basis_of_subset hXE m
+def basis_of_subset (X : finset E) (m : of_indep E) : finset α :=
+encodable.choose $ exists_basis_of_subset X m
 
-def basis_of_subset_spec {X : finset α} (hXE : X ⊆ E) (m : indep E) :
-  basis_of_subset hXE m ∈ bases_bases_of_indep (m ¦ hXE) :=
-encodable.choose_spec $ exists_basis_of_subset hXE m
+def basis_of_subset_spec {X : finset E} (m : of_indep E) :
+  basis_of_subset X m ∈ (m ¦ X).bases_bases :=
+encodable.choose_spec $ exists_basis_of_subset X m
 
 notation `𝔹` := basis_of_subset
 notation `𝔹ₛ` := basis_of_subset_spec
 
-def rank_of_subset {X : finset α} (hXE : X ⊆ E) (m : indep E) : ℕ :=
+def rank_of_subset {X : finset E} (m : of_indep E) : ℕ :=
 card $ 𝔹 hXE m
 
 notation `𝓇` := rank_of_subset
 
-lemma R2_of_indep (m : indep E) {X Y : finset α} (hXY : X ⊆ Y) (hYE : Y ⊆ E) :
+lemma R2 (m : of_indep E) {X Y : finset α} (hXY : X ⊆ Y) :
   𝓇 (subset.trans hXY hYE) m ≤ 𝓇 hYE m :=
 let hXE : X ⊆ E := subset.trans hXY hYE in let bX := 𝔹 hXE m in let bY := 𝔹 hYE m in
 have bXs : _ := 𝔹ₛ hXE m, have bYs : _ := 𝔹ₛ hYE m,
@@ -899,14 +1326,14 @@ by { simp only [bases_bases_of_indep, mem_powerset, filter_congr_decidable, mem_
     ... = card bY : bases_of_indep_card_eq hB.2 bYs.2) }
 
 /-- Lemma 1.3.1 -/
-lemma R3_of_indep (m : indep E) {X Y : finset α} (hX : X ⊆ E) (hY : Y ⊆ E) :
+lemma R3 (m : of_indep E) {X Y : finset α} (hX : X ⊆ E) (hY : Y ⊆ E) :
   𝓇 (union_subset hX hY) m +
-  𝓇 (subset.trans (@inter_subset_left _ _ X Y) hX) m ≤
+  𝓇 (subset.trans (inter_subset_left X Y) hX) m ≤
   𝓇 hX m + 𝓇 hY m :=
 begin
-  have hXXuY : X ⊆ X ∪ Y := @subset_union_left _ _ X Y,
-  have hYXuY : Y ⊆ X ∪ Y := @subset_union_right _ _ X Y,
-  have hXiYX : X ∩ Y ⊆ X := @inter_subset_left _ _ X Y,
+  have hXXuY : X ⊆ X ∪ Y := subset_union_left X Y,
+  have hYXuY : Y ⊆ X ∪ Y := subset_union_right X Y,
+  have hXiYX : X ∩ Y ⊆ X := inter_subset_left X Y,
   have hXuY : X ∪ Y ⊆ E := union_subset hX hY,
   have hXiY : X ∩ Y ⊆ E := subset.trans hXiYX hX,
   let bXuY := 𝔹 hXuY m, let bXiY := 𝔹 hXiY m,
@@ -926,11 +1353,11 @@ begin
       exact bases_of_indep_card_eq bXuYs.2 hB.2 },
     have hBXuY : B ⊆ X ∪ Y := mem_powerset.mp ((m ¦ hXuY).indep_subset_powerset_ground hB.2.1),
     have hBX : B ∩ X ∈ (m ¦ hX).indep := have hsub : _ := restriction_trans hXXuY hXuY m,
-      have hBX : _ := ((m ¦ hXuY).indep_of_subset_indep hB.2.1 $ @inter_subset_left _ _ B X),
-      hsub.symm ▸ (subset_restriction_indep hBX (@inter_subset_right _ _ B X) hXXuY),
+      have hBX : _ := ((m ¦ hXuY).indep_of_subset_indep hB.2.1 $ inter_subset_left B X),
+      hsub.symm ▸ (subset_restriction_indep hBX (inter_subset_right B X) hXXuY),
     have hBY : B ∩ Y ∈ (m ¦ hY).indep := have hsub : _ := restriction_trans hYXuY hXuY m,
-      have hBY : _ := ((m ¦ hXuY).indep_of_subset_indep hB.2.1 $ @inter_subset_left _ _ B Y),
-      hsub.symm ▸ (subset_restriction_indep hBY (@inter_subset_right _ _ B Y) hYXuY),
+      have hBY : _ := ((m ¦ hXuY).indep_of_subset_indep hB.2.1 $ inter_subset_left B Y),
+      hsub.symm ▸ (subset_restriction_indep hBY (inter_subset_right B Y) hYXuY),
     have hBXr : card (B ∩ X) ≤ 𝓇 hX m := by { unfold rank_of_subset,
       exact card_of_indep_le_card_basis hBX bXs.2 },
     have hBYr : card (B ∩ Y) ≤ 𝓇 hY m := by { unfold rank_of_subset,
@@ -977,7 +1404,7 @@ r (union_subset hX hY) + r (subset.trans (@inter_subset_left _ _ X Y) hX) ≤ r 
 section encodable
 variable [encodable α]
 
-def rank_of_indep (m : indep E) : rank E :=
+def rank_of_indep (m : of_indep E) : rank E :=
 ⟨λ X hX, rank_of_subset hX m,
 λ X hX, ⟨dec_trivial, (by { have := basis_of_subset_spec hX m,
   simp only [bases_bases_of_indep, mem_powerset, filter_congr_decidable, mem_filter] at this,
@@ -993,7 +1420,7 @@ structure rank_R2_R3 (ground : finset α) :=
 (order_preserving {X Y : finset α} (hXY : X ⊆ Y) (hY : Y ⊆ ground) : r (subset.trans hXY hY) ≤ r hY)
 -- (R3)
 (submodular {X Y : finset α} (hX : X ⊆ ground) (hY : Y ⊆ ground) :
-r (union_subset hX hY) + r (subset.trans (@inter_subset_left _ _ X Y) hX) ≤ r hX + r hY)
+r (union_subset hX hY) + r (subset.trans (inter_subset_left X Y) hX) ≤ r hX + r hY)
 
 lemma congr_for_rank (rk : rank_R2_R3 E ) {X Y : finset α} (hX : X ⊆ E) (hY : Y ⊆ E) (h : X = Y) :
 rk.r hX = rk.r hY :=
@@ -1022,7 +1449,7 @@ begin
         exact mem_sdiff.mpr ((h y).mpr $ or.inr Hy.1) }, exact hy y this })
         hXS (by { simp only [ext, mem_insert, mem_sdiff] at h ⊢,
           exact λ y, iff.intro (λ Hy, Hy.1) $ λ Hy, ⟨Hy, ((h y).mpr $ or.inr Hy).2⟩ }) },
-    have hXuSiaX : (X ∪ S) ∩ insert a X ⊆ E := (subset.trans (@inter_subset_right _ _ (X ∪ S)
+    have hXuSiaX : (X ∪ S) ∩ insert a X ⊆ E := (subset.trans (inter_subset_right (X ∪ S)
       (insert a X)) haX),
     have hr₁ : rk.r (union_subset hXS haX) = rk.r hXuY :=
       by { exact congr_for_rank rk (union_subset hXS haX) hXuY (by {
@@ -1044,8 +1471,8 @@ begin
     ... ≥ rk.r (union_subset hXS haX) + rk.r hXuSiaX : rk.submodular (union_subset hX hS) haX
     ... = _ : by rw [hr₁, hr₂] },
   replace h₁ := le_of_add_le_add_right h₁,
-  have h₂ : rk.r hX ≤ rk.r hXuY := rk.order_preserving (@subset_union_left _ _ X Y) hXuY,
-  exact nat.le_antisymm h₁ h₂ }
+  have h₂ : rk.r hX ≤ rk.r hXuY := rk.order_preserving (subset_union_left X Y) hXuY,
+  exact nat.le_antisymm h₁ h₂, },
 end
 
 def indep_of_rank (r : rank E) : indep E :=
