src/filter_map.lean
@@ -1,0 +1,152 @@
+import .matroid
+
+open finset nat
+
+namespace matroid
+variables {E : Type*} [decidable_eq E] [fintype E]
+
+/-- def by Mario Carneiro https://leanprover.zulipchat.com/#narrow/stream/113489-new-members/subject/finset.20of.20subtype.20from.20filter/near/134721936 -/
+def {u v} indep.filter_map {α : Type u} {β : Type v} [decidable_eq α] [decidable_eq β]
+  [fintype α] [fintype β] (f : α → option β) (m : indep α) : indep β :=
+{ indep := m.indep.image (filter_map f),
+  empty_mem_indep := mem_image.2 ⟨∅, m.empty_mem_indep, rfl⟩,
+  indep_of_subset_indep := λ x y, begin
+    rw [mem_image, mem_image],
+    rintro ⟨x, hx, rfl⟩ xy,
+    refine ⟨x.filter (λ a, ∃ b ∈ f a, b ∈ y),
+      m.indep_of_subset_indep hx (filter_subset _), _⟩,
+    ext b, simp only [filter_congr_decidable, exists_prop, mem_filter,
+      mem_filter_map, option.mem_def], split,
+    { rintro ⟨a, ⟨ha, b', hb', hy⟩, hb⟩,
+      rcases option.some_inj.1 (hb.symm.trans hb'),
+      exact hy, },
+    { intro hb,
+      rcases mem_filter_map.1 (xy hb) with ⟨a, ha, ab⟩,
+      exact ⟨a, ⟨ha, b, ab, hb⟩, ab⟩, },
+  end,
+  indep_exch := λ x y, begin
+    rw [mem_image, mem_image],
+    rintro ⟨x, xi, rfl⟩ ⟨y, yi, rfl⟩ xy,
+    rcases exists_subset_filter_map_eq f x with ⟨z, zx, hz, cz⟩,
+    rcases exists_subset_filter_map_eq f y with ⟨w, wy, hw, cw⟩,
+    have zi := m.indep_of_subset_indep xi zx,
+    have wi := m.indep_of_subset_indep yi wy,
+    rw [hz, cz, hw, cw] at xy, rw [hz, hw], clear xi zx hz x yi wy hw y,
+    induction h : card (w \ z) generalizing z,
+    { have := ext.1 (card_eq_zero.1 h),
+      simp only [not_and, mem_sdiff, not_not, iff_false, not_mem_empty] at this,
+      exact (not_le_of_gt xy (card_le_of_subset this)).elim, },
+    rcases m.indep_exch zi wi xy with ⟨a, ha, ii⟩, rw mem_sdiff at ha,
+    rcases mem_of_card_filter_map cw ha.1 with ⟨b, ab⟩,
+    by_cases bz : b ∈ filter_map f z,
+    { rcases mem_filter_map.1 bz with ⟨a', ha', fa'⟩,
+      let z' := erase (insert a z) a',
+      have az' : a ∈ z',
+      { refine mem_erase.2 ⟨mt _ ha.2, mem_insert_self _ _⟩,
+        rintro rfl, exact ha', },
+      have inz : insert a' z' = insert a z,
+      { rw [insert_erase (mem_insert_of_mem ha')], },
+      have zi' : z' ∈ m.indep :=
+        m.indep_of_subset_indep ii (erase_subset _ _),
+      have bz' : b ∈ filter_map f z' :=
+        mem_filter_map.2 ⟨a, az', ab⟩,
+      have hz' : z'.filter_map f = z.filter_map f,
+      { rw [← insert_eq_of_mem bz', ← filter_map_insert_some f fa',
+          inz, filter_map_insert_some f ab, insert_eq_of_mem bz], },
+      have cz' : card z' = card z,
+      { rw [← add_right_inj 1, ← card_insert_of_not_mem (not_mem_erase _ _),
+          inz, card_insert_of_not_mem ha.2], },
+      replace ih := ih z', rw [hz', cz'] at ih,
+      refine ih cz zi' xy ((add_right_inj 1).1 $ eq.trans _ h),
+      rw [← card_insert_of_not_mem (λ h, (mem_sdiff.1 h).2 az')],
+      congr, ext c, simp only [not_imp_comm, mem_insert, not_and, mem_sdiff, mem_erase, ne.def], split,
+      { rintro (rfl | ⟨h₁, h₂⟩),
+        { exact ha, },
+        { refine ⟨h₁, λ h₃, h₂ (λ h₄, _) (or.inr h₃)⟩,
+          subst c,
+          rcases inj_of_card_filter_map cw ha.1 h₁ ab fa',
+          exact ha.2 h₃, } },
+      { rintro ⟨h₁, h₂⟩,
+        refine or_iff_not_imp_left.2 (λ h₃, ⟨h₁, _⟩),
+        rintro h₄ (rfl | h₅),
+        { exact h₃ rfl, }, { exact h₂ h₅, } } },
+    { exact ⟨b, mem_sdiff.2 ⟨mem_filter_map.2 ⟨_, ha.1, ab⟩, bz⟩,
+        mem_image.2 ⟨_, ii, by rw [filter_map_insert_some f ab]⟩⟩, },
+  end }
+
+/-- This is not the right definition! This removes all elements of X from each independent set,
+but we want to remove all independent sets that contain elements of X.
+
+This definition is like looking at "augmented" independence (i.e. we look at
+which additions to a set X preserve independence)
+-/
+def partial_restrict {X : finset E} (x : E) : option {x : E // x ∈ X} :=
+if h : x ∈ X then some ⟨x, h⟩ else none
+
+lemma partial_restrict_eq {X : finset E} (x : {x : E // x ∈ X}) :
+partial_restrict x.val = some x :=
+begin
+  convert dif_pos _,
+  exact (subtype.eta x x.property).symm,
+end
+
+lemma partial_restrict_inj {X : finset E} (x : E) (y : {x : E // x ∈ X}) :
+(partial_restrict x) = some y ↔ x = y.val :=
+begin
+  split,
+  { intro h,
+    by_cases hX : x ∈ X,
+    { let x' : {x : E // x ∈ X} := ⟨x, hX⟩,
+      rw partial_restrict_eq x' at h,
+      cases h' : h,
+      refl, },
+    exfalso,
+    have : partial_restrict x = none := dif_neg hX,
+    rw this at h,
+    cases h, },
+  { rintro rfl,
+    exact partial_restrict_eq y, },
+end
+
+def restriction_aug (m : indep E) (X : finset E) : indep {x : E // x ∈ X} :=
+m.filter_map $ partial_restrict
+
+lemma indep_of_restriction_aug (m : indep E) (X : finset E) (i : (finset {x : E // x ∈ X})) :
+  ↑i ∈ m.indep ∧ ↑i ⊆ X → i ∈ (restriction_aug m X).indep :=
+begin
+  simp only [restriction_aug, indep.filter_map, mem_image, exists_prop],
+  -- conv_lhs { congr, funext,
+  --   rw [subset.antisymm_iff, subset_iff, subset_iff], },
+  -- split,
+  -- { rintro ⟨a, haindep, ha⟩,
+  --   -- replace ha1 := ha1 (ha2 i.property),
+  --   split,
+  --   { subst ha,
+  --     -- This goal is false.
+  --     rw [finset_embed_coe_def, finset_embed],
+  --     -- have :
+  --     -- have := mem_filter_map.1,
+  --     -- rw ha at this,
+  --     sorry, },
+  --   { rw subset_iff,
+  --     intros x hx,
+  --     have := finset_embed_subset_univ i,
+  --     exact mem_of_subset this hx, }, },
+  rintros ⟨hindep, hX⟩,
+  use [↑i, hindep],
+  rw [subset.antisymm_iff, subset_iff, subset_iff],
+  split,
+  { intros x hx,
+    rw mem_filter_map at hx,
+    rcases hx with ⟨a, ha, H⟩,
+    rw [option.mem_def, partial_restrict_inj] at H,
+    rw H at ha,
+    exact finset_embed_mem.2 ha, },
+  { intros x hx,
+    rw mem_filter_map,
+    replace hx : x.val ∈ ↑i := finset_embed_mem.1 hx,
+    use [x.val, hx],
+    rw [option.mem_def, partial_restrict_eq], }
+end
+
+end matroid
