src/matroid-old.lean
@@ -1,0 +1,1157 @@
+/-
+Matroids, after Chapter 1 of Oxley, Matroid Theory, 1992.
+-/
+import data.finset tactic.wlog data.equiv.list tactic.find
+
+variables {α : Type*} {β : Type*} [decidable_eq α]
+/- For mathlib?: -/
+/- Everything from here to inter_of_subsete is by Mario Carneiro:
+https://gist.github.com/digama0/edc2a9fe4d468c3921c87650eea5b77a -/
+namespace multiset
+open nat
+
+@[simp] theorem card_filter_map_le {α β} {f : α → option β}
+  (s : multiset α) : card (filter_map f s) ≤ card s :=
+multiset.induction_on s (nat.zero_le _) begin
+  intros a s IH,
+  cases h : f a,
+  { rw [filter_map_cons_none _ _ h, card_cons],
+    exact le_succ_of_le IH },
+  { rw [filter_map_cons_some _ _ _ h, card_cons, card_cons],
+    exact succ_le_succ IH }
+end
+
+end multiset
+
+namespace finset
+open nat
+
+def filter_map {α β} [decidable_eq β] (f : α → option β) (s : finset α) : finset β :=
+(s.1.filter_map f).to_finset
+
+@[simp] theorem filter_map_empty {α β} [decidable_eq β] (f : α → option β) :
+  filter_map f ∅ = ∅ := rfl
+
+@[simp] theorem mem_filter_map {α β} [decidable_eq β] {f : α → option β} {s : finset α}
+  {b : β} : b ∈ s.filter_map f ↔ ∃ a ∈ s, b ∈ f a :=
+by simp [filter_map]; refl
+
+theorem card_filter_map_le {α β} [decidable_eq β] {f : α → option β} {s : finset α} :
+  card (s.filter_map f) ≤ card s :=
+le_trans (multiset.card_le_of_le $ multiset.erase_dup_le _)
+  (multiset.card_filter_map_le _)
+
+theorem filter_map_insert_none {α β} [decidable_eq α] [decidable_eq β]
+  (f : α → option β) {a : α} {s : finset α} (hf : f a = none) :
+  filter_map f (insert a s) = filter_map f s :=
+begin
+  by_cases a ∈ s,
+  { rw insert_eq_of_mem h },
+  { simp [filter_map, multiset.ndinsert_of_not_mem h,
+      multiset.filter_map_cons_none _ _ hf] }
+end
+
+theorem filter_map_insert_some {α β} [decidable_eq α] [decidable_eq β]
+  (f : α → option β) {a : α} {s : finset α} {b} (hf : f a = some b) :
+  filter_map f (insert a s) = insert b (filter_map f s) :=
+begin
+  by_cases a ∈ s,
+  { rw [insert_eq_of_mem h, insert_eq_of_mem],
+    exact mem_filter_map.2 ⟨_, h, hf⟩ },
+  { simp [filter_map, multiset.ndinsert_of_not_mem h, multiset.filter_map_cons_some _ _ _ hf] }
+end
+
+theorem mem_of_card_filter_map {α β} [decidable_eq β] {f : α → option β} {s : finset α}
+  (h : card (s.filter_map f) = card s) {a} (ha : a ∈ s) : ∃ b, b ∈ f a :=
+begin
+  haveI := classical.dec_eq α,
+  cases h' : f a with b, swap, {exact ⟨b, rfl⟩},
+  refine (not_succ_le_self (card (erase s a)) (_ : _ + 1 ≤ _)).elim,
+  rw [← insert_erase ha, filter_map_insert_none f h',
+    card_insert_of_not_mem (not_mem_erase _ _)] at h, rw ← h,
+  apply card_filter_map_le
+end
+
+theorem inj_of_card_filter_map {α β} [decidable_eq β] {f : α → option β} {s : finset α}
+  (H : card (s.filter_map f) = card s) {a a'} (ha : a ∈ s) (ha' : a' ∈ s)
+    {b} (h1 : b ∈ f a) (h2 : b ∈ f a') : a = a' :=
+begin
+  haveI := classical.dec_eq α,
+  by_contra h,
+  rw [← insert_erase ha', filter_map_insert_some f h2,
+    card_insert_of_not_mem (not_mem_erase _ _), insert_eq_of_mem] at H,
+  { refine (not_succ_le_self (card (erase s a')) (_ : _ + 1 ≤ _)).elim,
+    rw ← H, apply card_filter_map_le },
+  { exact mem_filter_map.2 ⟨_, mem_erase.2 ⟨h, ha⟩, h1⟩ }
+end
+
+theorem exists_subset_filter_map_eq
+  {α β} [decidable_eq α] [decidable_eq β] (f : α → option β) (s : finset α) :
+  ∃ t ⊆ s, s.filter_map f = filter_map f t ∧ card (t.filter_map f) = card t :=
+begin
+  refine finset.induction_on s ⟨∅, by simp⟩ _,
+  rintro a s as ⟨t, ss, st, ct⟩,
+  cases h : f a with b,
+  { refine ⟨t, subset.trans ss (subset_insert _ _), _, ct⟩,
+    simpa [filter_map_insert_none f h] },
+  simp [filter_map_insert_some f h],
+  by_cases h' : b ∈ filter_map f s,
+  { simp [h'],
+    refine ⟨t, subset.trans ss (subset_insert _ _), _, ct⟩,
+    simpa [filter_map_insert_none f h] },
+  { refine ⟨insert a t, _⟩,
+    have ha := mt (@ss _) as,
+    rw [filter_map_insert_some f h],
+    refine ⟨insert_subset_insert _ ss, by rw st, _⟩,
+    rw [← st, card_insert_of_not_mem h', st, ct, card_insert_of_not_mem ha] }
+end
+
+lemma inter_of_subset {A B : finset α} (h : A ⊆ B) : A ∩ B = A :=
+lattice.inf_of_le_left h
+
+lemma subset_iff_sdiff_eq_empty {x y : finset α} : x ⊆ y ↔ x \ y = ∅ :=
+by simp only [sdiff_eq_filter, eq_empty_iff_forall_not_mem, subset_iff, not_and,
+  not_not, finset.mem_filter]
+
+lemma empty_sdiff (E : finset α): E \ ∅ = E :=
+by simp only [ext, finset.not_mem_empty, and_true, iff_self, finset.mem_sdiff,
+  not_false_iff, forall_true_iff]
+
+lemma sdiff_subset (A B : finset α): A \ B ⊆ A :=
+(empty_sdiff A).subst $ sdiff_subset_sdiff (subset.refl A) $ empty_subset B
+
+lemma sdiff_eq_sdiff_inter (A B : finset α) : A \ B = A \ (A ∩ B) :=
+by { simp only [ext, not_and, mem_sdiff, mem_inter],
+  exact λ a, iff.intro (λ h, ⟨h.1, λ x, h.2⟩) (λ h, ⟨h.1, h.2 h.1⟩) }
+
+lemma card_eq_inter_sdiff (A B : finset α) : card A = card (A ∩ B) + card (A \ B) :=
+begin
+  have hA : A \ B ∪ A ∩ B = A := by { simp only [ext, mem_union, union_comm, mem_sdiff, mem_inter],
+    exact λ a, iff.intro (λ ha, or.elim ha (λ H, H.1) (λ H, H.1))
+      (by { intro ha, by_cases h : a ∈ B, { exact or.inl ⟨ha, h⟩ }, { exact or.inr ⟨ha, h⟩ } }) },
+  have : disjoint (A \ B) (A ∩ B) := by simp only [disjoint, empty_subset, inf_eq_inter,
+    inter_empty, sdiff_inter_self, inter_left_comm, le_iff_subset],
+  replace this := card_disjoint_union this, rwa [hA, add_comm] at this
+end
+
+lemma card_sdiff_eq (A B : finset α) : card (A \ B) = card A - card (A ∩ B) :=
+(nat.sub_eq_of_eq_add $ card_eq_inter_sdiff A B).symm
+
+lemma card_union_inter (A B : finset α) : card A + card B = card (A ∪ B) + card (A ∩ B) :=
+begin
+  have hBA : card B = card (B \ A) + card (A ∩ B) := inter_comm B A ▸
+    (add_comm (card (B ∩ A)) (card (B \ A))) ▸ (card_eq_inter_sdiff B A),
+  have Hdis : disjoint A (B \ A) := by simp only [disjoint, empty_subset, inf_eq_inter,
+    inter_sdiff_self, le_iff_subset],
+  have H : card A + card (B \ A) = card (A ∪ B) :=
+    (congr_arg card $ union_sdiff_self_eq_union.symm).substr (card_disjoint_union Hdis).symm,
+  calc
+  card A + card B = card A + card (B \ A) + card (A ∩ B) : by rw [add_assoc, hBA]
+  ... = card (A ∪ B) + card (A ∩ B) : by rw H
+end
+
+/- proof by Kenny Lau https://leanprover.zulipchat.com/#narrow/stream/113489-new-members/subject/choosing.20from.20difference.20of.20finsets/near/133624012 -/
+lemma exists_sdiff_of_card_lt {x y : finset α} (hcard : card x < card y) : ∃ e : α, e ∈ y \ x :=
+suffices ∃ e ∈ y, e ∉ x, by simpa only [exists_prop, finset.mem_sdiff],
+by_contradiction $ λ H, not_le_of_lt hcard $ card_le_of_subset $ by simpa only [not_exists,
+  exists_prop, not_and, not_not] using H
+
+/- proof by chris hughes
+https://leanprover.zulipchat.com/#narrow/stream/113489-new-members/subject/maximal.20finset.20in.20finset.20of.20finsets/near/133905271 -/
+lemma max_fun_of_ne_empty {F : finset β} (func : β → ℕ) (h : F ≠ ∅) :
+  ∃ x ∈ F, ∀ g ∈ F, func g ≤ func x :=
+let ⟨n, hn⟩ := (max_of_ne_empty (mt image_eq_empty.1 h) : ∃ a, a ∈ finset.max (F.image func)) in
+let ⟨x, hx₁, hx₂⟩ := mem_image.1 (mem_of_max hn) in
+  ⟨x, hx₁, hx₂.symm ▸ λ g hg, le_max_of_mem (mem_image.2 ⟨g, hg, rfl⟩) hn⟩
+
+lemma min_fun_of_ne_empty {F : finset β} (func : β → ℕ) (h : F ≠ ∅) :
+  ∃ x ∈ F, ∀ g ∈ F, func x ≤ func g :=
+let ⟨n, hn⟩ := (min_of_ne_empty $ mt image_eq_empty.1 h : ∃ a, a ∈ finset.min (F.image func)) in
+let ⟨x, hx₁, hx₂⟩ := mem_image.1 (mem_of_min hn) in
+  ⟨x, hx₁, hx₂.symm ▸ λ g hg, min_le_of_mem (mem_image.2 ⟨g, hg, rfl⟩) hn⟩
+
+section inst
+
+variables {F : finset α} {Q : finset α → Prop} [decidable_pred Q] {P : α → Prop} [decidable_pred P]
+
+instance decidable_not_forall (c₁ : finset (finset α)) :
+  decidable (∃ x : finset α, ¬(x ∈ c₁ → ¬Q x)) :=
+decidable_of_iff (∃ x ∈ c₁, Q x) $ by simp only [exists_prop, not_forall_not]
+
+instance decidable_exists_and_mem : decidable (∃ e, e ∈ F ∧ P e) :=
+decidable_of_iff (∃ e ∈ F, P e) $ by simp only [exists_prop, not_forall_not]
+
+end inst
+
+end finset
+
+open finset
+
+-- § 1.1
+
+namespace matroid
+
+variables {E : finset α}
+
+/-- `indep E` is the type of matroids (encoded as systems of independent sets) with ground set `E` :
+`finset α` -/
+structure indep (E : finset α) :=
+(indep : finset (finset α))
+(indep_subset_powerset_ground : indep ⊆ powerset E)
+-- (I1)
+(empty_mem_indep : ∅ ∈ indep)
+-- (I2)
+(indep_of_subset_indep {x y} (hx : x ∈ indep) (hyx : y ⊆ x) : y ∈ indep)
+-- (I3)
+(indep_exch {x y} (hx : x ∈ indep) (hy : y ∈ indep) (hcard : card x < card y)
+    : ∃ e, e ∈ y \ x ∧ insert e x ∈ indep)
+--attribute [class] indep
+
+instance indep_repr [has_repr α] (E : finset α) : has_repr (indep E) :=
+⟨λ m, has_repr.repr m.indep⟩
+
+theorem eq_of_indep_eq : ∀ {M₁ M₂ : indep E}, M₁.1 = M₂.1 → M₁ = M₂
+  | ⟨I₁, p₁, q₁, r₁, s₁⟩ ⟨I₂, p₂, q₂, r₂, s₂⟩ h :=
+by simpa only []
+
+/-- A circuit of a matroid is a minimal dependent subset of the ground set -/
+def is_circuit (x : finset α) (m : indep E) : Prop :=
+x ∉ m.indep ∧ ∀ y, y ⊂ x → y ∈ m.indep
+
+/-- proof by Mario Carneiro https://leanprover.zulipchat.com/#narrow/stream/113489-new-members/subject/finsets.2C.20decidable_mem.2C.20and.20filter/near/133708937 -/
+instance decidable_circuit (x : finset α) (m : indep E) : decidable (is_circuit x m) :=
+decidable_of_iff (x ∉ m.indep ∧ ∀ y ∈ (powerset x).erase x, y ∈ m.indep)
+begin
+  simp only [is_circuit, has_ssubset.ssubset, mem_powerset, and_imp, mem_erase],
+  refine and_congr iff.rfl (forall_congr $ λ y, _),
+  refine ⟨λ H h₁ h₂, H (mt _ h₂) h₁, λ H h₁ h₂, H h₂ $ mt _ h₁⟩,
+  { rintro rfl, refl }, { exact subset.antisymm h₂ }
+end
+
+instance decidable_circuit_subset (x : finset α) (m : indep E) :
+  decidable (∃ (y : finset α) (H : y ⊆ x), is_circuit y m) :=
+decidable_of_iff (∃ (y : finset α) (H : y ∈ powerset x), is_circuit y m) $
+  by simp only [exists_prop, mem_powerset]
+
+/- should I make this definition reducible? I don't know when to use attributes... -/
+def circuits_circ_of_indep (m : indep E) : finset (finset α) :=
+(powerset E).filter (λ S, is_circuit S m)
+
+lemma C2_of_indep (m : indep E) (x y : finset α) (hx : x ∈ circuits_circ_of_indep m)
+  (hy : y ∈ circuits_circ_of_indep m) (hxy : x ⊆ y) : x = y :=
+begin
+  simp only [circuits_circ_of_indep, is_circuit, mem_filter] at *,
+  have hnxy : ¬x ⊂ y := λ h, hx.2.1 $ hy.2.2 x h,
+  rw ←lt_iff_ssubset at hnxy, rw [←le_iff_subset, le_iff_eq_or_lt] at hxy,
+  exact or.elim hxy id (λ hxy2, false.elim $ hnxy hxy2)
+end
+
+theorem dep_iff_circuit_subset {x : finset α} (m : indep E) :
+  x ⊆ E → (x ∉ m.indep ↔ ∃ y ⊆ x, is_circuit y m) :=
+λ hxE, iff.intro (λ hxd, exists.elim (min_fun_of_ne_empty card (ne_empty_of_mem $
+    mem_filter.mpr ⟨mem_powerset.mpr $ subset.refl x, hxd⟩)) $
+  λ a ha, exists.elim ha $
+    λ ha2 hamin, exists.intro a $ have hax : a ⊆ x := mem_powerset.mp (mem_filter.mp ha2).1,
+      exists.intro hax $ by { unfold is_circuit,
+        exact ⟨(mem_filter.mp ha2).2, by { intros y hy, by_contra h,
+          exact not_le_of_lt (card_lt_card hy) (hamin y $ mem_filter.mpr ⟨mem_powerset.mpr $
+            subset.trans (le_of_lt $ lt_iff_ssubset.mpr hy) hax, h⟩) }⟩ }) $
+  λ H, exists.elim H $ λ a ha, exists.elim ha $
+    by { intros hax hacirc hxi, unfold is_circuit at hacirc,
+    exact hacirc.1 (m.indep_of_subset_indep hxi hax) }
+
+/-- Lemma 1.1.3 -/
+lemma C3_of_indep (m : indep E) (x y : finset α) (e : α) (hx : x ∈ circuits_circ_of_indep m)
+  (hy : y ∈ circuits_circ_of_indep m) (hxny : x ≠ y) (he : e ∈ x ∩ y) :
+  ∃ z, z ∈ circuits_circ_of_indep m ∧ z ⊆ erase (x ∪ y) e :=
+have hxmy : x \ y ≠ ∅ := mt subset_iff_sdiff_eq_empty.mpr $ mt (C2_of_indep m x y hx hy) hxny,
+  exists.elim (exists_mem_of_ne_empty hxmy) $
+    by { clear hxny hxmy,
+    intros a ha, simp only [circuits_circ_of_indep, mem_powerset, mem_filter, mem_sdiff, mem_inter]
+      at ha hx hy he,
+    have hxai : erase x a ∈ m.indep := by { unfold is_circuit at hx,
+      exact hx.2.2 (erase x a) (erase_ssubset ha.1) },
+    let F := (powerset (x ∪ y)).filter (λ S, erase x a ⊆ S ∧ S ∈ m.indep),
+    have hxaF : erase x a ∈ F := mem_filter.2 ⟨mem_powerset.mpr $ subset.trans (erase_subset a x) $
+      @subset_union_left _ _ x y, ⟨subset.refl _, hxai⟩⟩, clear hxai,
+    exact exists.elim (max_fun_of_ne_empty card $ ne_empty_of_mem hxaF)
+      (λ I hEI2, exists.elim hEI2 $ by { clear hxaF hEI2,
+        exact λ hIF hI,
+          have hIFindep : I ∈ m.indep := (mem_filter.mp hIF).2.2,
+          have hIdep : _ → I ∉ m.indep := (dep_iff_circuit_subset m $ mem_powerset.1 $
+            m.indep_subset_powerset_ground hIFindep).2,
+          have hIFxa : erase x a ⊆ I := (mem_filter.mp hIF).2.1,
+          have hIxuy : I ⊆ x ∪ y := mem_powerset.mp (mem_filter.mp hIF).1,
+          have haniI : a ∉ I :=
+            λ H, have hxI : x ⊆ I := (insert_erase ha.1) ▸ insert_subset.mpr ⟨H, hIFxa⟩,
+              have ∃ A ⊆ I, is_circuit A m := exists.intro x (exists.intro hxI hx.2),
+              hIdep this hIFindep,
+          have hEg : ∃ g ∈ y, g ∉ I :=
+            by { have hIdep2 := mt hIdep, simp only [not_exists, exists_prop, not_and, not_not]
+              at hIdep2,
+            have hyI0 := mt (hIdep2 hIFindep y), simp only [not_not] at hyI0,
+            have hYI : ¬y ⊆ I := hyI0 hy.2,
+            have this := exists_mem_of_ne_empty (mt subset_iff_sdiff_eq_empty.mpr hYI),
+            simp only [mem_sdiff] at this, simpa only [exists_prop] },
+          exists.elim hEg $ λ g hEg2, exists.elim hEg2 $ by { clear hEg hEg2 hIdep,
+            intros hgy hgnI,
+            have hga : g ≠ a := λ H, ha.2 (H ▸ hgy),
+            have hIag : I ⊆ erase (erase (x ∪ y) a) g :=
+              subset_iff.mpr (λ xx hxx, mem_erase.mpr ⟨λ hgg, hgnI $ hgg ▸ hxx,
+                mem_erase.mpr ⟨λ hgga, haniI $ hgga ▸ hxx, mem_of_subset hIxuy hxx⟩⟩),
+            have haxuy : a ∈ x ∪ y := mem_union_left y ha.1,
+            have hcardxye : card (erase (x ∪ y) a) = nat.pred (card (x ∪ y)) :=
+              card_erase_of_mem haxuy,
+            have hpcard : nat.pred (card (x ∪ y)) > 0 := by { rw ←hcardxye,
+              exact card_pos.mpr (ne_empty_of_mem $ mem_erase.mpr ⟨hga, mem_union_right x hgy⟩) },
+            have hcard : card I < card (erase (x ∪ y) e) :=
+              calc card I ≤ card (erase (erase (x ∪ y) a) g) : card_le_of_subset hIag
+              ... = nat.pred (nat.pred (card (x ∪ y))) : by rw [card_erase_of_mem
+                (mem_erase.mpr ⟨hga, mem_union_right x hgy⟩), hcardxye]
+              ... < card (erase (x ∪ y) e) :
+                by { rw [card_erase_of_mem (mem_union_left y he.1),
+                ←nat.succ_pred_eq_of_pos hpcard], exact nat.lt_succ_self _ },
+            clear hga hIag haxuy hcardxye hpcard he,
+            by_contra h, simp only [circuits_circ_of_indep, mem_powerset, not_exists, and_imp,
+              mem_filter, not_and] at h,
+            have hinE : erase (x ∪ y) e ⊆ E :=
+              subset.trans (erase_subset e (x ∪ y)) (union_subset hx.1 hy.1),
+            have : (∀ x_1 : finset α, x_1 ⊆ erase (x ∪ y) e → ¬is_circuit x_1 m) :=
+              λ x1 hx1, (mt $ h x1 $ subset.trans hx1 hinE) $ not_not.mpr hx1,
+            have hindep := mt (dep_iff_circuit_subset m hinE).mp,
+              simp only [not_exists, exists_prop, not_and, not_not] at hindep,
+            replace hindep : erase (x ∪ y) e ∈ m.indep := hindep this,
+            have hfinal := m.indep_exch hIFindep hindep hcard,
+            exact exists.elim hfinal (λ El ⟨hElxy, hElindep⟩,
+              have hElF : insert El I ∈ F := mem_filter.mpr ⟨mem_powerset.mpr
+                (insert_subset.mpr ⟨(mem_erase.mp (mem_sdiff.mp hElxy).1).2, hIxuy⟩),
+                ⟨subset.trans hIFxa (subset_insert El I), hElindep⟩⟩,
+              have hcardEl : card I < card (insert El I) :=
+                by { rw card_insert_of_not_mem (mem_sdiff.mp hElxy).2,
+                exact lt_add_one (card I) },
+              not_lt.mpr (hI (insert El I) hElF) hcardEl) } }) }
+
+structure circuits (E : finset α) :=
+(circuits : finset (finset α))
+(circuits_subset_powerset_ground : circuits ⊆ powerset E)
+-- (C1)
+(empty_not_mem_circuits : ∅ ∉ circuits)
+-- (C2)
+(circuits_eq_of_subset {x y} (hx : x ∈ circuits) (hy : y ∈ circuits) (hxy : x ⊆ y) : x = y)
+-- (C3)
+(circuit_elim {x y e} (hx : x ∈ circuits) (hy : y ∈ circuits) (hxy : x ≠ y) (he : e ∈ x ∩ y) :
+  ∃ z, z ∈ circuits ∧ z ⊆ erase (x ∪ y) e)
+--attribute [class] circuits
+
+instance circuits_repr [has_repr α] (E : finset α) : has_repr (circuits E) :=
+⟨λ c, has_repr.repr c.circuits⟩
+
+theorem eq_of_circ_eq : ∀ {C₁ C₂ : circuits E}, C₁.1 = C₂.1 → C₁ = C₂
+  | ⟨c₁, p₁, q₁, r₁, s₁⟩ ⟨c₂, p₂, q₂, r₂, s₂⟩ h :=
+by simpa only []
+
+def circuits_of_indep (m : indep E) : circuits E :=
+{ circuits := circuits_circ_of_indep m,
+  circuits_subset_powerset_ground := filter_subset _,
+  empty_not_mem_circuits :=
+    begin
+      simp only [circuits_circ_of_indep, is_circuit, mem_filter, not_and],
+      exact λ h h1, (h1 m.empty_mem_indep).elim
+    end,
+  circuits_eq_of_subset := C2_of_indep m,
+  circuit_elim := C3_of_indep m }
+
+/- make reducible? -/
+def indep_indep_of_circuits (C : circuits E) : finset (finset α) :=
+(powerset E).filter (λ S, ∀ c ∈ C.circuits, ¬c ⊆ S)
+
+/-- first part of Theorem 1.1.4 -/
+lemma I2_of_circuits (C : circuits E) (x y : finset α) : x ∈ indep_indep_of_circuits C → y ⊆ x →
+  y ∈ indep_indep_of_circuits C :=
+begin
+  simp only [indep_indep_of_circuits, mem_powerset, and_imp, mem_filter],
+  exact λ hxE hx hxy, ⟨subset.trans hxy hxE, λ c hc H, hx c hc $ subset.trans H hxy⟩
+end
+
+/-- second part of Theorem 1.1.4 -/
+lemma I3_of_circuits (C : circuits E) (x y : finset α) (hx : x ∈ indep_indep_of_circuits C)
+  (hy : y ∈ indep_indep_of_circuits C) (hcardxy : card x < card y)
+  : ∃ e, e ∈ y \ x ∧ insert e x ∈ indep_indep_of_circuits C :=
+begin
+  unfold indep_indep_of_circuits at ⊢,
+  simp only [indep_indep_of_circuits, mem_powerset, mem_filter] at hx hy,
+  by_contra h,
+  simp only [mem_powerset, not_exists, and_imp, mem_filter, not_and, mem_sdiff] at h,
+  let F := (powerset $ x ∪ y).filter (λ S, (∀ c ∈ C.circuits, ¬c ⊆ S) ∧ card x < card S),
+  have hyF : y ∈ F := mem_filter.mpr ⟨mem_powerset.mpr $ subset_union_right x y,
+    ⟨hy.2, hcardxy⟩⟩,
+  exact exists.elim (min_fun_of_ne_empty (λ f, card (x \ f)) $ ne_empty_of_mem hyF)
+    (λ z Hz, exists.elim Hz $ by { clear hcardxy Hz hyF,
+      intros hz hminz,
+      have hzxuy : z ⊆ x ∪ y := mem_powerset.mp (mem_filter.mp hz).1,
+      replace hz := (mem_filter.mp hz).2,
+      exact exists.elim (exists_sdiff_of_card_lt hz.2)
+        (by { intros a ha, rw mem_sdiff at ha,
+        have hxsdiffz : x \ z ≠ ∅ :=
+          by { intro H,
+          have Hxsubz : x ⊆ z := subset_iff_sdiff_eq_empty.mpr H,
+          have hay : a ∈ y := or.elim (mem_union.mp $ mem_of_subset hzxuy ha.1)
+            (λ Hax, false.elim $ ha.2 Hax) id,
+          have haindep : insert a x ∈ indep_indep_of_circuits C := I2_of_circuits C z (insert a x)
+            (by { simp only [indep_indep_of_circuits, mem_powerset, mem_filter],
+            exact ⟨subset.trans hzxuy $ union_subset hx.1 hy.1, hz.1⟩ })
+            (insert_subset.mpr ⟨ha.1, Hxsubz⟩),
+          simp only [indep_indep_of_circuits, mem_powerset, mem_filter] at haindep,
+          exact h a hay ha.2 haindep.1 haindep.2 },
+        exact exists.elim (exists_mem_of_ne_empty hxsdiffz)
+          (by { clear h ha hxsdiffz,
+          intros e he, rw mem_sdiff at he,
+          let T : α → finset α := λ f, erase (insert e z) f,
+          have hTf1 : ∀ f, f ∈ z \ x → T f ⊆ x ∪ y :=
+            by { intros f hf, rw [mem_sdiff] at hf,
+            rw [subset_iff],
+            intros gg hgg, simp only [mem_insert, mem_erase, ne.def] at hgg,
+            simp only [mem_union],
+            exact or.elim hgg.2 (λ gge, or.inl $ gge.symm ▸ he.1)
+              (λ ggz, mem_union.mp $ mem_of_subset hzxuy ggz) },
+          have hTf2 : ∀ f, f ∈ z \ x → card (x \ T f) < card (x \ z) :=
+            by { intros f hf, rw mem_sdiff at hf,
+            suffices H : x \ T f ⊂ x \ z, exact card_lt_card H,
+            by { simp only [ssubset_iff, exists_prop, mem_insert, not_forall_not, not_and,
+                            mem_sdiff, mem_erase],
+              exact exists.intro e
+                ⟨λ h_, ⟨λ hef, hf.2 $ hef ▸ he.1, or.inl rfl⟩,
+                by { rw [subset_iff],
+                  intros gg hgg,
+                  simp only [mem_insert, not_and, mem_sdiff, mem_erase, ne.def] at hgg,
+                  have ggnef : gg ≠ f := λ ggef, or.elim hgg
+                    (λ gge, (gge.symm ▸ he.2) $ ggef.substr hf.1) (λ H, (ggef.substr hf.2) H.1),
+                  have he0 := mem_sdiff.mpr he,
+                  exact or.elim hgg (λ gge, gge.symm ▸ he0)
+                  (λ H, mem_sdiff.mpr ⟨H.1, λ ggz, (H.2 ggnef) $ or.inr ggz⟩) }⟩ } },
+          have hTfindep : ∀ f, f ∈ z \ x → T f ∉ indep_indep_of_circuits C :=
+            by { intros f hf,
+            simp only [indep_indep_of_circuits, mem_powerset, mem_filter, not_and],
+            intros hTfE H,
+            have HTf1 : T f ⊆ x ∪ y := hTf1 f hf,
+            have HTf2 : card (x \ T f) < card (x \ z) := hTf2 f hf,
+            rw mem_sdiff at hf,
+            have HTfcard : card z = card (T f) :=
+              by { simp only [card_erase_of_mem (mem_insert.mpr $ or.inr hf.1),
+              card_insert_of_not_mem he.2, mem_insert, card_insert_of_not_mem, nat.pred_succ] },
+            replace HTfcard : card x < card (T f) := HTfcard ▸ hz.2,
+            have : T f ∈ F := mem_filter.mpr ⟨mem_powerset.mpr HTf1, ⟨H, HTfcard⟩⟩,
+            exact not_lt.mpr (hminz (T f) this) HTf2 },
+          have hTfC : ∀ f, f ∈ z \ x → ∃ c ∈ C.circuits, c ⊆ T f :=
+            by { intros f hf,
+            have : T f ∉ indep_indep_of_circuits C := hTfindep f hf,
+              simp only [indep_indep_of_circuits, mem_powerset, mem_filter, not_and] at this,
+            have hfc := this (subset.trans (hTf1 f hf) $ union_subset hx.1 hy.1),
+            by_contra H, simp only [not_exists, exists_prop, not_and] at H, contradiction },
+          exact exists.elim (exists_sdiff_of_card_lt hz.2) (λ g hg, exists.elim (hTfC g hg) $
+              λ Cg hCg, exists.elim hCg $
+                by { clear hCg hTf1 hTf2 hTfindep hg,
+                intros HCg1 HCg2,
+                have hCgsub : Cg ⊆ insert e z := subset.trans HCg2 (erase_subset g $ insert e z),
+                rw [subset_iff] at HCg2,
+                have HCgzx : Cg ∩ (z \ x) ≠ ∅ :=
+                  λ H, suffices Cg ⊆ x, from hx.2 Cg HCg1 this,
+                    suffices H1 : Cg ⊆ erase (insert e (x ∩ z)) g, from
+                    suffices H2 : erase (insert e (x ∩ z)) g ⊆ x, from
+                    subset.trans H1 H2,
+                    show erase (insert e (x ∩ z)) g ⊆ x, by
+                      { rw [subset_iff],
+                      intros gg hgg,
+                      simp only [mem_insert, mem_erase, mem_inter] at hgg,
+                      exact or.elim hgg.2 (λ gge, gge.symm ▸ he.1) (λ ggxggz, ggxggz.1) },
+                    show Cg ⊆ erase (insert e (x ∩ z)) g, by
+                      { rw [subset_iff],
+                      intros gg hgg,
+                      replace HCg2 : gg ∈ T g := HCg2 hgg,
+                      simp only [mem_insert, mem_erase, mem_inter] at HCg2 ⊢,
+                      split,
+                        { exact HCg2.1 },
+                        { rw eq_empty_iff_forall_not_mem at H,
+                        replace H : gg ∉ Cg ∩ (z \ x) := H gg,
+                        simp only [not_and, mem_sdiff, not_not, mem_inter] at H,
+                      exact or.elim HCg2.2 (λ gge, or.inl gge) (λ ggz, or.inr ⟨H hgg ggz, ggz⟩) } },
+                clear HCg2,
+                exact exists.elim (exists_mem_of_ne_empty HCgzx)
+                  (by { intros h0 hh0, rw [mem_inter] at hh0,
+                  exact exists.elim (hTfC h0 hh0.2)
+                    (λ Ch0 HCh0, exists.elim HCh0 $ λ hCh0circ hCh0T,
+                      have hCgneCh0 : Cg ≠ Ch0 :=
+                        λ H, have hh0Ch0 : h0 ∉ Ch0 := λ HH, (mem_erase.mp $
+                          mem_of_subset hCh0T HH).1 rfl, (H.symm ▸ hh0Ch0) hh0.1,
+                      have hCh0sub : Ch0 ⊆ insert e z :=
+                        subset.trans hCh0T (erase_subset h0 $ insert e z),
+                      have heCgCh0 : e ∈ Cg ∩ Ch0 :=
+                        by { rw mem_inter, split,
+                          { by_contra heCg, have hCgz : Cg ⊆ z :=
+                              (erase_eq_of_not_mem heCg) ▸ (subset_insert_iff.mp hCgsub),
+                            exact hz.1 Cg HCg1 hCgz },
+                          { by_contra heCh0, have hCh0z : Ch0 ⊆ z :=
+                              (erase_eq_of_not_mem heCh0) ▸ (subset_insert_iff.1 hCh0sub),
+                            exact hz.1 Ch0 hCh0circ hCh0z } },
+                      exists.elim (C.circuit_elim HCg1 hCh0circ hCgneCh0 heCgCh0) $
+                        λ CC ⟨hCCcirc, hCCCguCh0⟩,
+                          have hCCz : CC ⊆ z :=
+                            by { rw [subset_iff],
+                            intros t ht,
+                            rw [subset_iff] at hCCCguCh0,
+                            have htCguCh0 := hCCCguCh0 ht,
+                              simp only [mem_union, mem_erase] at htCguCh0,
+                            rw [subset_iff] at hCgsub hCh0sub,
+                            have orCg : t ∈ Cg → t ∈ z :=
+                              λ htCg, or.elim (mem_insert.mp $ hCgsub htCg)
+                                (λ H, false.elim $ htCguCh0.1 H) id,
+                            have orCh0 : t ∈ Ch0 → t ∈ z :=
+                              λ htCh0, or.elim (mem_insert.mp $ hCh0sub htCh0)
+                              (λ H, false.elim $ htCguCh0.1 H) id,
+                            exact or.elim htCguCh0.2 orCg orCh0 },
+                          hz.1 CC hCCcirc hCCz) }) }) }) }) })
+end
+
+def indep_of_circuits (C : circuits E) : indep E :=
+⟨indep_indep_of_circuits C,
+by simp only [indep_indep_of_circuits, filter_subset],
+mem_filter.mpr
+  ⟨empty_mem_powerset E, λ c hc H, C.empty_not_mem_circuits $ (subset_empty.mp H) ▸ hc⟩,
+I2_of_circuits C,
+I3_of_circuits C⟩
+
+-- instance circ_indep : has_coe (circuits E) (indep E) := ⟨indep_of_circuits⟩
+-- instance indep_circ : has_coe (indep E) (circuits E) := ⟨circuits_of_indep⟩
+
+/-- third part of Theorem 1.1.4 -/
+theorem circ_indep_circ : ∀ C : circuits E, C = circuits_of_indep (indep_of_circuits C)
+  | ⟨c₁, p₁, q₁, r₁, s₁⟩ :=
+by { simp only [indep_of_circuits, circuits_of_indep, indep_indep_of_circuits,
+  circuits_circ_of_indep, is_circuit, ext, mem_filter, mem_powerset, and_imp, not_and],
+exact λ c, iff.intro
+  (λ hc : c ∈ c₁, have ce : c ⊆ E := mem_powerset.mp (mem_of_subset p₁ hc),
+  ⟨ce, ⟨λ _ H, (H c hc) $ subset.refl c, λ f hf,
+    ⟨subset.trans (le_of_lt $ lt_iff_ssubset.mpr hf) ce,
+    λ g hg H, have Hc : g < c := lt_of_le_of_lt (le_iff_subset.mpr H) $ lt_iff_ssubset.mpr hf,
+      have r : g = c := r₁ hg hc $ le_of_lt Hc, (not_le_of_lt Hc) $ le_of_eq r.symm⟩⟩⟩) $
+  λ hc, have ∃ c_1 ∈ c₁, c_1 ⊆ c := by { have := not_forall.mp (hc.2.1 hc.1),
+    simpa only [exists_prop, not_forall_not] },
+  exists.elim this $ λ c' H, exists.elim H $ by { intros hc' hcc',
+    by_cases h : c = c', { exact h.symm ▸ hc' },
+      { have hc'lt : c' ⊂ c := lt_of_le_of_ne (le_iff_subset.mpr hcc') (ne.symm h),
+        have : c' ∉ c₁ := mt ((hc.2.2 c' hc'lt).2 c') (not_not.mpr $ subset.refl c'),
+        exact false.elim (this hc') } } }
+
+theorem indep_circ_indep (M : indep E) : M = indep_of_circuits (circuits_of_indep M) :=
+suffices M.indep = (indep_of_circuits $ circuits_of_indep M).indep, from eq_of_indep_eq this,
+begin
+  simp only [circuits_of_indep, indep_of_circuits, circuits_circ_of_indep, indep_indep_of_circuits,
+    ext, mem_powerset, and_imp, mem_filter],
+  intro I,
+  have hI : I ∈ M.indep → I ⊆ E := λ H, mem_powerset.mp $
+    mem_of_subset (M.indep_subset_powerset_ground) H,
+  rw [←and_iff_right_of_imp hI, and_congr_right],
+  intro hIE, have := not_iff_not_of_iff (dep_iff_circuit_subset M hIE),
+  simp only [not_exists, exists_prop, not_and, not_not] at this,
+  rw [this, forall_congr],
+  exact λ a, ⟨λ h h₁ h₂ h₃, (h h₃) h₂, λ h h₁ h₂, h (subset.trans h₁ hIE) h₂ h₁⟩
+end
+
+/-- Proposition 1.1.6 -/
+theorem existsu_circuit_of_dep_of_insert_indep {I : finset α} {e : α} {m : indep E}
+  (hI : I ∈ m.indep) (he : e ∈ E) (hIe : insert e I ∉ m.indep) :
+  ∃ c, c ∈ circuits_circ_of_indep m ∧ c ⊆ insert e I ∧ e ∈ c ∧
+  ∀ c' ∈ circuits_circ_of_indep m, c' ⊆ insert e I ∧ e ∈ c → c' = c :=
+by { simp only [circuits_circ_of_indep, mem_powerset, and_imp, mem_filter],
+exact have hIE : I ⊆ E, from mem_powerset.mp (mem_of_subset m.indep_subset_powerset_ground hI),
+have hIeE : insert e I ⊆ E, from insert_subset.mpr ⟨he, hIE⟩,
+have hc : _, from (dep_iff_circuit_subset m hIeE).mp hIe,
+exists.elim hc $ λ c hEc, exists.elim hEc $ λ hceI hccirc,
+  have hcE : c ⊆ E := subset.trans hceI hIeE,
+  have hecirc : ∀ c' ⊆ insert e I, is_circuit c' m → e ∈ c' :=
+    by { intros c' hc'eI hc'circ,
+    have h₁ := subset_insert_iff.mp hc'eI,
+    by_contra h,
+    have h₂ := (erase_eq_of_not_mem h).symm,
+    have h₃ : c' ⊆ I := calc
+    c' = erase c' e : h₂
+    ... ⊆ I : h₁,
+    exact (dep_iff_circuit_subset m hIE).mpr (exists.intro c' $ exists.intro h₃ $ hc'circ) hI },
+  have hec : e ∈ c := hecirc c hceI hccirc,
+  exists.intro c $ by { exact ⟨⟨hcE, hccirc⟩, ⟨hceI,⟨hec, by { intros c' hc'E hc'circ hc'eI _,
+    have hec' : e ∈ c' := hecirc c' hc'eI hc'circ,
+    have hcuc'eI : erase (c ∪ c') e ⊆ I := by {
+      simp only [subset_iff, and_imp, mem_union, mem_insert, mem_erase, ne.def] at hceI hc'eI ⊢,
+      exact λ a hane ha, or.elim ha (λ H, or.elim (hceI H) (λ H, false.elim $ hane H) id)
+        (λ H, or.elim (hc'eI H) (λ H, false.elim $ hane H) id) },
+    have : erase (c ∪ c') e ∈ m.indep := m.indep_of_subset_indep hI hcuc'eI,
+    by_contra h,
+    have C3 := C3_of_indep m c c' e,
+      simp only [circuits_circ_of_indep, mem_powerset, and_imp,
+        filter_congr_decidable, mem_filter, mem_inter] at C3,
+    exact exists.elim (C3 hcE hccirc hc'E hc'circ (ne.symm h) hec hec')
+      (λ c₀ hc₀, (dep_iff_circuit_subset m hIE).mpr (exists.intro c₀ $ exists.intro
+        (subset.trans hc₀.2 hcuc'eI) hc₀.1.2) hI) }⟩⟩⟩ } }
+
+section encodable
+variable [encodable α]
+
+def circuit_of_dep_of_insert_indep {I : finset α} {e : α} {m : indep E}
+  (hI : I ∈ m.indep) (he : e ∈ E) (hIe : insert e I ∉ m.indep) : finset α :=
+encodable.choose (existsu_circuit_of_dep_of_insert_indep hI he hIe)
+
+local notation `cdii` := circuit_of_dep_of_insert_indep
+
+def circuit_of_dep_of_insert_indep_spec {I : finset α} {e : α} {m : indep E}
+  (hI : I ∈ m.indep) (he : e ∈ E) (hIe : insert e I ∉ m.indep) :
+  cdii hI he hIe ∈ circuits_circ_of_indep m ∧ cdii hI he hIe ⊆ insert e I ∧
+  e ∈ cdii hI he hIe ∧ ∀ (c' : finset α), c' ∈ circuits_circ_of_indep m →
+  c' ⊆ insert e I ∧ e ∈ cdii hI he hIe → c' = cdii hI he hIe  :=
+encodable.choose_spec (existsu_circuit_of_dep_of_insert_indep hI he hIe)
+
+end encodable
+
+-- § 1.2
+
+def is_basis (x : finset α) (m : indep E) : Prop :=
+x ∈ m.indep ∧ (∀ y ⊆ E, x ⊂ y → y ∉ m.indep)
+
+instance decidable_basis (x : finset α) (m : indep E) : decidable (is_basis x m) :=
+decidable_of_iff (x ∈ m.indep ∧ (∀ y ∈ powerset E, x ⊂ y → y ∉ m.indep)) $
+  by simp only [is_basis, iff_self, finset.mem_powerset]
+
+/-- Lemma 1.2.1 -/
+theorem bases_of_indep_card_eq {x y : finset α} {m : indep E} : is_basis x m → is_basis y m →
+  card x = card y :=
+begin
+  intros hx hy,
+  by_contra heq,
+  wlog h : card x < card y using [x y, y x],
+  exact lt_or_gt_of_ne heq,
+  unfold is_basis at hx hy,
+  exact exists.elim (m.indep_exch hx.1 hy.1 h) (λ e ⟨he1, he2⟩,
+    have hins : insert e x ⊆ E := mem_powerset.mp
+      (mem_of_subset (m.indep_subset_powerset_ground) he2),
+    have hememx : e ∉ x := (mem_sdiff.mp he1).2,
+    (hx.2 (insert e x) hins $ ssubset_insert hememx) he2)
+end
+
+theorem exists_basis_containing_indep {I : finset α} {m : indep E} (h : I ∈ m.indep) :
+  ∃ B : finset α, I ⊆ B ∧ is_basis B m :=
+let F := (m.indep).filter (λ a, I ⊆ a) in
+have FI : I ∈ F := mem_filter.mpr ⟨h, subset.refl I⟩,
+exists.elim (max_fun_of_ne_empty card $ ne_empty_of_mem FI) $
+  λ B HB, exists.elim HB $ by { clear HB, intros HBF Hg, rw mem_filter at HBF,
+    have hBB : is_basis B m := ⟨HBF.1, λ y hy hBy hyI,
+      have hxsy : I ⊆ y := le_of_lt $ lt_of_le_of_lt (le_iff_subset.mpr HBF.2) $
+        lt_iff_ssubset.mpr hBy,
+      have hyF : y ∈ F := mem_filter.mpr ⟨hyI, hxsy⟩,
+      lt_irrefl (card B) $ lt_of_lt_of_le (card_lt_card hBy) $ Hg y hyF⟩,
+    exact exists.intro B ⟨HBF.2, hBB⟩ }
+
+section encodable
+
+def basis_containing_indep [encodable α] {I : finset α} {m : indep E} (h : I ∈ m.indep) :
+  finset α :=
+encodable.choose $ exists_basis_containing_indep h
+
+local notation `bci` := basis_containing_indep
+
+def basis_containing_indep_spec [encodable α] {I : finset α} {m : indep E} (h : I ∈ m.indep) :
+  I ⊆ bci h ∧ is_basis (bci h) m :=
+encodable.choose_spec $ exists_basis_containing_indep h
+
+end encodable
+
+theorem dep_of_card_gt_card_basis {x B : finset α} {m : indep E} (hB : is_basis B m)
+  (hcard : card B < card x) : x ∉ m.indep :=
+λ hxI, exists.elim (exists_basis_containing_indep hxI) $ λ B' hB',
+  ne_of_lt (lt_of_lt_of_le hcard $ card_le_of_subset hB'.1) $ bases_of_indep_card_eq hB hB'.2
+
+theorem card_of_indep_le_card_basis {x B : finset α} {m : indep E} (hx : x ∈ m.indep)
+  (hB : is_basis B m) : card x ≤ card B :=
+by { by_contra h, exact dep_of_card_gt_card_basis hB (lt_of_not_ge h) hx }
+
+structure bases (E : finset α) :=
+(bases : finset (finset α))
+(bases_subset_powerset_ground : bases ⊆ powerset E)
+-- (B1)
+(bases_not_empty : bases ≠ ∅)
+-- (B2)
+(basis_exch {x y e} (hx : x ∈ bases) (hy : y ∈ bases) (he : e ∈ x \ y)
+    : ∃ a, a ∈ y \ x ∧ insert a (erase x e) ∈ bases)
+--attribute [class] bases
+
+instance bases_repr [has_repr α] (E : finset α) : has_repr (bases E) :=
+⟨λ b, has_repr.repr b.bases⟩
+
+theorem eq_of_base_eq : ∀ {B₁ B₂ : bases E}, B₁.1 = B₂.1 → B₁ = B₂
+  | ⟨b₁, p₁, q₁, r₁⟩ ⟨b₂, p₂, q₂, r₂⟩ h :=
+by simpa only []
+
+def bases_bases_of_indep (m : indep E) : finset (finset α) :=
+(powerset E).filter (λ S, is_basis S m)
+
+lemma B1_of_indep (m : indep E) : bases_bases_of_indep m ≠ ∅ :=
+by { simp only [is_basis, bases_bases_of_indep, ext, ne.def, mem_filter, mem_powerset,
+    not_mem_empty, not_and, iff_false],
+  exact λ h, exists.elim (max_fun_of_ne_empty card $ ne_empty_of_mem m.empty_mem_indep)
+  (λ a ha, exists.elim ha $ λ ha1 hg, (h a (mem_powerset.mp $
+    mem_of_subset m.indep_subset_powerset_ground ha1)
+  ha1) $ λ F _ Fcontainsa Findep, not_le_of_lt (card_lt_card Fcontainsa) $ hg F Findep) }
+
+/- Lemma 1.2.2 -/
+lemma B2_of_indep (m : indep E) : ∀ (x y : finset α) (e : α), x ∈ bases_bases_of_indep m →
+  y ∈ bases_bases_of_indep m → e ∈ x \ y →
+  ∃ a, a ∈ y \ x ∧ insert a (erase x e) ∈ bases_bases_of_indep m :=
+by { simp only [is_basis, bases_bases_of_indep, filter_and, mem_filter, mem_sdiff,
+  mem_powerset, and_imp],
+exact λ x y e hxE hxI hx hyE hyI hy hex hey,
+  have hxr : erase x e ∈ m.indep := m.indep_of_subset_indep hxI $ erase_subset e x,
+  have hxB : is_basis x m := ⟨hxI, hx⟩, have hyB : is_basis y m := ⟨hyI, hy⟩,
+  have hcard : card (erase x e) < card y := calc
+    card (erase x e) < card x : card_lt_card $ erase_ssubset hex
+    ... = card y : bases_of_indep_card_eq hxB hyB,
+  exists.elim (m.indep_exch hxr hyI hcard) $
+    by { clear hxr hyI hcard hyB, intros a ha,
+      have ha1 := mem_sdiff.mp ha.1,
+      have hae : a ≠ e := λ hae, hey $ hae ▸ ha1.1,
+      have hax : a ∉ x := by { simp only [not_and, mem_erase, ne.def] at ha1, exact ha1.2 hae },
+      have hcx : card x > 0 := card_pos.mpr (ne_empty_of_mem hex),
+      have hayycard : card (insert a $ erase x e) = card x := calc
+        card (insert a $ erase x e) = nat.pred (card x) + 1 : by rw [card_insert_of_not_mem ha1.2,
+            card_erase_of_mem hex]
+        ... = card x : nat.succ_pred_eq_of_pos hcx,
+      exact exists.intro a ⟨⟨ha1.1, hax⟩, mem_powerset.mp $
+        mem_of_subset m.indep_subset_powerset_ground ha.2, ha.2,
+        λ _ _ hayy, dep_of_card_gt_card_basis hxB $ hayycard ▸ (card_lt_card hayy)⟩ } }
+
+def bases_of_indep (m : indep E) : bases E :=
+⟨bases_bases_of_indep m,
+filter_subset _,
+B1_of_indep m,
+B2_of_indep m⟩
+
+/-- Lemma 1.2.4 -/
+theorem bases_card_eq {x y : finset α} {b : bases E} (hx : x ∈ b.bases) (hy : y ∈ b.bases) :
+  card x = card y :=
+begin
+  by_contra heq,
+  wlog h : card y < card x using [x y, y x],
+  exact lt_or_gt_of_ne (ne.symm heq), clear heq,
+  let F : finset (finset α × finset α) := (finset.product b.bases b.bases).filter
+    (λ e : finset α × finset α, card e.1 < card e.2),
+  have hyx : (y, x) ∈ F := mem_filter.mpr ⟨mem_product.mpr ⟨hy, hx⟩, h⟩, clear hy hx,
+  exact exists.elim (min_fun_of_ne_empty (λ f : finset α × finset α, card (f.2 \ f.1)) $
+      ne_empty_of_mem hyx)
+    (λ a ha, exists.elim ha $ by { clear hyx ha,
+      intros haF Ha, replace haF := mem_filter.mp haF,
+      have hab : a.1 ∈ b.bases ∧ a.2 ∈ b.bases := mem_product.mp haF.1,
+      exact exists.elim (exists_sdiff_of_card_lt haF.2)
+        (λ e he, exists.elim (b.basis_exch hab.2 hab.1 he) $ λ aa ⟨haa1, haa2⟩,
+          by { rw mem_sdiff at haa1,
+          let a2 : finset α := insert aa (erase a.2 e),
+          have haani : aa ∉ erase a.2 e := λ h, haa1.2 (mem_erase.mp h).2,
+          have hea2 : e ∈ a.2 := (mem_sdiff.mp he).1,
+          have hpos : 0 < card a.2 := card_pos.mpr (ne_empty_of_mem hea2),
+          have hcarda2 : card a.1 < card a2 := by { rw [card_insert_of_not_mem haani,
+            card_erase_of_mem hea2, ←nat.succ_eq_add_one, nat.succ_pred_eq_of_pos hpos],
+            exact haF.2 }, clear haani hpos,
+          have : e ∉ a2 := λ hh, or.elim (mem_insert.mp hh)
+            (λ h4, haa1.2 $ h4 ▸ hea2) $ λ h5, (mem_erase.mp h5).1 rfl,
+          have hcard : card (a2 \ a.1) < card (a.2 \ a.1) :=
+            suffices a2 \ a.1 ⊂ a.2 \ a.1, from card_lt_card this,
+            by { rw ssubset_iff,
+            exact exists.intro e ⟨λ h0, this (mem_sdiff.mp h0).1,
+              by { rw subset_iff,
+              intros A hA, rw mem_insert at hA,
+              exact or.elim hA (λ hA1, hA1.symm ▸ he)
+                (by { intro hA2, rw [mem_sdiff, mem_insert] at hA2,
+                exact mem_sdiff.mpr ⟨or.elim hA2.1 (λ h6, false.elim $ hA2.2 $ h6.symm ▸ haa1.1) $
+                  λ h7, (mem_erase.mp h7).2, hA2.2⟩ }) }⟩ },
+          have ha2F : (a.1, a2) ∈ F := mem_filter.mpr ⟨mem_product.mpr ⟨hab.1, haa2⟩, hcarda2⟩,
+          exact not_le_of_lt hcard (Ha (a.1, a2) ha2F) }) })
+end
+
+def indep_indep_of_bases (b : bases E) : finset (finset α) :=
+(powerset E).filter (λ x, ∃ a ∈ b.bases, x ⊆ a)
+
+/-- first part of Theorem 1.2.3 -/
+def indep_of_bases (b : bases E) : indep E :=
+⟨indep_indep_of_bases b,
+filter_subset _,
+mem_filter.mpr ⟨empty_mem_powerset E, exists.elim (exists_mem_of_ne_empty b.bases_not_empty) $
+    λ a ha, exists.intro a $ exists.intro ha $ empty_subset a⟩,
+begin
+  intros x y hx hxy, simp only [indep_indep_of_bases, mem_powerset, filter_congr_decidable,
+    exists_prop, mem_filter] at hx ⊢,
+  exact ⟨subset.trans hxy hx.1,
+    exists.elim hx.2 $ λ a ha, exists.intro a ⟨ha.1, subset.trans hxy ha.2⟩⟩
+end,
+begin
+  intros x y hx hy hcard, unfold indep_indep_of_bases at *,
+  let F := (b.bases).filter (λ S, S ⊆ y),
+  by_contra h, simp only [mem_powerset, not_exists, and_imp, filter_congr_decidable,
+    exists_prop, mem_filter, not_and, mem_sdiff] at hx hy h,
+  exact exists.elim hx.2 (λ b1 hb1, exists.elim hy.2 $ λ b2 hb2, exists.elim
+    (min_fun_of_ne_empty (λ f, card (f \ (y ∪ b1))) $ ne_empty_of_mem $ mem_filter.mpr hb2) $
+    λ B2 hEB2, exists.elim hEB2 $ by { clear hb2 b2 hEB2,
+      intros hB2filt hB2min, replace hB2filt : B2 ∈ b.bases ∧ y ⊆ B2 := mem_filter.mp hB2filt,
+      have hysdiff : y \ b1 = y \ x := by { simp only [ext, mem_sdiff],
+        exact λ gg, ⟨λ hgg, ⟨hgg.1, λ hggnx, hgg.2 $ mem_of_subset hb1.2 hggnx⟩,
+          λ hgg, ⟨hgg.1, λ ggb1, h gg hgg.1 hgg.2 (insert_subset.mpr
+          ⟨mem_of_subset hy.1 hgg.1, hx.1⟩) b1 hb1.1 $ insert_subset.mpr ⟨ggb1, hb1.2⟩⟩⟩ },
+      have hB2yub1: B2 \ (y ∪ b1) = ∅ := by { by_contra H,
+        exact exists.elim (exists_mem_of_ne_empty H) (by { clear H,
+          intros X hX, simp only [not_or_distrib, mem_union, mem_sdiff] at hX,
+          have hXB2b1 : X ∈ B2 \ b1 := by { rw mem_sdiff, exact ⟨hX.1, hX.2.2⟩ },
+          exact exists.elim (b.basis_exch hB2filt.1 hb1.1 hXB2b1)
+            (λ Y ⟨hYb1B2, hYbases⟩, by { rw mem_sdiff at hYb1B2 hXB2b1,
+              have hssubY : insert Y (erase B2 X) \ (y ∪ b1) ⊂  B2 \ (y ∪ b1) :=
+                by { rw [ssubset_iff],
+                exact exists.intro X (by {
+                  simp only [subset_iff, not_or_distrib, mem_union, mem_insert, not_and, mem_sdiff,
+                    not_not, mem_erase, not_true, or_false, ne.def, false_and, or_false,
+                    eq_self_iff_true],
+                  exact ⟨λ hXY, false.elim $ hYb1B2.2 (hXY ▸ hXB2b1.1),
+                  λ gg hgg, or.elim hgg (λ ggx, ggx.symm ▸ hX) $ λ ggor2, or.elim ggor2.1
+                    (λ ggY, false.elim $ (ggY ▸ ggor2.2.2) hYb1B2.1) $
+                      λ ggXB2, ⟨ggXB2.2, ggor2.2⟩⟩ }) },
+              replace hssubY := card_lt_card hssubY,
+              have hysubY : y ⊆ insert Y (erase B2 X) := by {
+                simp only [subset_iff, mem_insert, mem_erase, ne.def],
+                exact λ gg hgg, or.inr ⟨λ ggx, hX.2.1 $ ggx ▸ hgg, mem_of_subset hB2filt.2 hgg⟩ },
+              exact not_lt_of_le (hB2min (insert Y $ erase B2 X) $ mem_filter.mpr
+                  ⟨hYbases, hysubY⟩) hssubY }) }) }, clear hB2min,
+      rw [←subset_iff_sdiff_eq_empty, subset_iff] at hB2yub1, simp only [mem_union] at hB2yub1,
+      have hB2b1y : B2 \ b1 = y \ b1 := by { simp only [ext, mem_sdiff],
+        exact λ gg, ⟨λ hgg, ⟨or.elim (hB2yub1 hgg.1) id $ λ hb1, false.elim $ hgg.2 hb1, hgg.2⟩,
+            λ hgg, ⟨mem_of_subset hB2filt.2 hgg.1, hgg.2⟩⟩ },
+      rw [hysdiff] at hB2b1y, clear hysdiff,
+      have hb1xuB2 : b1 \ (x ∪ B2) = ∅ := by { by_contra H,
+        exact exists.elim (exists_mem_of_ne_empty H)
+          (by { intros X hX, simp only [not_or_distrib, mem_union, mem_sdiff] at hX,
+          exact exists.elim (b.basis_exch hb1.1 hB2filt.1 $ mem_sdiff.mpr ⟨hX.1, hX.2.2⟩)
+            (by { intros Y hY, rw mem_sdiff at hY,
+            have hYyx : Y ∈ y ∧ Y ∉ x := mem_sdiff.mp (hB2b1y ▸ (mem_sdiff.mpr hY.1)),
+            have hxYsub : insert Y x ⊆ insert Y (erase b1 X) := by {
+              simp only [subset_iff, mem_insert, mem_erase, ne.def],
+              exact λ gg hgg, or.elim hgg (λ ggY, or.inl ggY) $ λ ggx, or.inr ⟨λ ggX, hX.2.1 $
+                ggX ▸ ggx, mem_of_subset hb1.2 ggx⟩ },
+            have : insert Y x ⊆ E := insert_subset.mpr ⟨mem_of_subset hy.1 hYyx.1, hx.1⟩,
+            exact h Y hYyx.1 hYyx.2 this (insert Y $ erase b1 X) hY.2 hxYsub }) }) },
+      clear h hx hy,
+      rw [←subset_iff_sdiff_eq_empty, subset_iff] at hb1xuB2, simp only [mem_union] at hb1xuB2,
+      have hb1B2 : b1 \ B2 = x \ B2 := by { simp only [ext, mem_sdiff],
+        exact λ gg, ⟨λ hgg, ⟨or.elim (hb1xuB2 hgg.1) id $ λ ggB2, false.elim $ hgg.2 ggB2, hgg.2⟩,
+            λ hgg, ⟨mem_of_subset hb1.2 hgg.1, hgg.2⟩⟩ }, clear hb1xuB2,
+      replace hb1B2 : b1 \ B2 ⊆ x \ y := hb1B2.symm ▸ (sdiff_subset_sdiff (subset.refl x)
+          hB2filt.2),
+      have hcardeq : card b1 = card B2 := bases_card_eq hb1.1 hB2filt.1,
+      have hcardb1B2 : card (b1 \ B2) = card (B2 \ b1) := calc
+        card (b1 \ B2) = card b1 - card (b1 ∩ B2) : card_sdiff_eq b1 B2
+        ... = card B2 - card (B2 ∩ b1) : by rw [hcardeq, inter_comm]
+        ... = card (B2 \ b1) : by rw ←card_sdiff_eq B2 b1,
+      have hcardcontra0 : card (y \ x) ≤ card (x \ y) := calc
+        card (y \ x) = card (B2 \ b1) : by rw hB2b1y
+        ... = card (b1 \ B2) : by rw hcardb1B2
+        ... ≤ card (x \ y) : card_le_of_subset hb1B2,
+      rw [card_sdiff_eq y x, card_sdiff_eq x y, inter_comm] at hcardcontra0,
+      have hcardcontra : card y ≤ card x := nat.le_of_le_of_sub_le_sub_right
+          (card_le_of_subset $ @inter_subset_left _ _ x y) hcardcontra0,
+      exact not_lt_of_le hcardcontra hcard })
+end⟩
+
+instance base_indep : has_coe (bases E) (indep E) := ⟨indep_of_bases⟩
+instance indep_base : has_coe (indep E) (bases E) := ⟨bases_of_indep⟩
+
+/-- second part of Theorem 1.2.3 -/
+theorem base_indep_base (B : bases E) : B = bases_of_indep (indep_of_bases B) :=
+suffices B.bases = (bases_of_indep $ indep_of_bases B).bases, from eq_of_base_eq this,
+by { simp only [indep_of_bases, bases_of_indep, indep_indep_of_bases, is_basis,
+  ext, bases_bases_of_indep, mem_filter, mem_powerset, not_and, not_exists, exists_prop],
+exact λ b, iff.intro
+  (λ hb, have hB : b ⊆ E := mem_powerset.mp (mem_of_subset B.bases_subset_powerset_ground hb),
+    ⟨hB, ⟨⟨hB, exists.intro b ⟨hb, subset.refl b⟩⟩, λ b' _ hbb' _ _ hx H,
+    (ne_of_lt $ lt_of_lt_of_le (card_lt_card hbb') $ card_le_of_subset H) $ bases_card_eq hb hx⟩⟩) $
+  λ hb, exists.elim hb.2.1.2 $ λ a ha, have a ⊆ E := mem_powerset.mp $
+    B.bases_subset_powerset_ground ha.1, by { by_cases h : a = b,
+      { exact h ▸ ha.1 },
+      { have hba : b ⊂ a := lt_iff_ssubset.mp (lt_of_le_of_ne (le_iff_subset.mpr ha.2) $ ne.symm h),
+        exact false.elim (hb.2.2 a this hba this a ha.1 $ subset.refl a) } } }
+
+theorem indep_base_indep (M : indep E) : M = indep_of_bases (bases_of_indep M) :=
+suffices M.indep = (indep_of_bases $ bases_of_indep M).indep, from eq_of_indep_eq this,
+by { simp only [indep_of_bases, bases_of_indep, indep_indep_of_bases, is_basis,
+  ext, bases_bases_of_indep, mem_filter, mem_powerset, exists_prop],
+  exact λ I, iff.intro (λ hI, ⟨mem_powerset.mp $ mem_of_subset M.indep_subset_powerset_ground hI,
+  exists.elim (exists_basis_containing_indep hI) $ λ B hB, by { unfold is_basis at hB,
+    exact exists.intro B ⟨⟨mem_powerset.1 $ mem_of_subset M.indep_subset_powerset_ground hB.2.1,
+      hB.2⟩, hB.1⟩ }⟩) $ λ hI, exists.elim hI.2 $ λ B hB, M.indep_of_subset_indep hB.1.2.1 hB.2 }
+
+/-- Corollary 1.2.6 -/
+theorem existsu_fund_circ_of_basis {m : indep E} {B : finset α} (hB : is_basis B m) {e : α}
+  (he : e ∈ E \ B) : ∃ C, C ∈ circuits_circ_of_indep m ∧ C ⊆ insert e B ∧
+  ∀ C' ∈ circuits_circ_of_indep m, C' ⊆ insert e B → C' = C :=
+begin
+  unfold is_basis at hB, rw mem_sdiff at he,
+  have : insert e B ∉ m.indep := hB.2 (insert e B) (insert_subset.mpr ⟨he.1,
+    mem_powerset.mp $ mem_of_subset m.indep_subset_powerset_ground hB.1⟩) (ssubset_insert he.2),
+  replace := existsu_circuit_of_dep_of_insert_indep hB.1 he.1 this,
+  exact exists.elim this (λ C ⟨hCcirc, HC⟩, exists.intro C $
+    ⟨hCcirc, ⟨HC.1, λ C' hC'circ hC', HC.2.2 C' hC'circ ⟨hC', HC.2.1⟩⟩⟩)
+end
+
+section encodable
+
+def fund_circ_of_basis [encodable α] {m : indep E} {B : finset α} (hB : is_basis B m) {e : α}
+  (he : e ∈ E \ B) : finset α :=
+encodable.choose (existsu_fund_circ_of_basis hB he)
+
+def fund_circ_of_basis_spec [encodable α] {m : indep E} {B : finset α} (hB : is_basis B m) {e : α}
+  (he : e ∈ E \ B) : fund_circ_of_basis hB he ∈ circuits_circ_of_indep m ∧
+  fund_circ_of_basis hB he  ⊆ insert e B ∧ ∀ C' ∈ circuits_circ_of_indep m, C' ⊆ insert e B →
+  C' = fund_circ_of_basis hB he :=
+encodable.choose_spec (existsu_fund_circ_of_basis hB he)
+
+end encodable
+
+-- § 1.3
+
+def indep_of_restriction (m : indep E) {X : finset α} (hXE : X ⊆ E) : finset (finset α) :=
+(m.indep).filter (λ I, I ⊆ X)
+
+def restriction (m : indep E) {X : finset α} (hXE : X ⊆ E) : indep X :=
+⟨indep_of_restriction m hXE,
+by simp only [indep_of_restriction, subset_iff, and_imp, imp_self,
+  mem_powerset, mem_filter, forall_true_iff],
+by simp only [indep_of_restriction, m.empty_mem_indep, empty_subset, and_self, mem_filter],
+by { unfold indep_of_restriction, exact λ x y hx hy, mem_filter.mpr
+  ⟨m.indep_of_subset_indep (mem_filter.mp hx).1 hy, subset.trans hy (mem_filter.mp hx).2⟩ },
+by { unfold indep_of_restriction, exact λ x y hx hy hcard,
+  have hxm : x ∈ m.indep := (mem_filter.mp hx).1, have hym : y ∈ m.indep := (mem_filter.mp hy).1,
+  have hxX : x ⊆ X := (mem_filter.mp hx).2, have hyX : y ⊆ X := (mem_filter.mp hy).2,
+  have H : _ := m.indep_exch hxm hym hcard,
+  let ⟨e, H, h₁⟩ := H in
+    ⟨e, H, mem_filter.mpr ⟨h₁, insert_subset.mpr ⟨mem_of_subset hyX (mem_sdiff.mp H).1, hxX⟩⟩⟩ }⟩
+
+def deletion (m : indep E) {X : finset α} (hXE : X ⊆ E) : indep (E \ X) :=
+restriction m $ sdiff_subset E X
+
+notation m `¦` hxe := restriction m hxe
+notation m `\` hxe := deletion m hxe
+
+lemma restriction_subset_restriction {X : finset α} (hX : X ⊆ E) (m : indep E) :
+  (m ¦ hX).indep ⊆ m.indep :=
+by { simp only [restriction, indep_of_restriction, subset_iff, and_imp,
+  filter_congr_decidable, mem_filter],
+  exact λ _ hX'I _, hX'I }
+
+lemma restriction_trans {X Y : finset α} (hXY : X ⊆ Y) (hY : Y ⊆ E) (m : indep E) :
+  (m ¦ subset.trans hXY hY) = ((m ¦ hY) ¦ hXY) :=
+by { simp only [restriction, indep_of_restriction, ext, mem_filter],
+  exact λ I, iff.intro (λ h, ⟨⟨h.1, subset.trans h.2 hXY⟩, h.2⟩) $ λ h, ⟨h.1.1, h.2⟩ }
+
+lemma subset_restriction_indep {X Y : finset α} {m : indep E} (hX : X ∈ m.indep) (hXY : X ⊆ Y)
+  (hY : Y ⊆ E) : X ∈ (m ¦ hY).indep :=
+by { simp only [restriction, indep_of_restriction, mem_filter], exact ⟨hX, hXY⟩ }
+
+/-def spans (X : finset α) {Y : finset α} (hY : Y ⊆ E) (m : indep E) : Prop :=
+X ∈ bases_bases_of_indep (m ¦ hY)-/
+
+lemma exists_basis_of_subset {X : finset α} (hXE : X ⊆ E) (m : indep E) :
+  ∃ B, B ∈ bases_bases_of_indep (m ¦ hXE) :=
+exists_mem_of_ne_empty $ B1_of_indep (m ¦ hXE)
+
+/-lemma inter_of_span_of_subset_span {m : indep E} {X Y bX bY : finset α} {hXE : X ⊆ E}
+  (hbX : spans bX hXE m) {hYE : Y ⊆ E} (hbY : spans bY hYE m) (hbXbY : bX ⊆ bY) : bY ∩ X = bX :=
+sorry-/
+
+section encodable
+variable [encodable α]
+
+def basis_of_subset {X : finset α} (hXE : X ⊆ E) (m : indep E) : finset α :=
+encodable.choose $ exists_basis_of_subset hXE m
+
+def basis_of_subset_spec {X : finset α} (hXE : X ⊆ E) (m : indep E) :
+  basis_of_subset hXE m ∈ bases_bases_of_indep (m ¦ hXE) :=
+encodable.choose_spec $ exists_basis_of_subset hXE m
+
+notation `𝔹` := basis_of_subset
+notation `𝔹ₛ` := basis_of_subset_spec
+
+def rank_of_subset {X : finset α} (hXE : X ⊆ E) (m : indep E) : ℕ :=
+card $ 𝔹 hXE m
+
+notation `𝓇` := rank_of_subset
+
+lemma R2_of_indep (m : indep E) {X Y : finset α} (hXY : X ⊆ Y) (hYE : Y ⊆ E) :
+  𝓇 (subset.trans hXY hYE) m ≤ 𝓇 hYE m :=
+let hXE : X ⊆ E := subset.trans hXY hYE in let bX := 𝔹 hXE m in let bY := 𝔹 hYE m in
+have bXs : _ := 𝔹ₛ hXE m, have bYs : _ := 𝔹ₛ hYE m,
+by { simp only [bases_bases_of_indep, mem_powerset, filter_congr_decidable, mem_filter] at bXs bYs,
+  unfold rank_of_subset,
+  have hBX : bX ∈ (m ¦ hYE).indep := mem_of_subset (restriction_subset_restriction hXY (m ¦ hYE))
+    ((restriction_trans hXY hYE m) ▸ bXs.2.1),
+  exact exists.elim (exists_basis_containing_indep hBX) (λ B hB, calc
+    card bX ≤ card B : card_le_of_subset hB.1
+    ... = card bY : bases_of_indep_card_eq hB.2 bYs.2) }
+
+/-- Lemma 1.3.1 -/
+lemma R3_of_indep (m : indep E) {X Y : finset α} (hX : X ⊆ E) (hY : Y ⊆ E) :
+  𝓇 (union_subset hX hY) m +
+  𝓇 (subset.trans (@inter_subset_left _ _ X Y) hX) m ≤
+  𝓇 hX m + 𝓇 hY m :=
+begin
+  have hXXuY : X ⊆ X ∪ Y := @subset_union_left _ _ X Y,
+  have hYXuY : Y ⊆ X ∪ Y := @subset_union_right _ _ X Y,
+  have hXiYX : X ∩ Y ⊆ X := @inter_subset_left _ _ X Y,
+  have hXuY : X ∪ Y ⊆ E := union_subset hX hY,
+  have hXiY : X ∩ Y ⊆ E := subset.trans hXiYX hX,
+  let bXuY := 𝔹 hXuY m, let bXiY := 𝔹 hXiY m,
+  let bX := 𝔹 hX m, let bY := 𝔹 hY m,
+  unfold rank_of_subset,
+  have bXuYs := 𝔹ₛ hXuY m, have bXiYs := 𝔹ₛ hXiY m,
+  have bXs := 𝔹ₛ hX m, have bYs := 𝔹ₛ hY m,
+  simp only [bases_bases_of_indep, mem_powerset, filter_congr_decidable, mem_filter]
+    at bXuYs bXiYs bXs bYs,
+  have rXiY : 𝓇 hXiY m = card bXiY := by simp only [rank_of_subset],
+  have hiu : X ∩ Y ⊆ X ∪ Y := subset.trans hXiYX hXXuY,
+  have hbXiY : bXiY ∈ (m ¦ hXuY).indep := mem_of_subset
+    (restriction_subset_restriction hiu (m ¦ hXuY)) ((restriction_trans hiu hXuY m) ▸ bXiYs.2.1),
+  have HbbXiY := exists_basis_containing_indep hbXiY,
+  exact exists.elim HbbXiY (by { intros B hB,
+    have rXuY : 𝓇 hXuY m = card B := by { simp only [rank_of_subset],
+      exact bases_of_indep_card_eq bXuYs.2 hB.2 },
+    have hBXuY : B ⊆ X ∪ Y := mem_powerset.mp ((m ¦ hXuY).indep_subset_powerset_ground hB.2.1),
+    have hBX : B ∩ X ∈ (m ¦ hX).indep := have hsub : _ := restriction_trans hXXuY hXuY m,
+      have hBX : _ := ((m ¦ hXuY).indep_of_subset_indep hB.2.1 $ @inter_subset_left _ _ B X),
+      hsub.symm ▸ (subset_restriction_indep hBX (@inter_subset_right _ _ B X) hXXuY),
+    have hBY : B ∩ Y ∈ (m ¦ hY).indep := have hsub : _ := restriction_trans hYXuY hXuY m,
+      have hBY : _ := ((m ¦ hXuY).indep_of_subset_indep hB.2.1 $ @inter_subset_left _ _ B Y),
+      hsub.symm ▸ (subset_restriction_indep hBY (@inter_subset_right _ _ B Y) hYXuY),
+    have hBXr : card (B ∩ X) ≤ 𝓇 hX m := by { unfold rank_of_subset,
+      exact card_of_indep_le_card_basis hBX bXs.2 },
+    have hBYr : card (B ∩ Y) ≤ 𝓇 hY m := by { unfold rank_of_subset,
+      exact card_of_indep_le_card_basis hBY bYs.2 },
+    have hinter : (B ∩ X) ∩ (B ∩ Y) = B ∩ X ∩ Y := by simp only [finset.inter_assoc,
+      inter_right_comm, inter_self, inter_comm, inter_left_comm],
+    have hBXiY : B ∩ X ∩ Y = bXiY :=
+      by { have hsub : B ∩ X ∩ Y ⊆ bXiY :=
+        by { by_contra h,
+        exact exists.elim (exists_mem_of_ne_empty $ (mt subset_iff_sdiff_eq_empty.mpr) h)
+          (by { intros a ha, rw [mem_sdiff, inter_assoc, mem_inter] at ha, unfold is_basis at bXiYs,
+          have := ssubset_insert ha.2,
+          have hbXiYsubXiY : insert a bXiY ⊆ X ∩ Y:= insert_subset.mpr ⟨ha.1.2, bXiYs.1⟩,
+          have hrestrict : (m ¦ hXiY) = (m ¦ hXuY ¦ hiu) := restriction_trans hiu hXuY m,
+          have hindep : insert a bXiY ∈ (m ¦ hXiY).indep := hrestrict.symm ▸
+            (subset_restriction_indep ((m ¦ hXuY).indep_of_subset_indep hB.2.1
+            $ insert_subset.mpr ⟨ha.1.1, hB.1⟩) hbXiYsubXiY hiu),
+          exact bXiYs.2.2 (insert a bXiY) hbXiYsubXiY this hindep }) },
+      have hsuper : bXiY ⊆ B ∩ X ∩ Y :=
+        by { rw [inter_assoc],
+        have := inter_subset_inter_right hB.1,
+        have h : bXiY ∩ (X ∩ Y) = bXiY := inter_of_subset bXiYs.1,
+        exact h ▸ this },
+      exact subset.antisymm hsub hsuper },
+    exact calc 𝓇 hX m + 𝓇 hY m ≥ card (B ∩ X) + card (B ∩ Y) : add_le_add hBXr hBYr
+    ... = card ((B ∩ X) ∪ (B ∩ Y)) + card ((B ∩ X) ∩ (B ∩ Y)) : card_union_inter (B ∩ X) (B ∩ Y)
+    ... = card (B ∩ (X ∪ Y)) + card (B ∩ X ∩ Y) : by rw [←inter_distrib_left, hinter]
+    ... = card B + card bXiY : by rw [inter_of_subset hBXuY, hBXiY]
+    ... = 𝓇 hXuY m + 𝓇 hXiY m : by rw [rXuY, rXiY] })
+end
+
+end encodable
+
+structure rank (ground : finset α) :=
+(r {X : finset α} (hX : X ⊆ ground) : ℕ)
+-- (R1)
+(bounded {X : finset α} (hX : X ⊆ ground) : 0 ≤ r hX ∧ r hX ≤ card X)
+-- (R2)
+(order_preserving {X Y : finset α} (hXY : X ⊆ Y) (hY : Y ⊆ ground) : r (subset.trans hXY hY) ≤ r hY)
+-- (R3)
+(submodular {X Y : finset α} (hX : X ⊆ ground) (hY : Y ⊆ ground) :
+r (union_subset hX hY) + r (subset.trans (@inter_subset_left _ _ X Y) hX) ≤ r hX + r hY)
+
+section encodable
+variable [encodable α]
+
+def rank_of_indep (m : indep E) : rank E :=
+⟨λ X hX, rank_of_subset hX m,
+λ X hX, ⟨dec_trivial, (by { have := basis_of_subset_spec hX m,
+  simp only [bases_bases_of_indep, mem_powerset, filter_congr_decidable, mem_filter] at this,
+  exact card_le_of_subset this.1 })⟩,
+λ X Y hXY hY, R2_of_indep m hXY hY,
+λ X Y hX hY, R3_of_indep m hX hY⟩
+
+end encodable
+
+structure rank_R2_R3 (ground : finset α) :=
+(r {X : finset α} (hX : X ⊆ ground) : ℕ)
+-- (R2)
+(order_preserving {X Y : finset α} (hXY : X ⊆ Y) (hY : Y ⊆ ground) : r (subset.trans hXY hY) ≤ r hY)
+-- (R3)
+(submodular {X Y : finset α} (hX : X ⊆ ground) (hY : Y ⊆ ground) :
+r (union_subset hX hY) + r (subset.trans (@inter_subset_left _ _ X Y) hX) ≤ r hX + r hY)
+
+lemma congr_for_rank (rk : rank_R2_R3 E ) {X Y : finset α} (hX : X ⊆ E) (hY : Y ⊆ E) (h : X = Y) :
+rk.r hX = rk.r hY :=
+by { congr, exact h }
+
+-- Lemma 1.3.3
+lemma rank_union_lemma (rk : rank_R2_R3 E) {X Y : finset α} (hX : X ⊆ E) (hY : Y ⊆ E)
+  (hy : ∀ y, ∀ (h : y ∈ Y \ X), rk.r (by { rw mem_sdiff at h,
+    exact insert_subset.mpr ⟨mem_of_subset hY h.1, hX⟩ }) = rk.r hX) :
+  rk.r (union_subset hX hY) = rk.r hX :=
+begin
+  have hXuY : X ∪ Y ⊆ E := union_subset hX hY,
+  induction h : (Y \ X) using finset.induction with a S ha ih generalizing X Y,
+  { congr, have H := congr_arg (λ x, X ∪ x) h,
+    simp only [union_sdiff_self_eq_union, union_empty] at H, exact H },
+  { have h₁ : rk.r hX + rk.r hX ≥ rk.r hXuY + rk.r hX :=
+    by { have haa : a ∈ Y \ X := h.substr (mem_insert_self a S),
+    have haX : insert a X ⊆ E := insert_subset.mpr ⟨mem_of_subset hY (mem_sdiff.mp haa).1, hX⟩,
+    have hins : insert a S ⊆ E := h ▸ subset.trans (sdiff_subset Y X) hY,
+    have hS : S ⊆ E := subset.trans (subset_insert a S) hins,
+    have hXS : X ∪ S ⊆ E := union_subset hX hS,
+    have hrins : rk.r haX = rk.r hX := hy a haa, rw mem_sdiff at haa,
+    have hrS : rk.r hXS = rk.r hX := by {
+      exact ih hX hS (by { intros y Hy, have : y ∈ Y \ X := by { rw mem_sdiff at Hy,
+        simp only [ext, mem_insert, mem_sdiff] at h,
+        exact mem_sdiff.mpr ((h y).mpr $ or.inr Hy.1) }, exact hy y this })
+        hXS (by { simp only [ext, mem_insert, mem_sdiff] at h ⊢,
+          exact λ y, iff.intro (λ Hy, Hy.1) $ λ Hy, ⟨Hy, ((h y).mpr $ or.inr Hy).2⟩ }) },
+    have hXuSiaX : (X ∪ S) ∩ insert a X ⊆ E := (subset.trans (@inter_subset_right _ _ (X ∪ S)
+      (insert a X)) haX),
+    have hr₁ : rk.r (union_subset hXS haX) = rk.r hXuY :=
+      by { exact congr_for_rank rk (union_subset hXS haX) hXuY (by {
+        simp only [ext, mem_union, union_comm, mem_insert, mem_sdiff, union_insert,
+          union_self, union_assoc] at h ⊢,
+      exact λ x, iff.intro (λ hx, or.elim hx (λ hxa, or.inr $ hxa.substr haa.1) $
+        λ H, or.elim H (by { intro hxS, exact or.inr ((h x).mpr $ or.inr hxS).1}) $
+          by {exact (λ hxX, or.inl hxX) }) $
+        λ hx, or.elim hx (by {intro hxX, exact or.inr (or.inr hxX)}) $
+          by { intro hxY, by_cases hxX : x ∈ X,
+            { exact or.inr (or.inr hxX) },
+            { exact or.elim ((h x).mp ⟨hxY, hxX⟩) (λ H, or.inl H)
+              (λ HS, or.inr $ or.inl HS) } } }) },
+    have hr₂ : rk.r hXuSiaX = rk.r hX := by { congr,
+      simp only [ext, mem_union, union_comm, mem_insert, mem_inter],
+      exact λ x, iff.intro (λ hx, or.elim hx.1 (or.elim hx.2
+        (λ H₁ H₂, false.elim $ ha $ H₁.subst H₂) $ λ h _, h) id) (λ hx, ⟨or.inr hx, or.inr hx⟩) },
+    calc rk.r hX + rk.r hX = rk.r hXS + rk.r haX : by rw [hrS, hrins]
+    ... ≥ rk.r (union_subset hXS haX) + rk.r hXuSiaX : rk.submodular (union_subset hX hS) haX
+    ... = _ : by rw [hr₁, hr₂] },
+  replace h₁ := le_of_add_le_add_right h₁,
+  have h₂ : rk.r hX ≤ rk.r hXuY := rk.order_preserving (@subset_union_left _ _ X Y) hXuY,
+  exact nat.le_antisymm h₁ h₂ }
+end
+
+def indep_of_rank (r : rank E) : indep E :=
+⟨sorry,
+sorry,
+sorry,
+sorry,
+sorry⟩
+
+end matroid
